Tame some over-eager tactics

examples/dll_dupleton.v
@@ -12,23 +12,23 @@ Inductive dll (x : ptr) (z : ptr) (s : seq nat) (h : heap) : Prop :=
   @perm_eq nat_eqType (s) (nil) /\ h = empty
 | dll_2 of (x == null) = false of
   exists (v : nat) (s1 : seq nat) (w : ptr),
-  exists h_dll_wxs1_552,
-  @perm_eq nat_eqType (s) ([:: v] ++ s1) /\ h = x :-> v \+ x .+ 1 :-> w \+ x .+ 2 :-> z \+ h_dll_wxs1_552 /\ dll w x s1 h_dll_wxs1_552.
+  exists h_dll_wxs1_551,
+  @perm_eq nat_eqType (s) ([:: v] ++ s1) /\ h = x :-> v \+ x .+ 1 :-> w \+ x .+ 2 :-> z \+ h_dll_wxs1_551 /\ dll w x s1 h_dll_wxs1_551.
 
 Inductive sll (x : ptr) (s : seq nat) (h : heap) : Prop :=
 | sll_1 of x == null of
   @perm_eq nat_eqType (s) (nil) /\ h = empty
 | sll_2 of (x == null) = false of
   exists (v : nat) (s1 : seq nat) (nxt : ptr),
-  exists h_sll_nxts1_553,
-  @perm_eq nat_eqType (s) ([:: v] ++ s1) /\ h = x :-> v \+ x .+ 1 :-> nxt \+ h_sll_nxts1_553 /\ sll nxt s1 h_sll_nxts1_553.
+  exists h_sll_nxts1_552,
+  @perm_eq nat_eqType (s) ([:: v] ++ s1) /\ h = x :-> v \+ x .+ 1 :-> nxt \+ h_sll_nxts1_552 /\ sll nxt s1 h_sll_nxts1_552.
 
-Lemma dll_perm_eq_trans39 x z h s_1 s_2 : perm_eq s_1 s_2 -> dll x z s_1 h -> dll x z s_2 h. Admitted.
-Hint Resolve dll_perm_eq_trans39: ssl_pred.
-Lemma sll_perm_eq_trans40 x h s_1 s_2 : perm_eq s_1 s_2 -> sll x s_1 h -> sll x s_2 h. Admitted.
-Hint Resolve sll_perm_eq_trans40: ssl_pred.
-Lemma pure41 x y : @perm_eq nat_eqType ([:: x; y]) ([:: y] ++ [:: x]). Admitted.
-Hint Resolve pure41: ssl_pure.
+Lemma dll_perm_eq_trans30 x z h s_1 s_2 : perm_eq s_1 s_2 -> dll x z s_1 h -> dll x z s_2 h. Admitted.
+Hint Resolve dll_perm_eq_trans30: ssl_pred.
+Lemma sll_perm_eq_trans31 x h s_1 s_2 : perm_eq s_1 s_2 -> sll x s_1 h -> sll x s_2 h. Admitted.
+Hint Resolve sll_perm_eq_trans31: ssl_pred.
+Lemma pure32 x y : @perm_eq nat_eqType ([:: x; y]) ([:: y] ++ [:: x]). Admitted.
+Hint Resolve pure32: ssl_pure.
 
 Definition dll_dupleton_type :=
   forall (vprogs : nat * nat * ptr),
@@ -42,14 +42,15 @@ Definition dll_dupleton_type :=
       let: (x, y, r) := vprogs in
       let: (a) := vghosts in
       exists elems z,
-      exists h_dll_zelems_554,
-      @perm_eq nat_eqType (elems) ([:: x; y]) /\ h = r :-> z \+ h_dll_zelems_554 /\ dll z null elems h_dll_zelems_554
+      exists h_dll_zelems_553,
+      @perm_eq nat_eqType (elems) ([:: x; y]) /\ h = r :-> z \+ h_dll_zelems_553 /\ dll z null elems h_dll_zelems_553
     ]).
 
 Program Definition dll_dupleton : dll_dupleton_type :=
   Fix (fun (dll_dupleton : dll_dupleton_type) vprogs =>
     let: (x, y, r) := vprogs in
     Do (
+      a2 <-- @read ptr r;
       z2 <-- allocb null 3;
       wz2 <-- allocb null 3;
       r ::= z2;;
@@ -64,12 +65,34 @@ Program Definition dll_dupleton : dll_dupleton_type :=
 Obligation Tactic := intro; move=>[[x y] r]; ssl_program_simpl.
 Next Obligation.
 ssl_ghostelim_pre.
-move=>a2.
+move=>a.
 move=>[sigma_self].
 subst h_self.
 ssl_ghostelim_post.
+try rename h_dll_zelems_553 into h_dll_zxy_553.
+try rename H_dll_zelems_553 into H_dll_zxy_553.
+ssl_read r.
+try rename a into a2.
+try rename h_dll_wzzs1z_551z into h_dll_wzzvwzs1wz_551z.
+try rename H_dll_wzzs1z_551z into H_dll_wzzvwzs1wz_551z.
+try rename h_dll_wwzwzs1wz_551wz into h_dll_wwzwz_551wz.
+try rename H_dll_wwzwzs1wz_551wz into H_dll_wwzwz_551wz.
+try rename h_dll_wzzvwzs1wz_551z into h_dll_wzzvwz_551z.
+try rename H_dll_wzzvwzs1wz_551z into H_dll_wzzvwz_551z.
+try rename h_dll_wwzwz_551wz into h_dll_wz_551wz.
+try rename H_dll_wwzwz_551wz into H_dll_wz_551wz.
 ssl_alloc z2.
+try rename z into z2.
+try rename h_dll_wzzvwz_551z into h_dll_wzz2vwz_551z.
+try rename H_dll_wzzvwz_551z into H_dll_wzz2vwz_551z.
+try rename h_dll_zxy_553 into h_dll_z2xy_553.
+try rename H_dll_zxy_553 into H_dll_z2xy_553.
 ssl_alloc wz2.
+try rename wz into wz2.
+try rename h_dll_wzz2vwz_551z into h_dll_wz2z2vwz_551z.
+try rename H_dll_wzz2vwz_551z into H_dll_wz2z2vwz_551z.
+try rename h_dll_wz_551wz into h_dll_wz2_551wz.
+try rename H_dll_wz_551wz into H_dll_wz2_551wz.
 ssl_write r.
 ssl_write_post r.
 ssl_write (z2 .+ 1).
@@ -80,6 +103,8 @@ ssl_write (wz2 .+ 1).
 ssl_write_post (wz2 .+ 1).
 ssl_write (wz2 .+ 2).
 ssl_write_post (wz2 .+ 2).
+try rename h_dll_wz2z2vwz_551z into h_dll_wz2z2x_551z.
+try rename H_dll_wz2z2vwz_551z into H_dll_wz2z2x_551z.
 ssl_write z2.
 ssl_write_post z2.
 ssl_write wz2.
@@ -87,18 +112,13 @@ ssl_write_post wz2.
 ssl_emp;
 exists ([:: x; y]), (z2);
 exists (z2 :-> y \+ z2 .+ 1 :-> wz2 \+ z2 .+ 2 :-> null \+ wz2 :-> x \+ wz2 .+ 1 :-> null \+ wz2 .+ 2 :-> z2);
-sslauto;
-solve [
+sslauto.
 unfold_constructor 2;
-exists (y), ([:: x] ++ nil), (wz2);
-exists (wz2 :-> x \+ wz2 .+ 1 :-> null \+ wz2 .+ 2 :-> z2);
-sslauto;
-solve [
+exists (y), ([:: x] ++ nil), (wz2), (wz2 :-> x \+ wz2 .+ 1 :-> null \+ wz2 .+ 2 :-> z2);
+sslauto.
 unfold_constructor 2;
-exists (x), (nil), (null);
-exists (empty);
-sslauto;
-solve [
+exists (x), (nil), (null), (empty);
+sslauto.
 unfold_constructor 1;
-sslauto ] ] ].
+sslauto.
 Qed.
