examples/dll_singleton.v
@@ -12,23 +12,23 @@ Inductive dll (x : ptr) (z : ptr) (s : seq nat) (h : heap) : Prop :=
   @perm_eq nat_eqType (s) (nil) /\ h = empty
 | dll_2 of (x == null) = false of
   exists (v : nat) (s1 : seq nat) (w : ptr),
-  exists h_dll_wxs1_555,
-  @perm_eq nat_eqType (s) ([:: v] ++ s1) /\ h = x :-> v \+ x .+ 1 :-> w \+ x .+ 2 :-> z \+ h_dll_wxs1_555 /\ dll w x s1 h_dll_wxs1_555.
+  exists h_dll_wxs1_554,
+  @perm_eq nat_eqType (s) ([:: v] ++ s1) /\ h = x :-> v \+ x .+ 1 :-> w \+ x .+ 2 :-> z \+ h_dll_wxs1_554 /\ dll w x s1 h_dll_wxs1_554.
 
 Inductive sll (x : ptr) (s : seq nat) (h : heap) : Prop :=
 | sll_1 of x == null of
   @perm_eq nat_eqType (s) (nil) /\ h = empty
 | sll_2 of (x == null) = false of
   exists (v : nat) (s1 : seq nat) (nxt : ptr),
-  exists h_sll_nxts1_556,
-  @perm_eq nat_eqType (s) ([:: v] ++ s1) /\ h = x :-> v \+ x .+ 1 :-> nxt \+ h_sll_nxts1_556 /\ sll nxt s1 h_sll_nxts1_556.
+  exists h_sll_nxts1_555,
+  @perm_eq nat_eqType (s) ([:: v] ++ s1) /\ h = x :-> v \+ x .+ 1 :-> nxt \+ h_sll_nxts1_555 /\ sll nxt s1 h_sll_nxts1_555.
 
-Lemma dll_perm_eq_trans42 x z h s_1 s_2 : perm_eq s_1 s_2 -> dll x z s_1 h -> dll x z s_2 h. Admitted.
-Hint Resolve dll_perm_eq_trans42: ssl_pred.
-Lemma sll_perm_eq_trans43 x h s_1 s_2 : perm_eq s_1 s_2 -> sll x s_1 h -> sll x s_2 h. Admitted.
-Hint Resolve sll_perm_eq_trans43: ssl_pred.
-Lemma pure44 x : @perm_eq nat_eqType ([:: x]) ([:: x]). Admitted.
-Hint Resolve pure44: ssl_pure.
+Lemma dll_perm_eq_trans33 x z h s_1 s_2 : perm_eq s_1 s_2 -> dll x z s_1 h -> dll x z s_2 h. Admitted.
+Hint Resolve dll_perm_eq_trans33: ssl_pred.
+Lemma sll_perm_eq_trans34 x h s_1 s_2 : perm_eq s_1 s_2 -> sll x s_1 h -> sll x s_2 h. Admitted.
+Hint Resolve sll_perm_eq_trans34: ssl_pred.
+Lemma pure35 x : @perm_eq nat_eqType ([:: x]) ([:: x]). Admitted.
+Hint Resolve pure35: ssl_pure.
 
 Definition dll_singleton_type :=
   forall (vprogs : nat * ptr),
@@ -42,14 +42,15 @@ Definition dll_singleton_type :=
       let: (x, r) := vprogs in
       let: (a) := vghosts in
       exists elems y,
-      exists h_dll_yelems_557,
-      @perm_eq nat_eqType (elems) ([:: x]) /\ h = r :-> y \+ h_dll_yelems_557 /\ dll y null elems h_dll_yelems_557
+      exists h_dll_yelems_556,
+      @perm_eq nat_eqType (elems) ([:: x]) /\ h = r :-> y \+ h_dll_yelems_556 /\ dll y null elems h_dll_yelems_556
     ]).
 
 Program Definition dll_singleton : dll_singleton_type :=
   Fix (fun (dll_singleton : dll_singleton_type) vprogs =>
     let: (x, r) := vprogs in
     Do (
+      a2 <-- @read ptr r;
       y2 <-- allocb null 3;
       r ::= y2;;
       (y2 .+ 1) ::= null;;
@@ -60,11 +61,24 @@ Program Definition dll_singleton : dll_singleton_type :=
 Obligation Tactic := intro; move=>[x r]; ssl_program_simpl.
 Next Obligation.
 ssl_ghostelim_pre.
-move=>a2.
+move=>a.
 move=>[sigma_self].
 subst h_self.
 ssl_ghostelim_post.
+try rename h_dll_yelems_556 into h_dll_yx_556.
+try rename H_dll_yelems_556 into H_dll_yx_556.
+ssl_read r.
+try rename a into a2.
+try rename h_dll_wyys1y_554y into h_dll_wyy_554y.
+try rename H_dll_wyys1y_554y into H_dll_wyy_554y.
+try rename h_dll_wyy_554y into h_dll_y_554y.
+try rename H_dll_wyy_554y into H_dll_y_554y.
 ssl_alloc y2.
+try rename y into y2.
+try rename h_dll_y_554y into h_dll_y2_554y.
+try rename H_dll_y_554y into H_dll_y2_554y.
+try rename h_dll_yx_556 into h_dll_y2x_556.
+try rename H_dll_yx_556 into H_dll_y2x_556.
 ssl_write r.
 ssl_write_post r.
 ssl_write (y2 .+ 1).
@@ -76,13 +90,10 @@ ssl_write_post y2.
 ssl_emp;
 exists ([:: x]), (y2);
 exists (y2 :-> x \+ y2 .+ 1 :-> null \+ y2 .+ 2 :-> null);
-sslauto;
-solve [
+sslauto.
 unfold_constructor 2;
-exists (x), (nil), (null);
-exists (empty);
-sslauto;
-solve [
+exists (x), (nil), (null), (empty);
+sslauto.
 unfold_constructor 1;
-sslauto ] ].
+sslauto.
 Qed.
