examples/sll_append.v
@@ -12,13 +12,13 @@ Inductive sll (x : ptr) (s : seq nat) (h : heap) : Prop :=
   @perm_eq nat_eqType (s) (nil) /\ h = empty
 | sll_2 of (x == null) = false of
   exists (v : nat) (s1 : seq nat) (nxt : ptr),
-  exists h_sll_nxts1_543,
-  @perm_eq nat_eqType (s) ([:: v] ++ s1) /\ h = x :-> v \+ x .+ 1 :-> nxt \+ h_sll_nxts1_543 /\ sll nxt s1 h_sll_nxts1_543.
+  exists h_sll_nxts1_542,
+  @perm_eq nat_eqType (s) ([:: v] ++ s1) /\ h = x :-> v \+ x .+ 1 :-> nxt \+ h_sll_nxts1_542 /\ sll nxt s1 h_sll_nxts1_542.
 
-Lemma sll_perm_eq_trans32 x h s_1 s_2 : perm_eq s_1 s_2 -> sll x s_1 h -> sll x s_2 h. Admitted.
-Hint Resolve sll_perm_eq_trans32: ssl_pred.
-Lemma pure33 vx12 s1x1 s2 : @perm_eq nat_eqType ([:: vx12] ++ s1x1 ++ s2) ([:: vx12] ++ s1x1 ++ s2). Admitted.
-Hint Resolve pure33: ssl_pure.
+Lemma sll_perm_eq_trans23 x h s_1 s_2 : perm_eq s_1 s_2 -> sll x s_1 h -> sll x s_2 h. Admitted.
+Hint Resolve sll_perm_eq_trans23: ssl_pred.
+Lemma pure24 vx12 s1x1 s2 : @perm_eq nat_eqType ([:: vx12] ++ s1x1 ++ s2) ([:: vx12] ++ s1x1 ++ s2). Admitted.
+Hint Resolve pure24: ssl_pure.
 
 Definition sll_append_type :=
   forall (vprogs : ptr * ptr),
@@ -27,24 +27,26 @@ Definition sll_append_type :=
     fun h =>
       let: (x1, r) := vprogs in
       let: (s1, x2, s2) := vghosts in
-      exists h_sll_x1s1_544 h_sll_x2s2_545,
-      h = r :-> x2 \+ h_sll_x1s1_544 \+ h_sll_x2s2_545 /\ sll x1 s1 h_sll_x1s1_544 /\ sll x2 s2 h_sll_x2s2_545,
+      exists h_sll_x1s1_543 h_sll_x2s2_544,
+      h = r :-> x2 \+ h_sll_x1s1_543 \+ h_sll_x2s2_544 /\ sll x1 s1 h_sll_x1s1_543 /\ sll x2 s2 h_sll_x2s2_544,
     [vfun (_: unit) h =>
       let: (x1, r) := vprogs in
       let: (s1, x2, s2) := vghosts in
       exists s y,
-      exists h_sll_ys_546,
-      @perm_eq nat_eqType (s) (s1 ++ s2) /\ h = r :-> y \+ h_sll_ys_546 /\ sll y s h_sll_ys_546
+      exists h_sll_ys_545,
+      @perm_eq nat_eqType (s) (s1 ++ s2) /\ h = r :-> y \+ h_sll_ys_545 /\ sll y s h_sll_ys_545
     ]).
 
 Program Definition sll_append : sll_append_type :=
   Fix (fun (sll_append : sll_append_type) vprogs =>
     let: (x1, r) := vprogs in
     Do (
+      x22 <-- @read ptr r;
       if x1 == null
       then
         ret tt
       else
+        vx12 <-- @read nat x1;
         nxtx12 <-- @read ptr (x1 .+ 1);
         sll_append (nxtx12, r);;
         y12 <-- @read ptr r;
@@ -55,53 +57,92 @@ Program Definition sll_append : sll_append_type :=
 Obligation Tactic := intro; move=>[x1 r]; ssl_program_simpl.
 Next Obligation.
 ssl_ghostelim_pre.
-move=>[[s1 x22] s2].
-ex_elim h_sll_x1s1_544 h_sll_x22s2_545.
+move=>[[s1 x2] s2].
+ex_elim h_sll_x1s1_543 h_sll_x2s2_544.
 move=>[sigma_self].
 subst h_self.
-move=>[H_sll_x1s1_544 H_sll_x22s2_545].
+move=>[H_sll_x1s1_543 H_sll_x2s2_544].
 ssl_ghostelim_post.
-ssl_open (x1 == null);
-ssl_open_post H_sll_x1s1_544.
-move=>[phi_sll_x1s1_5440].
-move=>[sigma_sll_x1s1_544].
-subst h_sll_x1s1_544.
+try rename h_sll_ys_545 into h_sll_ys1s2_545.
+try rename H_sll_ys_545 into H_sll_ys1s2_545.
+ssl_read r.
+try rename x2 into x22.
+try rename h_sll_x2s2_544 into h_sll_x22s2_544.
+try rename H_sll_x2s2_544 into H_sll_x22s2_544.
+ssl_open (x1 == null) H_sll_x1s1_543.
+move=>[phi_sll_x1s1_5430].
+move=>[sigma_sll_x1s1_543].
+subst h_sll_x1s1_543.
+shelve.
+ex_elim vx1 s1x1 nxtx1.
+ex_elim h_sll_nxtx1s1x1_542x1.
+move=>[phi_sll_x1s1_5430].
+move=>[sigma_sll_x1s1_543].
+subst h_sll_x1s1_543.
+move=>H_sll_nxtx1s1x1_542x1.
+shelve.
+Unshelve.
+try rename h_sll_ys1s2_545 into h_sll_ys2_545.
+try rename H_sll_ys1s2_545 into H_sll_ys2_545.
+try rename h_sll_x1s1_543 into h_sll_x1_543.
+try rename H_sll_x1s1_543 into H_sll_x1_543.
+try rename h_sll_ys2_545 into h_sll_ys2_544.
+try rename H_sll_ys2_545 into H_sll_ys2_544.
+try rename h_sll_ys2_544 into h_sll_x22s2_544.
+try rename H_sll_ys2_544 into H_sll_x22s2_544.
 ssl_emp;
 exists (nil ++ s2), (x22);
-exists (h_sll_x22s2_545);
+exists (h_sll_x22s2_544);
 sslauto.
-ex_elim vx12 s1x1 nxtx12.
-ex_elim h_sll_nxtx12s1x1_543x1.
-move=>[phi_sll_x1s1_5440].
-move=>[sigma_sll_x1s1_544].
-subst h_sll_x1s1_544.
-move=>H_sll_nxtx12s1x1_543x1.
+try rename h_sll_ys1s2_545 into h_sll_yvx1s1x1s2_545.
+try rename H_sll_ys1s2_545 into H_sll_yvx1s1x1s2_545.
+try rename h_sll_x1s1_543 into h_sll_x1vx1s1x1_543.
+try rename H_sll_x1s1_543 into H_sll_x1vx1s1x1_543.
+ssl_read x1.
+try rename vx1 into vx12.
+try rename h_sll_yvx1s1x1s2_545 into h_sll_yvx12s1x1s2_545.
+try rename H_sll_yvx1s1x1s2_545 into H_sll_yvx12s1x1s2_545.
+try rename h_sll_x1vx1s1x1_543 into h_sll_x1vx12s1x1_543.
+try rename H_sll_x1vx1s1x1_543 into H_sll_x1vx12s1x1_543.
 ssl_read (x1 .+ 1).
-ssl_call_pre (r :-> x22 \+ h_sll_nxtx12s1x1_543x1 \+ h_sll_x22s2_545).
+try rename nxtx1 into nxtx12.
+try rename h_sll_nxtx1s1x1_542x1 into h_sll_nxtx12s1x1_542x1.
+try rename H_sll_nxtx1s1x1_542x1 into H_sll_nxtx12s1x1_542x1.
+ssl_call_pre (r :-> x22 \+ h_sll_nxtx12s1x1_542x1 \+ h_sll_x22s2_544).
 ssl_call (s1x1, x22, s2).
-exists (h_sll_nxtx12s1x1_543x1);
-exists (h_sll_x22s2_545);
+exists (h_sll_nxtx12s1x1_542x1), (h_sll_x22s2_544);
 sslauto.
-move=>h_call1.
-ex_elim s3 y12.
-ex_elim h_sll_y12s1x1s2_5461.
-move=>[phi_call10].
-move=>[sigma_call1].
-subst h_call1.
-move=>H_sll_y12s3_5461.
+move=>h_call0.
+ex_elim s3 y1.
+ex_elim h_sll_y1s3_5451.
+move=>[phi_call00].
+move=>[sigma_call0].
+subst h_call0.
+move=>H_sll_y1s3_5451.
 store_valid.
+try rename h_sll_y1s3_5451 into h_sll_y1s1x1s2_5451.
+try rename H_sll_y1s3_5451 into H_sll_y1s1x1s2_5451.
 ssl_read r.
+try rename y1 into y12.
+try rename h_sll_y1s1x1s2_5451 into h_sll_y12s1x1s2_5451.
+try rename H_sll_y1s1x1s2_5451 into H_sll_y12s1x1s2_5451.
+try rename h_sll_nxtys12y_542y into h_sll_nxtys12y_5451.
+try rename H_sll_nxtys12y_542y into H_sll_nxtys12y_5451.
+try rename h_sll_nxtys12y_5451 into h_sll_y12s12y_5451.
+try rename H_sll_nxtys12y_5451 into H_sll_y12s12y_5451.
+try rename h_sll_y12s12y_5451 into h_sll_y12s1x1s2_5451.
+try rename H_sll_y12s12y_5451 into H_sll_y12s1x1s2_5451.
+try rename h_sll_yvx12s1x1s2_545 into h_sll_x1vx12s1x1s2_545.
+try rename H_sll_yvx12s1x1s2_545 into H_sll_x1vx12s1x1s2_545.
 ssl_write (x1 .+ 1).
 ssl_write_post (x1 .+ 1).
 ssl_write r.
 ssl_write_post r.
 ssl_emp;
 exists ([:: vx12] ++ s1x1 ++ s2), (x1);
-exists (x1 :-> vx12 \+ x1 .+ 1 :-> y12 \+ h_sll_y12s1x1s2_5461);
-sslauto;
-solve [
+exists (x1 :-> vx12 \+ x1 .+ 1 :-> y12 \+ h_sll_y12s1x1s2_5451);
+sslauto.
 unfold_constructor 2;
-exists (vx12), (s1x1 ++ s2), (y12);
-exists (h_sll_y12s1x1s2_5461);
-sslauto ].
+exists (vx12), (s1x1 ++ s2), (y12), (h_sll_y12s1x1s2_5451);
+sslauto.
 Qed.
