examples/sll_copy.v
@@ -12,19 +12,19 @@ Inductive sll (x : ptr) (s : seq nat) (h : heap) : Prop :=
   @perm_eq nat_eqType (s) (nil) /\ h = empty
 | sll_2 of (x == null) = false of
   exists (v : nat) (s1 : seq nat) (nxt : ptr),
-  exists h_sll_nxts1_540,
-  @perm_eq nat_eqType (s) ([:: v] ++ s1) /\ h = x :-> v \+ x .+ 1 :-> nxt \+ h_sll_nxts1_540 /\ sll nxt s1 h_sll_nxts1_540.
+  exists h_sll_nxts1_539,
+  @perm_eq nat_eqType (s) ([:: v] ++ s1) /\ h = x :-> v \+ x .+ 1 :-> nxt \+ h_sll_nxts1_539 /\ sll nxt s1 h_sll_nxts1_539.
 
-Lemma sll_perm_eq_trans26 x h s_1 s_2 : perm_eq s_1 s_2 -> sll x s_1 h -> sll x s_2 h. Admitted.
-Hint Resolve sll_perm_eq_trans26: ssl_pred.
-Lemma pure27 : @perm_eq nat_eqType (nil) (nil). Admitted.
-Hint Resolve pure27: ssl_pure.
-Lemma pure28 b1 : b1 < b1 + 1. Admitted.
-Hint Resolve pure28: ssl_pure.
-Lemma pure29 vx22 s1x2 : @perm_eq nat_eqType ([:: vx22] ++ s1x2) ([:: vx22] ++ s1x2). Admitted.
-Hint Resolve pure29: ssl_pure.
-Lemma pure30 vx22 s1x2 : @perm_eq nat_eqType ([:: vx22] ++ s1x2) ([:: vx22] ++ s1x2). Admitted.
-Hint Resolve pure30: ssl_pure.
+Lemma sll_perm_eq_trans17 x h s_1 s_2 : perm_eq s_1 s_2 -> sll x s_1 h -> sll x s_2 h. Admitted.
+Hint Resolve sll_perm_eq_trans17: ssl_pred.
+Lemma pure18 : @perm_eq nat_eqType (nil) (nil). Admitted.
+Hint Resolve pure18: ssl_pure.
+Lemma pure19 b1 : b1 < b1 + 1. Admitted.
+Hint Resolve pure19: ssl_pure.
+Lemma pure20 vx22 s1x2 : @perm_eq nat_eqType ([:: vx22] ++ s1x2) ([:: vx22] ++ s1x2). Admitted.
+Hint Resolve pure20: ssl_pure.
+Lemma pure21 vx22 s1x2 : @perm_eq nat_eqType ([:: vx22] ++ s1x2) ([:: vx22] ++ s1x2). Admitted.
+Hint Resolve pure21: ssl_pure.
 
 Definition sll_copy_type :=
   forall (vprogs : ptr),
@@ -66,50 +66,90 @@ Program Definition sll_copy : sll_copy_type :=
 Obligation Tactic := intro; move=>r; ssl_program_simpl.
 Next Obligation.
 ssl_ghostelim_pre.
-move=>[x2 s].
-ex_elim h_sll_x2s_a.
+move=>[x s].
+ex_elim h_sll_xs_a.
 move=>[sigma_self].
 subst h_self.
-move=>H_sll_x2s_a.
+move=>H_sll_xs_a.
 ssl_ghostelim_post.
 ssl_read r.
-ssl_open (x2 == null);
-ssl_open_post H_sll_x2s_a.
+try rename x into x2.
+try rename h_sll_xs_a into h_sll_x2s_a.
+try rename H_sll_xs_a into H_sll_x2s_a.
+ssl_open (x2 == null) H_sll_x2s_a.
 move=>[phi_sll_x2s_a0].
 move=>[sigma_sll_x2s_a].
 subst h_sll_x2s_a.
+shelve.
+ex_elim vx2 s1x2 nxtx2.
+ex_elim h_sll_nxtx2s1x2_539x2.
+move=>[phi_sll_x2s_a0].
+move=>[sigma_sll_x2s_a].
+subst h_sll_x2s_a.
+move=>H_sll_nxtx2s1x2_539x2.
+shelve.
+Unshelve.
+try rename h_sll_ys_b into h_sll_y_b.
+try rename H_sll_ys_b into H_sll_y_b.
+try rename h_sll_x2s_a into h_sll_x2_a.
+try rename H_sll_x2s_a into H_sll_x2_a.
+try rename h_sll_y_b into h_sll__b.
+try rename H_sll_y_b into H_sll__b.
 ssl_emp;
 exists (null);
 exists (empty);
 exists (empty);
-sslauto;
-solve [
-unfold_constructor 1;
-sslauto |
-unfold_constructor 1;
-sslauto ].
-ex_elim vx22 s1x2 nxtx22.
-ex_elim h_sll_nxtx22s1x2_540x2.
-move=>[phi_sll_x2s_a0].
-move=>[sigma_sll_x2s_a].
-subst h_sll_x2s_a.
-move=>H_sll_nxtx22s1x2_540x2.
-ssl_read x2.
-ssl_read (x2 .+ 1).
-ssl_write r.
-ssl_call_pre (r :-> nxtx22 \+ h_sll_nxtx22s1x2_540x2).
-ssl_call (nxtx22, s1x2).
-exists (h_sll_nxtx22s1x2_540x2);
 sslauto.
-move=>h_call1.
-ex_elim y12.
-ex_elim h_sll_nxtx22s1x2_540x2 h_sll_y12s1x2_b1.
-move=>[sigma_call1].
-subst h_call1.
-move=>[H_sll_nxtx22s1x2_540x2 H_sll_y12s1x2_b1].
+unfold_constructor 1;
+sslauto.
+unfold_constructor 1;
+sslauto.
+try rename h_sll_ys_b into h_sll_yvx2s1x2_b.
+try rename H_sll_ys_b into H_sll_yvx2s1x2_b.
+try rename h_sll_x2s_a into h_sll_x2vx2s1x2_a.
+try rename H_sll_x2s_a into H_sll_x2vx2s1x2_a.
+ssl_read x2.
+try rename vx2 into vx22.
+try rename h_sll_x2vx2s1x2_a into h_sll_x2vx22s1x2_a.
+try rename H_sll_x2vx2s1x2_a into H_sll_x2vx22s1x2_a.
+try rename h_sll_yvx2s1x2_b into h_sll_yvx22s1x2_b.
+try rename H_sll_yvx2s1x2_b into H_sll_yvx22s1x2_b.
+ssl_read (x2 .+ 1).
+try rename nxtx2 into nxtx22.
+try rename h_sll_nxtx2s1x2_539x2 into h_sll_nxtx22s1x2_539x2.
+try rename H_sll_nxtx2s1x2_539x2 into H_sll_nxtx22s1x2_539x2.
+ssl_write r.
+ssl_call_pre (r :-> nxtx22 \+ h_sll_nxtx22s1x2_539x2).
+ssl_call (nxtx22, s1x2).
+exists (h_sll_nxtx22s1x2_539x2);
+sslauto.
+move=>h_call0.
+ex_elim y1.
+ex_elim h_sll_nxtx22s1x2_539x2 h_sll_y1s1x2_b1.
+move=>[sigma_call0].
+subst h_call0.
+move=>[H_sll_nxtx22s1x2_539x2 H_sll_y1s1x2_b1].
 store_valid.
 ssl_read r.
+try rename y1 into y12.
+try rename h_sll_y1s1x2_b1 into h_sll_y12s1x2_b1.
+try rename H_sll_y1s1x2_b1 into H_sll_y12s1x2_b1.
+try rename h_sll_nxtx21s11x2_539x21 into h_sll_nxtx21s11x2_539x2.
+try rename H_sll_nxtx21s11x2_539x21 into H_sll_nxtx21s11x2_539x2.
+try rename h_sll_nxtx21s11x2_539x2 into h_sll_nxtx22s11x2_539x2.
+try rename H_sll_nxtx21s11x2_539x2 into H_sll_nxtx22s11x2_539x2.
+try rename h_sll_nxtx22s11x2_539x2 into h_sll_nxtx22s1x2_539x2.
+try rename H_sll_nxtx22s11x2_539x2 into H_sll_nxtx22s1x2_539x2.
+try rename h_sll_nxtys11y_539y into h_sll_nxtys11y_b1.
+try rename H_sll_nxtys11y_539y into H_sll_nxtys11y_b1.
+try rename h_sll_nxtys11y_b1 into h_sll_y12s11y_b1.
+try rename H_sll_nxtys11y_b1 into H_sll_y12s11y_b1.
+try rename h_sll_y12s11y_b1 into h_sll_y12s1x2_b1.
+try rename H_sll_y12s11y_b1 into H_sll_y12s1x2_b1.
 ssl_alloc y2.
+try rename y into y2.
+try rename h_sll_yvx22s1x2_b into h_sll_y2vx22s1x2_b.
+try rename H_sll_yvx22s1x2_b into H_sll_y2vx22s1x2_b.
 ssl_write r.
 ssl_write_post r.
 ssl_write (y2 .+ 1).
@@ -118,16 +158,13 @@ ssl_write y2.
 ssl_write_post y2.
 ssl_emp;
 exists (y2);
-exists (x2 :-> vx22 \+ x2 .+ 1 :-> nxtx22 \+ h_sll_nxtx22s1x2_540x2);
+exists (x2 :-> vx22 \+ x2 .+ 1 :-> nxtx22 \+ h_sll_nxtx22s1x2_539x2);
 exists (y2 :-> vx22 \+ y2 .+ 1 :-> y12 \+ h_sll_y12s1x2_b1);
-sslauto;
-solve [
+sslauto.
 unfold_constructor 2;
-exists (vx22), (s1x2), (nxtx22);
-exists (h_sll_nxtx22s1x2_540x2);
-sslauto |
+exists (vx22), (s1x2), (nxtx22), (h_sll_nxtx22s1x2_539x2);
+sslauto.
 unfold_constructor 2;
-exists (vx22), (s1x2), (y12);
-exists (h_sll_y12s1x2_b1);
-sslauto ].
+exists (vx22), (s1x2), (y12), (h_sll_y12s1x2_b1);
+sslauto.
 Qed.
