examples/sll_len.v
@@ -12,19 +12,19 @@ Inductive sll (x : ptr) (len : nat) (lo : nat) (hi : nat) (h : heap) : Prop :=
   hi == 0 /\ len == 0 /\ lo == 7 /\ h = empty
 | sll_2 of (x == null) = false of
   exists (len1 : nat) (v : nat) (hi1 : nat) (lo1 : nat) (nxt : ptr),
-  exists h_sll_nxtlen1lo1hi1_513,
-  0 <= len1 /\ 0 <= v /\ hi == (if hi1 <= v then v else hi1) /\ len == 1 + len1 /\ lo == (if v <= lo1 then v else lo1) /\ v <= 7 /\ h = x :-> v \+ x .+ 1 :-> nxt \+ h_sll_nxtlen1lo1hi1_513 /\ sll nxt len1 lo1 hi1 h_sll_nxtlen1lo1hi1_513.
+  exists h_sll_nxtlen1lo1hi1_516,
+  0 <= len1 /\ 0 <= v /\ hi == (if hi1 <= v then v else hi1) /\ len == 1 + len1 /\ lo == (if v <= lo1 then v else lo1) /\ v <= 7 /\ h = x :-> v \+ x .+ 1 :-> nxt \+ h_sll_nxtlen1lo1hi1_516 /\ sll nxt len1 lo1 hi1 h_sll_nxtlen1lo1hi1_516.
 
-Lemma pure1 : 0 == 0. Admitted.
-Hint Resolve pure1: ssl_pure.
-Lemma pure2 : 7 == 7. Admitted.
-Hint Resolve pure2: ssl_pure.
-Lemma pure3 len1x2 : 0 <= 1 + len1x2 -> 0 <= len1x2 -> 1 + len1x2 == 1 + len1x2. Admitted.
-Hint Resolve pure3: ssl_pure.
-Lemma pure4 hi1x vx2 : vx2 <= 7 -> 0 <= vx2 -> (if hi1x <= vx2 then vx2 else hi1x) == (if hi1x <= vx2 then vx2 else hi1x). Admitted.
-Hint Resolve pure4: ssl_pure.
-Lemma pure5 vx2 lo1x : vx2 <= 7 -> 0 <= vx2 -> (if vx2 <= lo1x then vx2 else lo1x) == (if vx2 <= lo1x then vx2 else lo1x). Admitted.
-Hint Resolve pure5: ssl_pure.
+Lemma pure6 : 0 == 0. Admitted.
+Hint Resolve pure6: ssl_pure.
+Lemma pure7 : 7 == 7. Admitted.
+Hint Resolve pure7: ssl_pure.
+Lemma pure8 len1x2 : 0 <= 1 + len1x2 -> 0 <= len1x2 -> 1 + len1x2 == 1 + len1x2. Admitted.
+Hint Resolve pure8: ssl_pure.
+Lemma pure9 hi1x vx2 : 0 <= vx2 -> vx2 <= 7 -> (if hi1x <= vx2 then vx2 else hi1x) == (if hi1x <= vx2 then vx2 else hi1x). Admitted.
+Hint Resolve pure9: ssl_pure.
+Lemma pure10 vx2 lo1x : 0 <= vx2 -> vx2 <= 7 -> (if vx2 <= lo1x then vx2 else lo1x) == (if vx2 <= lo1x then vx2 else lo1x). Admitted.
+Hint Resolve pure10: ssl_pure.
 
 Definition sll_len_type :=
   forall (vprogs : ptr * ptr),
@@ -33,24 +33,26 @@ Definition sll_len_type :=
     fun h =>
       let: (x, r) := vprogs in
       let: (n, lo, hi, a) := vghosts in
-      exists h_sll_xnlohi_514,
-      0 <= n /\ h = r :-> a \+ h_sll_xnlohi_514 /\ sll x n lo hi h_sll_xnlohi_514,
+      exists h_sll_xnlohi_517,
+      0 <= n /\ h = r :-> a \+ h_sll_xnlohi_517 /\ sll x n lo hi h_sll_xnlohi_517,
     [vfun (_: unit) h =>
       let: (x, r) := vprogs in
       let: (n, lo, hi, a) := vghosts in
-      exists h_sll_xnlohi_515,
-      h = r :-> n \+ h_sll_xnlohi_515 /\ sll x n lo hi h_sll_xnlohi_515
+      exists h_sll_xnlohi_518,
+      h = r :-> n \+ h_sll_xnlohi_518 /\ sll x n lo hi h_sll_xnlohi_518
     ]).
 
 Program Definition sll_len : sll_len_type :=
   Fix (fun (sll_len : sll_len_type) vprogs =>
     let: (x, r) := vprogs in
     Do (
+      a2 <-- @read ptr r;
       if x == null
       then
         r ::= 0;;
         ret tt
       else
+        vx2 <-- @read nat x;
         nxtx2 <-- @read ptr (x .+ 1);
         sll_len (nxtx2, r);;
         len1x2 <-- @read nat r;
@@ -60,52 +62,105 @@ Program Definition sll_len : sll_len_type :=
 Obligation Tactic := intro; move=>[x r]; ssl_program_simpl.
 Next Obligation.
 ssl_ghostelim_pre.
-move=>[[[n lo] hi] a2].
-ex_elim h_sll_xnlohi_514.
+move=>[[[n lo] hi] a].
+ex_elim h_sll_xnlohi_517.
 move=>[phi_self0].
 move=>[sigma_self].
 subst h_self.
-move=>H_sll_xnlohi_514.
+move=>H_sll_xnlohi_517.
 ssl_ghostelim_post.
-ssl_open (x == null);
-ssl_open_post H_sll_xnlohi_514.
-move=>[phi_sll_xnlohi_5140] [phi_sll_xnlohi_5141] [phi_sll_xnlohi_5142].
-move=>[sigma_sll_xnlohi_514].
-subst h_sll_xnlohi_514.
+ssl_read r.
+try rename a into a2.
+ssl_open (x == null) H_sll_xnlohi_517.
+move=>[phi_sll_xnlohi_5170] [phi_sll_xnlohi_5171] [phi_sll_xnlohi_5172].
+move=>[sigma_sll_xnlohi_517].
+subst h_sll_xnlohi_517.
+shelve.
+ex_elim len1x vx hi1x lo1x nxtx.
+ex_elim h_sll_nxtxlen1xlo1xhi1x_516x.
+move=>[phi_sll_xnlohi_5170] [phi_sll_xnlohi_5171] [phi_sll_xnlohi_5172] [phi_sll_xnlohi_5173] [phi_sll_xnlohi_5174] [phi_sll_xnlohi_5175].
+move=>[sigma_sll_xnlohi_517].
+subst h_sll_xnlohi_517.
+move=>H_sll_nxtxlen1xlo1xhi1x_516x.
+shelve.
+Unshelve.
+try rename h_sll_xnlohi_517 into h_sll_xnlo_517.
+try rename H_sll_xnlohi_517 into H_sll_xnlo_517.
+try rename h_sll_xnlohi_518 into h_sll_xnlo_518.
+try rename H_sll_xnlohi_518 into H_sll_xnlo_518.
+try rename h_sll_xnlo_517 into h_sll_xn_517.
+try rename H_sll_xnlo_517 into H_sll_xn_517.
+try rename h_sll_xnlo_518 into h_sll_xn_518.
+try rename H_sll_xnlo_518 into H_sll_xn_518.
+try rename h_sll_xn_517 into h_sll_x_517.
+try rename H_sll_xn_517 into H_sll_x_517.
+try rename h_sll_xn_518 into h_sll_x_518.
+try rename H_sll_xn_518 into H_sll_x_518.
 ssl_write r.
 ssl_write_post r.
 ssl_emp;
 exists (empty);
-sslauto;
-solve [
-unfold_constructor 1;
-sslauto ].
-ex_elim len1x2 vx2 hi1x lo1x nxtx2.
-ex_elim h_sll_nxtx2len1x2lo1xhi1x_513x.
-move=>[phi_sll_xnlohi_5140] [phi_sll_xnlohi_5141] [phi_sll_xnlohi_5142] [phi_sll_xnlohi_5143] [phi_sll_xnlohi_5144] [phi_sll_xnlohi_5145].
-move=>[sigma_sll_xnlohi_514].
-subst h_sll_xnlohi_514.
-move=>H_sll_nxtx2len1x2lo1xhi1x_513x.
-ssl_read (x .+ 1).
-ssl_call_pre (r :-> a2 \+ h_sll_nxtx2len1x2lo1xhi1x_513x).
-ssl_call (len1x2, lo1x, hi1x, a2).
-exists (h_sll_nxtx2len1x2lo1xhi1x_513x);
 sslauto.
-move=>h_call1.
-ex_elim h_sll_nxtx2len1x2lo1xhi1x_5151.
-move=>[sigma_call1].
-subst h_call1.
-move=>H_sll_nxtx2len1x2lo1xhi1x_5151.
+unfold_constructor 1;
+sslauto.
+try rename h_sll_xnlohi_517 into h_sll_xnlohi1xvxvxhi1x_517.
+try rename H_sll_xnlohi_517 into H_sll_xnlohi1xvxvxhi1x_517.
+try rename h_sll_xnlohi_518 into h_sll_xnlohi1xvxvxhi1x_518.
+try rename H_sll_xnlohi_518 into H_sll_xnlohi1xvxvxhi1x_518.
+try rename h_sll_xnlohi1xvxvxhi1x_517 into h_sll_xnvxlo1xvxlo1xhi1xvxvxhi1x_517.
+try rename H_sll_xnlohi1xvxvxhi1x_517 into H_sll_xnvxlo1xvxlo1xhi1xvxvxhi1x_517.
+try rename h_sll_xnlohi1xvxvxhi1x_518 into h_sll_xnvxlo1xvxlo1xhi1xvxvxhi1x_518.
+try rename H_sll_xnlohi1xvxvxhi1x_518 into H_sll_xnvxlo1xvxlo1xhi1xvxvxhi1x_518.
+try rename h_sll_xnvxlo1xvxlo1xhi1xvxvxhi1x_517 into h_sll_xlen1xvxlo1xvxlo1xhi1xvxvxhi1x_517.
+try rename H_sll_xnvxlo1xvxlo1xhi1xvxvxhi1x_517 into H_sll_xlen1xvxlo1xvxlo1xhi1xvxvxhi1x_517.
+try rename h_sll_xnvxlo1xvxlo1xhi1xvxvxhi1x_518 into h_sll_xlen1xvxlo1xvxlo1xhi1xvxvxhi1x_518.
+try rename H_sll_xnvxlo1xvxlo1xhi1xvxvxhi1x_518 into H_sll_xlen1xvxlo1xvxlo1xhi1xvxvxhi1x_518.
+ssl_read x.
+try rename vx into vx2.
+try rename h_sll_xlen1xvxlo1xvxlo1xhi1xvxvxhi1x_518 into h_sll_xlen1xvx2lo1xvx2lo1xhi1xvx2vx2hi1x_518.
+try rename H_sll_xlen1xvxlo1xvxlo1xhi1xvxvxhi1x_518 into H_sll_xlen1xvx2lo1xvx2lo1xhi1xvx2vx2hi1x_518.
+try rename h_sll_xlen1xvxlo1xvxlo1xhi1xvxvxhi1x_517 into h_sll_xlen1xvx2lo1xvx2lo1xhi1xvx2vx2hi1x_517.
+try rename H_sll_xlen1xvxlo1xvxlo1xhi1xvxvxhi1x_517 into H_sll_xlen1xvx2lo1xvx2lo1xhi1xvx2vx2hi1x_517.
+ssl_read (x .+ 1).
+try rename nxtx into nxtx2.
+try rename h_sll_nxtxlen1xlo1xhi1x_516x into h_sll_nxtx2len1xlo1xhi1x_516x.
+try rename H_sll_nxtxlen1xlo1xhi1x_516x into H_sll_nxtx2len1xlo1xhi1x_516x.
+ssl_call_pre (r :-> a2 \+ h_sll_nxtx2len1xlo1xhi1x_516x).
+ssl_call (len1x, lo1x, hi1x, a2).
+exists (h_sll_nxtx2len1xlo1xhi1x_516x);
+sslauto.
+move=>h_call0.
+ex_elim h_sll_nxtx2len1xlo1xhi1x_5181.
+move=>[sigma_call0].
+subst h_call0.
+move=>H_sll_nxtx2len1xlo1xhi1x_5181.
 store_valid.
 ssl_read r.
+try rename len1x into len1x2.
+try rename h_sll_xlen1xvx2lo1xvx2lo1xhi1xvx2vx2hi1x_518 into h_sll_xlen1x2vx2lo1xvx2lo1xhi1xvx2vx2hi1x_518.
+try rename H_sll_xlen1xvx2lo1xvx2lo1xhi1xvx2vx2hi1x_518 into H_sll_xlen1x2vx2lo1xvx2lo1xhi1xvx2vx2hi1x_518.
+try rename h_sll_nxtx2len1xlo1xhi1x_5181 into h_sll_nxtx2len1x2lo1xhi1x_5181.
+try rename H_sll_nxtx2len1xlo1xhi1x_5181 into H_sll_nxtx2len1x2lo1xhi1x_5181.
+try rename h_sll_xlen1xvx2lo1xvx2lo1xhi1xvx2vx2hi1x_517 into h_sll_xlen1x2vx2lo1xvx2lo1xhi1xvx2vx2hi1x_517.
+try rename H_sll_xlen1xvx2lo1xvx2lo1xhi1xvx2vx2hi1x_517 into H_sll_xlen1x2vx2lo1xvx2lo1xhi1xvx2vx2hi1x_517.
+try rename h_sll_nxtx2len1xlo1xhi1x_516x into h_sll_nxtx2len1x2lo1xhi1x_516x.
+try rename H_sll_nxtx2len1xlo1xhi1x_516x into H_sll_nxtx2len1x2lo1xhi1x_516x.
+try rename h_sll_nxtx1len1x1lo11xhi11x_516x1 into h_sll_nxtx1len1x1lo11xhi11x_5181.
+try rename H_sll_nxtx1len1x1lo11xhi11x_516x1 into H_sll_nxtx1len1x1lo11xhi11x_5181.
+try rename h_sll_nxtx1len1x1lo11xhi11x_5181 into h_sll_nxtx1len1x1lo11xhi1x_5181.
+try rename H_sll_nxtx1len1x1lo11xhi11x_5181 into H_sll_nxtx1len1x1lo11xhi1x_5181.
+try rename h_sll_nxtx1len1x1lo11xhi1x_5181 into h_sll_nxtx1len1x2lo11xhi1x_5181.
+try rename H_sll_nxtx1len1x1lo11xhi1x_5181 into H_sll_nxtx1len1x2lo11xhi1x_5181.
+try rename h_sll_nxtx1len1x2lo11xhi1x_5181 into h_sll_nxtx1len1x2lo1xhi1x_5181.
+try rename H_sll_nxtx1len1x2lo11xhi1x_5181 into H_sll_nxtx1len1x2lo1xhi1x_5181.
+try rename h_sll_nxtx1len1x2lo1xhi1x_5181 into h_sll_nxtx2len1x2lo1xhi1x_5181.
+try rename H_sll_nxtx1len1x2lo1xhi1x_5181 into H_sll_nxtx2len1x2lo1xhi1x_5181.
 ssl_write r.
 ssl_write_post r.
 ssl_emp;
-exists (x :-> vx2 \+ x .+ 1 :-> nxtx2 \+ h_sll_nxtx2len1x2lo1xhi1x_5151);
-sslauto;
-solve [
+exists (x :-> vx2 \+ x .+ 1 :-> nxtx2 \+ h_sll_nxtx2len1x2lo1xhi1x_5181);
+sslauto.
 unfold_constructor 2;
-exists (len1x2), (vx2), (hi1x), (lo1x), (nxtx2);
-exists (h_sll_nxtx2len1x2lo1xhi1x_5151);
-sslauto ].
+exists (len1x2), (vx2), (hi1x), (lo1x), (nxtx2), (h_sll_nxtx2len1x2lo1xhi1x_5181);
+sslauto.
 Qed.
