examples/sll_max.v
@@ -12,19 +12,19 @@ Inductive sll (x : ptr) (len : nat) (lo : nat) (hi : nat) (h : heap) : Prop :=
   hi == 0 /\ len == 0 /\ lo == 7 /\ h = empty
 | sll_2 of (x == null) = false of
   exists (len1 : nat) (v : nat) (hi1 : nat) (lo1 : nat) (nxt : ptr),
-  exists h_sll_nxtlen1lo1hi1_513,
-  0 <= len1 /\ 0 <= v /\ hi == (if hi1 <= v then v else hi1) /\ len == 1 + len1 /\ lo == (if v <= lo1 then v else lo1) /\ v <= 7 /\ h = x :-> v \+ x .+ 1 :-> nxt \+ h_sll_nxtlen1lo1hi1_513 /\ sll nxt len1 lo1 hi1 h_sll_nxtlen1lo1hi1_513.
+  exists h_sll_nxtlen1lo1hi1_519,
+  0 <= len1 /\ 0 <= v /\ hi == (if hi1 <= v then v else hi1) /\ len == 1 + len1 /\ lo == (if v <= lo1 then v else lo1) /\ v <= 7 /\ h = x :-> v \+ x .+ 1 :-> nxt \+ h_sll_nxtlen1lo1hi1_519 /\ sll nxt len1 lo1 hi1 h_sll_nxtlen1lo1hi1_519.
 
-Lemma pure1 : 0 == 0. Admitted.
-Hint Resolve pure1: ssl_pure.
-Lemma pure2 : 7 == 7. Admitted.
-Hint Resolve pure2: ssl_pure.
-Lemma pure3 len1x : 0 <= len1x -> 1 + len1x == 1 + len1x. Admitted.
-Hint Resolve pure3: ssl_pure.
-Lemma pure4 hi1x2 vx2 : vx2 <= 7 -> 0 <= vx2 -> (if hi1x2 <= vx2 then vx2 else hi1x2) == (if hi1x2 <= vx2 then vx2 else hi1x2). Admitted.
-Hint Resolve pure4: ssl_pure.
-Lemma pure5 vx2 lo1x : vx2 <= 7 -> 0 <= vx2 -> (if vx2 <= lo1x then vx2 else lo1x) == (if vx2 <= lo1x then vx2 else lo1x). Admitted.
-Hint Resolve pure5: ssl_pure.
+Lemma pure11 : 0 == 0. Admitted.
+Hint Resolve pure11: ssl_pure.
+Lemma pure12 : 7 == 7. Admitted.
+Hint Resolve pure12: ssl_pure.
+Lemma pure13 len1x : 0 <= len1x -> 1 + len1x == 1 + len1x. Admitted.
+Hint Resolve pure13: ssl_pure.
+Lemma pure14 hi1x2 vx2 : 0 <= vx2 -> vx2 <= 7 -> (if hi1x2 <= vx2 then vx2 else hi1x2) == (if hi1x2 <= vx2 then vx2 else hi1x2). Admitted.
+Hint Resolve pure14: ssl_pure.
+Lemma pure15 vx2 lo1x : 0 <= vx2 -> vx2 <= 7 -> (if vx2 <= lo1x then vx2 else lo1x) == (if vx2 <= lo1x then vx2 else lo1x). Admitted.
+Hint Resolve pure15: ssl_pure.
 
 Definition sll_max_type :=
   forall (vprogs : ptr * ptr),
@@ -33,19 +33,20 @@ Definition sll_max_type :=
     fun h =>
       let: (x, r) := vprogs in
       let: (n, lo, hi, a) := vghosts in
-      exists h_sll_xnlohi_514,
-      h = r :-> a \+ h_sll_xnlohi_514 /\ sll x n lo hi h_sll_xnlohi_514,
+      exists h_sll_xnlohi_520,
+      h = r :-> a \+ h_sll_xnlohi_520 /\ sll x n lo hi h_sll_xnlohi_520,
     [vfun (_: unit) h =>
       let: (x, r) := vprogs in
       let: (n, lo, hi, a) := vghosts in
-      exists h_sll_xnlohi_515,
-      h = r :-> hi \+ h_sll_xnlohi_515 /\ sll x n lo hi h_sll_xnlohi_515
+      exists h_sll_xnlohi_521,
+      h = r :-> hi \+ h_sll_xnlohi_521 /\ sll x n lo hi h_sll_xnlohi_521
     ]).
 
 Program Definition sll_max : sll_max_type :=
   Fix (fun (sll_max : sll_max_type) vprogs =>
     let: (x, r) := vprogs in
     Do (
+      a2 <-- @read ptr r;
       if x == null
       then
         r ::= 0;;
@@ -61,52 +62,104 @@ Program Definition sll_max : sll_max_type :=
 Obligation Tactic := intro; move=>[x r]; ssl_program_simpl.
 Next Obligation.
 ssl_ghostelim_pre.
-move=>[[[n lo] hi] a2].
-ex_elim h_sll_xnlohi_514.
+move=>[[[n lo] hi] a].
+ex_elim h_sll_xnlohi_520.
 move=>[sigma_self].
 subst h_self.
-move=>H_sll_xnlohi_514.
+move=>H_sll_xnlohi_520.
 ssl_ghostelim_post.
-ssl_open (x == null);
-ssl_open_post H_sll_xnlohi_514.
-move=>[phi_sll_xnlohi_5140] [phi_sll_xnlohi_5141] [phi_sll_xnlohi_5142].
-move=>[sigma_sll_xnlohi_514].
-subst h_sll_xnlohi_514.
+ssl_read r.
+try rename a into a2.
+ssl_open (x == null) H_sll_xnlohi_520.
+move=>[phi_sll_xnlohi_5200] [phi_sll_xnlohi_5201] [phi_sll_xnlohi_5202].
+move=>[sigma_sll_xnlohi_520].
+subst h_sll_xnlohi_520.
+shelve.
+ex_elim len1x vx hi1x lo1x nxtx.
+ex_elim h_sll_nxtxlen1xlo1xhi1x_519x.
+move=>[phi_sll_xnlohi_5200] [phi_sll_xnlohi_5201] [phi_sll_xnlohi_5202] [phi_sll_xnlohi_5203] [phi_sll_xnlohi_5204] [phi_sll_xnlohi_5205].
+move=>[sigma_sll_xnlohi_520].
+subst h_sll_xnlohi_520.
+move=>H_sll_nxtxlen1xlo1xhi1x_519x.
+shelve.
+Unshelve.
+try rename h_sll_xnlohi_520 into h_sll_xnlo_520.
+try rename H_sll_xnlohi_520 into H_sll_xnlo_520.
+try rename h_sll_xnlohi_521 into h_sll_xnlo_521.
+try rename H_sll_xnlohi_521 into H_sll_xnlo_521.
+try rename h_sll_xnlo_520 into h_sll_xn_520.
+try rename H_sll_xnlo_520 into H_sll_xn_520.
+try rename h_sll_xnlo_521 into h_sll_xn_521.
+try rename H_sll_xnlo_521 into H_sll_xn_521.
+try rename h_sll_xn_521 into h_sll_x_521.
+try rename H_sll_xn_521 into H_sll_x_521.
+try rename h_sll_xn_520 into h_sll_x_520.
+try rename H_sll_xn_520 into H_sll_x_520.
 ssl_write r.
 ssl_write_post r.
 ssl_emp;
 exists (empty);
-sslauto;
-solve [
-unfold_constructor 1;
-sslauto ].
-ex_elim len1x vx2 hi1x2 lo1x nxtx2.
-ex_elim h_sll_nxtx2len1xlo1xhi1x2_513x.
-move=>[phi_sll_xnlohi_5140] [phi_sll_xnlohi_5141] [phi_sll_xnlohi_5142] [phi_sll_xnlohi_5143] [phi_sll_xnlohi_5144] [phi_sll_xnlohi_5145].
-move=>[sigma_sll_xnlohi_514].
-subst h_sll_xnlohi_514.
-move=>H_sll_nxtx2len1xlo1xhi1x2_513x.
-ssl_read x.
-ssl_read (x .+ 1).
-ssl_call_pre (r :-> a2 \+ h_sll_nxtx2len1xlo1xhi1x2_513x).
-ssl_call (len1x, lo1x, hi1x2, a2).
-exists (h_sll_nxtx2len1xlo1xhi1x2_513x);
 sslauto.
-move=>h_call1.
-ex_elim h_sll_nxtx2len1xlo1xhi1x2_5151.
-move=>[sigma_call1].
-subst h_call1.
-move=>H_sll_nxtx2len1xlo1xhi1x2_5151.
+unfold_constructor 1;
+sslauto.
+try rename h_sll_xnlohi_520 into h_sll_xnlohi1xvxvxhi1x_520.
+try rename H_sll_xnlohi_520 into H_sll_xnlohi1xvxvxhi1x_520.
+try rename h_sll_xnlohi_521 into h_sll_xnlohi1xvxvxhi1x_521.
+try rename H_sll_xnlohi_521 into H_sll_xnlohi1xvxvxhi1x_521.
+try rename h_sll_xnlohi1xvxvxhi1x_521 into h_sll_xnvxlo1xvxlo1xhi1xvxvxhi1x_521.
+try rename H_sll_xnlohi1xvxvxhi1x_521 into H_sll_xnvxlo1xvxlo1xhi1xvxvxhi1x_521.
+try rename h_sll_xnlohi1xvxvxhi1x_520 into h_sll_xnvxlo1xvxlo1xhi1xvxvxhi1x_520.
+try rename H_sll_xnlohi1xvxvxhi1x_520 into H_sll_xnvxlo1xvxlo1xhi1xvxvxhi1x_520.
+try rename h_sll_xnvxlo1xvxlo1xhi1xvxvxhi1x_521 into h_sll_xlen1xvxlo1xvxlo1xhi1xvxvxhi1x_521.
+try rename H_sll_xnvxlo1xvxlo1xhi1xvxvxhi1x_521 into H_sll_xlen1xvxlo1xvxlo1xhi1xvxvxhi1x_521.
+try rename h_sll_xnvxlo1xvxlo1xhi1xvxvxhi1x_520 into h_sll_xlen1xvxlo1xvxlo1xhi1xvxvxhi1x_520.
+try rename H_sll_xnvxlo1xvxlo1xhi1xvxvxhi1x_520 into H_sll_xlen1xvxlo1xvxlo1xhi1xvxvxhi1x_520.
+ssl_read x.
+try rename vx into vx2.
+try rename h_sll_xlen1xvxlo1xvxlo1xhi1xvxvxhi1x_520 into h_sll_xlen1xvx2lo1xvx2lo1xhi1xvx2vx2hi1x_520.
+try rename H_sll_xlen1xvxlo1xvxlo1xhi1xvxvxhi1x_520 into H_sll_xlen1xvx2lo1xvx2lo1xhi1xvx2vx2hi1x_520.
+try rename h_sll_xlen1xvxlo1xvxlo1xhi1xvxvxhi1x_521 into h_sll_xlen1xvx2lo1xvx2lo1xhi1xvx2vx2hi1x_521.
+try rename H_sll_xlen1xvxlo1xvxlo1xhi1xvxvxhi1x_521 into H_sll_xlen1xvx2lo1xvx2lo1xhi1xvx2vx2hi1x_521.
+ssl_read (x .+ 1).
+try rename nxtx into nxtx2.
+try rename h_sll_nxtxlen1xlo1xhi1x_519x into h_sll_nxtx2len1xlo1xhi1x_519x.
+try rename H_sll_nxtxlen1xlo1xhi1x_519x into H_sll_nxtx2len1xlo1xhi1x_519x.
+ssl_call_pre (r :-> a2 \+ h_sll_nxtx2len1xlo1xhi1x_519x).
+ssl_call (len1x, lo1x, hi1x, a2).
+exists (h_sll_nxtx2len1xlo1xhi1x_519x);
+sslauto.
+move=>h_call0.
+ex_elim h_sll_nxtx2len1xlo1xhi1x_5211.
+move=>[sigma_call0].
+subst h_call0.
+move=>H_sll_nxtx2len1xlo1xhi1x_5211.
 store_valid.
 ssl_read r.
+try rename hi1x into hi1x2.
+try rename h_sll_nxtx2len1xlo1xhi1x_519x into h_sll_nxtx2len1xlo1xhi1x2_519x.
+try rename H_sll_nxtx2len1xlo1xhi1x_519x into H_sll_nxtx2len1xlo1xhi1x2_519x.
+try rename h_sll_nxtx2len1xlo1xhi1x_5211 into h_sll_nxtx2len1xlo1xhi1x2_5211.
+try rename H_sll_nxtx2len1xlo1xhi1x_5211 into H_sll_nxtx2len1xlo1xhi1x2_5211.
+try rename h_sll_xlen1xvx2lo1xvx2lo1xhi1xvx2vx2hi1x_520 into h_sll_xlen1xvx2lo1xvx2lo1xhi1x2vx2vx2hi1x2_520.
+try rename H_sll_xlen1xvx2lo1xvx2lo1xhi1xvx2vx2hi1x_520 into H_sll_xlen1xvx2lo1xvx2lo1xhi1x2vx2vx2hi1x2_520.
+try rename h_sll_xlen1xvx2lo1xvx2lo1xhi1xvx2vx2hi1x_521 into h_sll_xlen1xvx2lo1xvx2lo1xhi1x2vx2vx2hi1x2_521.
+try rename H_sll_xlen1xvx2lo1xvx2lo1xhi1xvx2vx2hi1x_521 into H_sll_xlen1xvx2lo1xvx2lo1xhi1x2vx2vx2hi1x2_521.
+try rename h_sll_nxtx1len1x1lo11xhi11x_519x1 into h_sll_nxtx1len1x1lo11xhi11x_5211.
+try rename H_sll_nxtx1len1x1lo11xhi11x_519x1 into H_sll_nxtx1len1x1lo11xhi11x_5211.
+try rename h_sll_nxtx1len1x1lo11xhi11x_5211 into h_sll_nxtx1len1x1lo11xhi1x2_5211.
+try rename H_sll_nxtx1len1x1lo11xhi11x_5211 into H_sll_nxtx1len1x1lo11xhi1x2_5211.
+try rename h_sll_nxtx1len1x1lo11xhi1x2_5211 into h_sll_nxtx1len1xlo11xhi1x2_5211.
+try rename H_sll_nxtx1len1x1lo11xhi1x2_5211 into H_sll_nxtx1len1xlo11xhi1x2_5211.
+try rename h_sll_nxtx1len1xlo11xhi1x2_5211 into h_sll_nxtx1len1xlo1xhi1x2_5211.
+try rename H_sll_nxtx1len1xlo11xhi1x2_5211 into H_sll_nxtx1len1xlo1xhi1x2_5211.
+try rename h_sll_nxtx1len1xlo1xhi1x2_5211 into h_sll_nxtx2len1xlo1xhi1x2_5211.
+try rename H_sll_nxtx1len1xlo1xhi1x2_5211 into H_sll_nxtx2len1xlo1xhi1x2_5211.
 ssl_write r.
 ssl_write_post r.
 ssl_emp;
-exists (x :-> vx2 \+ x .+ 1 :-> nxtx2 \+ h_sll_nxtx2len1xlo1xhi1x2_5151);
-sslauto;
-solve [
+exists (x :-> vx2 \+ x .+ 1 :-> nxtx2 \+ h_sll_nxtx2len1xlo1xhi1x2_5211);
+sslauto.
 unfold_constructor 2;
-exists (len1x), (vx2), (hi1x2), (lo1x), (nxtx2);
-exists (h_sll_nxtx2len1xlo1xhi1x2_5151);
-sslauto ].
+exists (len1x), (vx2), (hi1x2), (lo1x), (nxtx2), (h_sll_nxtx2len1xlo1xhi1x2_5211);
+sslauto.
 Qed.
