examples/sll_to_dll.v
@@ -12,27 +12,27 @@ Inductive dll (x : ptr) (z : ptr) (s : seq nat) (h : heap) : Prop :=
   @perm_eq nat_eqType (s) (nil) /\ h = empty
 | dll_2 of (x == null) = false of
   exists (v : nat) (s1 : seq nat) (w : ptr),
-  exists h_dll_wxs1_558,
-  @perm_eq nat_eqType (s) ([:: v] ++ s1) /\ h = x :-> v \+ x .+ 1 :-> w \+ x .+ 2 :-> z \+ h_dll_wxs1_558 /\ dll w x s1 h_dll_wxs1_558.
+  exists h_dll_wxs1_557,
+  @perm_eq nat_eqType (s) ([:: v] ++ s1) /\ h = x :-> v \+ x .+ 1 :-> w \+ x .+ 2 :-> z \+ h_dll_wxs1_557 /\ dll w x s1 h_dll_wxs1_557.
 
 Inductive sll (x : ptr) (s : seq nat) (h : heap) : Prop :=
 | sll_1 of x == null of
   @perm_eq nat_eqType (s) (nil) /\ h = empty
 | sll_2 of (x == null) = false of
   exists (v : nat) (s1 : seq nat) (nxt : ptr),
-  exists h_sll_nxts1_559,
-  @perm_eq nat_eqType (s) ([:: v] ++ s1) /\ h = x :-> v \+ x .+ 1 :-> nxt \+ h_sll_nxts1_559 /\ sll nxt s1 h_sll_nxts1_559.
+  exists h_sll_nxts1_558,
+  @perm_eq nat_eqType (s) ([:: v] ++ s1) /\ h = x :-> v \+ x .+ 1 :-> nxt \+ h_sll_nxts1_558 /\ sll nxt s1 h_sll_nxts1_558.
 
-Lemma dll_perm_eq_trans45 x z h s_1 s_2 : perm_eq s_1 s_2 -> dll x z s_1 h -> dll x z s_2 h. Admitted.
-Hint Resolve dll_perm_eq_trans45: ssl_pred.
-Lemma sll_perm_eq_trans46 x h s_1 s_2 : perm_eq s_1 s_2 -> sll x s_1 h -> sll x s_2 h. Admitted.
-Hint Resolve sll_perm_eq_trans46: ssl_pred.
-Lemma pure47 : @perm_eq nat_eqType (nil) (nil). Admitted.
-Hint Resolve pure47: ssl_pure.
-Lemma pure48 vx22 : @perm_eq nat_eqType ([:: vx22]) ([:: vx22]). Admitted.
-Hint Resolve pure48: ssl_pure.
-Lemma pure49 vx22 vi122 s1i12 : @perm_eq nat_eqType ([:: vx22] ++ [:: vi122] ++ s1i12) ([:: vx22] ++ [:: vi122] ++ s1i12). Admitted.
-Hint Resolve pure49: ssl_pure.
+Lemma dll_perm_eq_trans36 x z h s_1 s_2 : perm_eq s_1 s_2 -> dll x z s_1 h -> dll x z s_2 h. Admitted.
+Hint Resolve dll_perm_eq_trans36: ssl_pred.
+Lemma sll_perm_eq_trans37 x h s_1 s_2 : perm_eq s_1 s_2 -> sll x s_1 h -> sll x s_2 h. Admitted.
+Hint Resolve sll_perm_eq_trans37: ssl_pred.
+Lemma pure38 : @perm_eq nat_eqType (nil) (nil). Admitted.
+Hint Resolve pure38: ssl_pure.
+Lemma pure39 vx22 : @perm_eq nat_eqType ([:: vx22]) ([:: vx22]). Admitted.
+Hint Resolve pure39: ssl_pure.
+Lemma pure40 vx22 vi122 s1i12 : @perm_eq nat_eqType ([:: vx22] ++ [:: vi122] ++ s1i12) ([:: vx22] ++ [:: vi122] ++ s1i12). Admitted.
+Hint Resolve pure40: ssl_pure.
 
 Definition sll_to_dll_type :=
   forall (vprogs : ptr),
@@ -41,14 +41,14 @@ Definition sll_to_dll_type :=
     fun h =>
       let: (f) := vprogs in
       let: (x, s) := vghosts in
-      exists h_sll_xs_560,
-      h = f :-> x \+ h_sll_xs_560 /\ sll x s h_sll_xs_560,
+      exists h_sll_xs_559,
+      h = f :-> x \+ h_sll_xs_559 /\ sll x s h_sll_xs_559,
     [vfun (_: unit) h =>
       let: (f) := vprogs in
       let: (x, s) := vghosts in
       exists i,
-      exists h_dll_is_561,
-      h = f :-> i \+ h_dll_is_561 /\ dll i null s h_dll_is_561
+      exists h_dll_is_560,
+      h = f :-> i \+ h_dll_is_560 /\ dll i null s h_dll_is_560
     ]).
 
 Program Definition sll_to_dll : sll_to_dll_type :=
@@ -76,6 +76,8 @@ Program Definition sll_to_dll : sll_to_dll_type :=
           i2 ::= vx22;;
           ret tt
         else
+          vi122 <-- @read nat i12;
+          wi122 <-- @read ptr (i12 .+ 1);
           i2 <-- allocb null 3;
           dealloc x2;;
           dealloc (x2 .+ 1);;
@@ -89,52 +91,102 @@ Program Definition sll_to_dll : sll_to_dll_type :=
 Obligation Tactic := intro; move=>f; ssl_program_simpl.
 Next Obligation.
 ssl_ghostelim_pre.
-move=>[x2 s].
-ex_elim h_sll_x2s_560.
+move=>[x s].
+ex_elim h_sll_xs_559.
 move=>[sigma_self].
 subst h_self.
-move=>H_sll_x2s_560.
+move=>H_sll_xs_559.
 ssl_ghostelim_post.
 ssl_read f.
-ssl_open (x2 == null);
-ssl_open_post H_sll_x2s_560.
-move=>[phi_sll_x2s_5600].
-move=>[sigma_sll_x2s_560].
-subst h_sll_x2s_560.
+try rename x into x2.
+try rename h_sll_xs_559 into h_sll_x2s_559.
+try rename H_sll_xs_559 into H_sll_x2s_559.
+ssl_open (x2 == null) H_sll_x2s_559.
+move=>[phi_sll_x2s_5590].
+move=>[sigma_sll_x2s_559].
+subst h_sll_x2s_559.
+shelve.
+ex_elim vx2 s1x2 nxtx2.
+ex_elim h_sll_nxtx2s1x2_558x2.
+move=>[phi_sll_x2s_5590].
+move=>[sigma_sll_x2s_559].
+subst h_sll_x2s_559.
+move=>H_sll_nxtx2s1x2_558x2.
+shelve.
+Unshelve.
+try rename h_dll_is_560 into h_dll_i_560.
+try rename H_dll_is_560 into H_dll_i_560.
+try rename h_sll_x2s_559 into h_sll_x2_559.
+try rename H_sll_x2s_559 into H_sll_x2_559.
+try rename h_dll_i_560 into h_dll__560.
+try rename H_dll_i_560 into H_dll__560.
 ssl_emp;
 exists (null);
 exists (empty);
-sslauto;
-solve [
-unfold_constructor 1;
-sslauto ].
-ex_elim vx22 s1x2 nxtx22.
-ex_elim h_sll_nxtx22s1x2_559x2.
-move=>[phi_sll_x2s_5600].
-move=>[sigma_sll_x2s_560].
-subst h_sll_x2s_560.
-move=>H_sll_nxtx22s1x2_559x2.
-ssl_read x2.
-ssl_read (x2 .+ 1).
-ssl_write f.
-ssl_call_pre (f :-> nxtx22 \+ h_sll_nxtx22s1x2_559x2).
-ssl_call (nxtx22, s1x2).
-exists (h_sll_nxtx22s1x2_559x2);
 sslauto.
-move=>h_call1.
-ex_elim i12.
-ex_elim h_dll_i12s1x2_5611.
-move=>[sigma_call1].
-subst h_call1.
-move=>H_dll_i12s1x2_5611.
+unfold_constructor 1;
+sslauto.
+try rename h_dll_is_560 into h_dll_ivx2s1x2_560.
+try rename H_dll_is_560 into H_dll_ivx2s1x2_560.
+try rename h_sll_x2s_559 into h_sll_x2vx2s1x2_559.
+try rename H_sll_x2s_559 into H_sll_x2vx2s1x2_559.
+ssl_read x2.
+try rename vx2 into vx22.
+try rename h_dll_ivx2s1x2_560 into h_dll_ivx22s1x2_560.
+try rename H_dll_ivx2s1x2_560 into H_dll_ivx22s1x2_560.
+try rename h_sll_x2vx2s1x2_559 into h_sll_x2vx22s1x2_559.
+try rename H_sll_x2vx2s1x2_559 into H_sll_x2vx22s1x2_559.
+ssl_read (x2 .+ 1).
+try rename nxtx2 into nxtx22.
+try rename h_sll_nxtx2s1x2_558x2 into h_sll_nxtx22s1x2_558x2.
+try rename H_sll_nxtx2s1x2_558x2 into H_sll_nxtx22s1x2_558x2.
+ssl_write f.
+ssl_call_pre (f :-> nxtx22 \+ h_sll_nxtx22s1x2_558x2).
+ssl_call (nxtx22, s1x2).
+exists (h_sll_nxtx22s1x2_558x2);
+sslauto.
+move=>h_call0.
+ex_elim i1.
+ex_elim h_dll_i1s1x2_5601.
+move=>[sigma_call0].
+subst h_call0.
+move=>H_dll_i1s1x2_5601.
 store_valid.
 ssl_read f.
-ssl_open (i12 == null);
-ssl_open_post H_dll_i12s1x2_5611.
-move=>[phi_dll_i12s1x2_56110].
-move=>[sigma_dll_i12s1x2_5611].
-subst h_dll_i12s1x2_5611.
+try rename i1 into i12.
+try rename h_dll_i1s1x2_5601 into h_dll_i12s1x2_5601.
+try rename H_dll_i1s1x2_5601 into H_dll_i12s1x2_5601.
+ssl_open (i12 == null) H_dll_i12s1x2_5601.
+move=>[phi_dll_i12s1x2_56010].
+move=>[sigma_dll_i12s1x2_5601].
+subst h_dll_i12s1x2_5601.
+shelve.
+ex_elim vi12 s1i12 wi12.
+ex_elim h_dll_wi12i12s1i12_557i12.
+move=>[phi_dll_i12s1x2_56010].
+move=>[sigma_dll_i12s1x2_5601].
+subst h_dll_i12s1x2_5601.
+move=>H_dll_wi12i12s1i12_557i12.
+shelve.
+Unshelve.
+try rename h_dll_ivx22s1x2_560 into h_dll_ivx22_560.
+try rename H_dll_ivx22s1x2_560 into H_dll_ivx22_560.
+try rename h_dll_i12s1x2_5601 into h_dll_i12_5601.
+try rename H_dll_i12s1x2_5601 into H_dll_i12_5601.
+try rename h_sll_x2vx22s1x2_559 into h_sll_x2vx22_559.
+try rename H_sll_x2vx22s1x2_559 into H_sll_x2vx22_559.
+try rename h_sll_nxtx22s1x2_558x2 into h_sll_nxtx22_558x2.
+try rename H_sll_nxtx22s1x2_558x2 into H_sll_nxtx22_558x2.
+try rename h_dll_wiis11i_557i into h_dll_wii_557i.
+try rename H_dll_wiis11i_557i into H_dll_wii_557i.
+try rename h_dll_wii_557i into h_dll_i_557i.
+try rename H_dll_wii_557i into H_dll_i_557i.
 ssl_alloc i2.
+try rename i into i2.
+try rename h_dll_ivx22_560 into h_dll_i2vx22_560.
+try rename H_dll_ivx22_560 into H_dll_i2vx22_560.
+try rename h_dll_i_557i into h_dll_i2_557i.
+try rename H_dll_i_557i into H_dll_i2_557i.
 ssl_dealloc x2.
 ssl_dealloc (x2 .+ 1).
 ssl_write f.
@@ -148,22 +200,54 @@ ssl_write_post i2.
 ssl_emp;
 exists (i2);
 exists (i2 :-> vx22 \+ i2 .+ 1 :-> null \+ i2 .+ 2 :-> null);
-sslauto;
-solve [
+sslauto.
 unfold_constructor 2;
-exists (vx22), (nil), (null);
-exists (empty);
-sslauto;
-solve [
+exists (vx22), (nil), (null), (empty);
+sslauto.
 unfold_constructor 1;
-sslauto ] ].
-ex_elim vi122 s1i12 wi122.
-ex_elim h_dll_wi122i12s1i12_558i12.
-move=>[phi_dll_i12s1x2_56110].
-move=>[sigma_dll_i12s1x2_5611].
-subst h_dll_i12s1x2_5611.
-move=>H_dll_wi122i12s1i12_558i12.
+sslauto.
+try rename h_dll_ivx22s1x2_560 into h_dll_ivx22vi12s1i12_560.
+try rename H_dll_ivx22s1x2_560 into H_dll_ivx22vi12s1i12_560.
+try rename h_dll_i12s1x2_5601 into h_dll_i12vi12s1i12_5601.
+try rename H_dll_i12s1x2_5601 into H_dll_i12vi12s1i12_5601.
+try rename h_sll_x2vx22s1x2_559 into h_sll_x2vx22vi12s1i12_559.
+try rename H_sll_x2vx22s1x2_559 into H_sll_x2vx22vi12s1i12_559.
+try rename h_sll_nxtx22s1x2_558x2 into h_sll_nxtx22vi12s1i12_558x2.
+try rename H_sll_nxtx22s1x2_558x2 into H_sll_nxtx22vi12s1i12_558x2.
+ssl_read i12.
+try rename vi12 into vi122.
+try rename h_sll_x2vx22vi12s1i12_559 into h_sll_x2vx22vi122s1i12_559.
+try rename H_sll_x2vx22vi12s1i12_559 into H_sll_x2vx22vi122s1i12_559.
+try rename h_sll_nxtx22vi12s1i12_558x2 into h_sll_nxtx22vi122s1i12_558x2.
+try rename H_sll_nxtx22vi12s1i12_558x2 into H_sll_nxtx22vi122s1i12_558x2.
+try rename h_dll_i12vi12s1i12_5601 into h_dll_i12vi122s1i12_5601.
+try rename H_dll_i12vi12s1i12_5601 into H_dll_i12vi122s1i12_5601.
+try rename h_dll_ivx22vi12s1i12_560 into h_dll_ivx22vi122s1i12_560.
+try rename H_dll_ivx22vi12s1i12_560 into H_dll_ivx22vi122s1i12_560.
+ssl_read (i12 .+ 1).
+try rename wi12 into wi122.
+try rename h_dll_wi12i12s1i12_557i12 into h_dll_wi122i12s1i12_557i12.
+try rename H_dll_wi12i12s1i12_557i12 into H_dll_wi122i12s1i12_557i12.
+try rename h_dll_wiis11i_557i into h_dll_wiivwis11wi_557i.
+try rename H_dll_wiis11i_557i into H_dll_wiivwis11wi_557i.
+try rename h_dll_wwiwis11wi_557wi into h_dll_wwiwis11wi_557i12.
+try rename H_dll_wwiwis11wi_557wi into H_dll_wwiwis11wi_557i12.
+try rename h_dll_wiivwis11wi_557i into h_dll_i12ivwis11wi_557i.
+try rename H_dll_wiivwis11wi_557i into H_dll_i12ivwis11wi_557i.
+try rename h_dll_wwiwis11wi_557i12 into h_dll_wwii12s11wi_557i12.
+try rename H_dll_wwiwis11wi_557i12 into H_dll_wwii12s11wi_557i12.
+try rename h_dll_wwii12s11wi_557i12 into h_dll_wwii12s1i12_557i12.
+try rename H_dll_wwii12s11wi_557i12 into H_dll_wwii12s1i12_557i12.
+try rename h_dll_i12ivwis11wi_557i into h_dll_i12ivwis1i12_557i.
+try rename H_dll_i12ivwis11wi_557i into H_dll_i12ivwis1i12_557i.
+try rename h_dll_wwii12s1i12_557i12 into h_dll_wi122i12s1i12_557i12.
+try rename H_dll_wwii12s1i12_557i12 into H_dll_wi122i12s1i12_557i12.
 ssl_alloc i2.
+try rename i into i2.
+try rename h_dll_i12ivwis1i12_557i into h_dll_i12i2vwis1i12_557i.
+try rename H_dll_i12ivwis1i12_557i into H_dll_i12i2vwis1i12_557i.
+try rename h_dll_ivx22vi122s1i12_560 into h_dll_i2vx22vi122s1i12_560.
+try rename H_dll_ivx22vi122s1i12_560 into H_dll_i2vx22vi122s1i12_560.
 ssl_dealloc x2.
 ssl_dealloc (x2 .+ 1).
 ssl_write (i12 .+ 2).
@@ -174,20 +258,18 @@ ssl_write (i2 .+ 1).
 ssl_write_post (i2 .+ 1).
 ssl_write (i2 .+ 2).
 ssl_write_post (i2 .+ 2).
+try rename h_dll_i12i2vwis1i12_557i into h_dll_i12i2vi122s1i12_557i.
+try rename H_dll_i12i2vwis1i12_557i into H_dll_i12i2vi122s1i12_557i.
 ssl_write i2.
 ssl_write_post i2.
 ssl_emp;
 exists (i2);
-exists (i2 :-> vx22 \+ i2 .+ 1 :-> i12 \+ i2 .+ 2 :-> null \+ i12 :-> vi122 \+ i12 .+ 1 :-> wi122 \+ i12 .+ 2 :-> i2 \+ h_dll_wi122i12s1i12_558i12);
-sslauto;
-solve [
+exists (i2 :-> vx22 \+ i2 .+ 1 :-> i12 \+ i2 .+ 2 :-> null \+ i12 :-> vi122 \+ i12 .+ 1 :-> wi122 \+ i12 .+ 2 :-> i2 \+ h_dll_wi122i12s1i12_557i12);
+sslauto.
 unfold_constructor 2;
-exists (vx22), ([:: vi122] ++ s1i12), (i12);
-exists (i12 :-> vi122 \+ i12 .+ 1 :-> wi122 \+ i12 .+ 2 :-> i2 \+ h_dll_wi122i12s1i12_558i12);
-sslauto;
-solve [
+exists (vx22), ([:: vi122] ++ s1i12), (i12), (i12 :-> vi122 \+ i12 .+ 1 :-> wi122 \+ i12 .+ 2 :-> i2 \+ h_dll_wi122i12s1i12_557i12);
+sslauto.
 unfold_constructor 2;
-exists (vi122), (s1i12), (wi122);
-exists (h_dll_wi122i12s1i12_558i12);
-sslauto ] ].
+exists (vi122), (s1i12), (wi122), (h_dll_wi122i12s1i12_557i12);
+sslauto.
 Qed.
