examples/tree_copy.v
@@ -12,25 +12,35 @@ Inductive tree (x : ptr) (s : seq nat) (h : heap) : Prop :=
   @perm_eq nat_eqType (s) (nil) /\ h = empty
 | tree_2 of (x == null) = false of
   exists (v : nat) (s1 : seq nat) (s2 : seq nat) (l : ptr) (r : ptr),
-  exists h_tree_ls1_529 h_tree_rs2_530,
-  @perm_eq nat_eqType (s) ([:: v] ++ s1 ++ s2) /\ h = x :-> v \+ x .+ 1 :-> l \+ x .+ 2 :-> r \+ h_tree_ls1_529 \+ h_tree_rs2_530 /\ tree l s1 h_tree_ls1_529 /\ tree r s2 h_tree_rs2_530.
+  exists h_tree_ls1_526 h_tree_rs2_527,
+  @perm_eq nat_eqType (s) ([:: v] ++ s1 ++ s2) /\ h = x :-> v \+ x .+ 1 :-> l \+ x .+ 2 :-> r \+ h_tree_ls1_526 \+ h_tree_rs2_527 /\ tree l s1 h_tree_ls1_526 /\ tree r s2 h_tree_rs2_527.
 
 Inductive treeN (x : ptr) (n : nat) (h : heap) : Prop :=
 | treeN_1 of x == null of
   n == 0 /\ h = empty
 | treeN_2 of (x == null) = false of
   exists (n1 : nat) (n2 : nat) (l : ptr) (r : ptr) (v : ptr),
-  exists h_treeN_ln1_531 h_treeN_rn2_532,
-  0 <= n1 /\ 0 <= n2 /\ n == 1 + n1 + n2 /\ h = x :-> v \+ x .+ 1 :-> l \+ x .+ 2 :-> r \+ h_treeN_ln1_531 \+ h_treeN_rn2_532 /\ treeN l n1 h_treeN_ln1_531 /\ treeN r n2 h_treeN_rn2_532.
+  exists h_treeN_ln1_528 h_treeN_rn2_529,
+  0 <= n1 /\ 0 <= n2 /\ n == 1 + n1 + n2 /\ h = x :-> v \+ x .+ 1 :-> l \+ x .+ 2 :-> r \+ h_treeN_ln1_528 \+ h_treeN_rn2_529 /\ treeN l n1 h_treeN_ln1_528 /\ treeN r n2 h_treeN_rn2_529.
 
-Lemma tree_perm_eq_trans19 x h s_1 s_2 : perm_eq s_1 s_2 -> tree x s_1 h -> tree x s_2 h. Admitted.
-Hint Resolve tree_perm_eq_trans19: ssl_pred.
-Lemma pure20 : @perm_eq nat_eqType (nil) (nil). Admitted.
-Hint Resolve pure20: ssl_pure.
-Lemma pure21 vx22 s1x2 s2x2 : @perm_eq nat_eqType ([:: vx22] ++ s1x2 ++ s2x2) ([:: vx22] ++ s1x2 ++ s2x2). Admitted.
-Hint Resolve pure21: ssl_pure.
-Lemma pure22 vx22 s1x2 s2x2 : @perm_eq nat_eqType ([:: vx22] ++ s1x2 ++ s2x2) ([:: vx22] ++ s1x2 ++ s2x2). Admitted.
-Hint Resolve pure22: ssl_pure.
+Inductive sll (x : ptr) (s : seq nat) (h : heap) : Prop :=
+| sll_1 of x == null of
+  @perm_eq nat_eqType (s) (nil) /\ h = empty
+| sll_2 of (x == null) = false of
+  exists (v : nat) (s1 : seq nat) (nxt : ptr),
+  exists h_sll_nxts1_530,
+  @perm_eq nat_eqType (s) ([:: v] ++ s1) /\ h = x :-> v \+ x .+ 1 :-> nxt \+ h_sll_nxts1_530 /\ sll nxt s1 h_sll_nxts1_530.
+
+Lemma tree_perm_eq_trans8 x h s_1 s_2 : perm_eq s_1 s_2 -> tree x s_1 h -> tree x s_2 h. Admitted.
+Hint Resolve tree_perm_eq_trans8: ssl_pred.
+Lemma sll_perm_eq_trans9 x h s_1 s_2 : perm_eq s_1 s_2 -> sll x s_1 h -> sll x s_2 h. Admitted.
+Hint Resolve sll_perm_eq_trans9: ssl_pred.
+Lemma pure10 : @perm_eq nat_eqType (nil) (nil). Admitted.
+Hint Resolve pure10: ssl_pure.
+Lemma pure11 vx22 s1x2 s2x2 : @perm_eq nat_eqType ([:: vx22] ++ s1x2 ++ s2x2) ([:: vx22] ++ s1x2 ++ s2x2). Admitted.
+Hint Resolve pure11: ssl_pure.
+Lemma pure12 vx22 s1x2 s2x2 : @perm_eq nat_eqType ([:: vx22] ++ s1x2 ++ s2x2) ([:: vx22] ++ s1x2 ++ s2x2). Admitted.
+Hint Resolve pure12: ssl_pure.
 
 Definition tree_copy_type :=
   forall (vprogs : ptr),
@@ -77,64 +87,122 @@ Program Definition tree_copy : tree_copy_type :=
 Obligation Tactic := intro; move=>r; ssl_program_simpl.
 Next Obligation.
 ssl_ghostelim_pre.
-move=>[x2 s].
-ex_elim h_tree_x2s_a.
+move=>[x s].
+ex_elim h_tree_xs_a.
 move=>[sigma_self].
 subst h_self.
-move=>H_tree_x2s_a.
+move=>H_tree_xs_a.
 ssl_ghostelim_post.
 ssl_read r.
-ssl_open (x2 == null);
-ssl_open_post H_tree_x2s_a.
+try rename x into x2.
+try rename h_tree_xs_a into h_tree_x2s_a.
+try rename H_tree_xs_a into H_tree_x2s_a.
+ssl_open (x2 == null) H_tree_x2s_a.
 move=>[phi_tree_x2s_a0].
 move=>[sigma_tree_x2s_a].
 subst h_tree_x2s_a.
+shelve.
+ex_elim vx2 s1x2 s2x2 lx2 rx2.
+ex_elim h_tree_lx2s1x2_526x2 h_tree_rx2s2x2_527x2.
+move=>[phi_tree_x2s_a0].
+move=>[sigma_tree_x2s_a].
+subst h_tree_x2s_a.
+move=>[H_tree_lx2s1x2_526x2 H_tree_rx2s2x2_527x2].
+shelve.
+Unshelve.
+try rename h_tree_ys_a into h_tree_y_a.
+try rename H_tree_ys_a into H_tree_y_a.
+try rename h_tree_x2s_a into h_tree_x2_a.
+try rename H_tree_x2s_a into H_tree_x2_a.
+try rename h_tree_y_a into h_tree__a.
+try rename H_tree_y_a into H_tree__a.
 ssl_emp;
 exists (null);
 exists (empty);
 exists (empty);
-sslauto;
-solve [
+sslauto.
 unfold_constructor 1;
-sslauto |
+sslauto.
 unfold_constructor 1;
-sslauto ].
-ex_elim vx22 s1x2 s2x2 lx22 rx22.
-ex_elim h_tree_lx22s1x2_529x2 h_tree_rx22s2x2_530x2.
-move=>[phi_tree_x2s_a0].
-move=>[sigma_tree_x2s_a].
-subst h_tree_x2s_a.
-move=>[H_tree_lx22s1x2_529x2 H_tree_rx22s2x2_530x2].
+sslauto.
+try rename h_tree_x2s_a into h_tree_x2vx2s1x2s2x2_a.
+try rename H_tree_x2s_a into H_tree_x2vx2s1x2s2x2_a.
+try rename h_tree_ys_a into h_tree_yvx2s1x2s2x2_a.
+try rename H_tree_ys_a into H_tree_yvx2s1x2s2x2_a.
 ssl_read x2.
+try rename vx2 into vx22.
+try rename h_tree_yvx2s1x2s2x2_a into h_tree_yvx22s1x2s2x2_a.
+try rename H_tree_yvx2s1x2s2x2_a into H_tree_yvx22s1x2s2x2_a.
+try rename h_tree_x2vx2s1x2s2x2_a into h_tree_x2vx22s1x2s2x2_a.
+try rename H_tree_x2vx2s1x2s2x2_a into H_tree_x2vx22s1x2s2x2_a.
 ssl_read (x2 .+ 1).
+try rename lx2 into lx22.
+try rename h_tree_lx2s1x2_526x2 into h_tree_lx22s1x2_526x2.
+try rename H_tree_lx2s1x2_526x2 into H_tree_lx22s1x2_526x2.
 ssl_read (x2 .+ 2).
+try rename rx2 into rx22.
+try rename h_tree_rx2s2x2_527x2 into h_tree_rx22s2x2_527x2.
+try rename H_tree_rx2s2x2_527x2 into H_tree_rx22s2x2_527x2.
 ssl_write r.
-ssl_call_pre (r :-> lx22 \+ h_tree_lx22s1x2_529x2).
+ssl_call_pre (r :-> lx22 \+ h_tree_lx22s1x2_526x2).
 ssl_call (lx22, s1x2).
-exists (h_tree_lx22s1x2_529x2);
+exists (h_tree_lx22s1x2_526x2);
+sslauto.
+move=>h_call0.
+ex_elim y1.
+ex_elim h_tree_lx22s1x2_526x2 h_tree_y1s1x2_526x2.
+move=>[sigma_call0].
+subst h_call0.
+move=>[H_tree_lx22s1x2_526x2 H_tree_y1s1x2_526x2].
+store_valid.
+ssl_read r.
+try rename y1 into y12.
+try rename h_tree_y1s1x2_526x2 into h_tree_y12s1x2_526x2.
+try rename H_tree_y1s1x2_526x2 into H_tree_y12s1x2_526x2.
+ssl_write r.
+ssl_call_pre (r :-> rx22 \+ h_tree_rx22s2x2_527x2).
+ssl_call (rx22, s2x2).
+exists (h_tree_rx22s2x2_527x2);
 sslauto.
 move=>h_call1.
-ex_elim y12.
-ex_elim h_tree_lx22s1x2_529x2 h_tree_y12s1x2_529x2.
+ex_elim y2.
+ex_elim h_tree_rx22s2x2_527x2 h_tree_y2s2x2_527x2.
 move=>[sigma_call1].
 subst h_call1.
-move=>[H_tree_lx22s1x2_529x2 H_tree_y12s1x2_529x2].
+move=>[H_tree_rx22s2x2_527x2 H_tree_y2s2x2_527x2].
 store_valid.
 ssl_read r.
-ssl_write r.
-ssl_call_pre (r :-> rx22 \+ h_tree_rx22s2x2_530x2).
-ssl_call (rx22, s2x2).
-exists (h_tree_rx22s2x2_530x2);
-sslauto.
-move=>h_call2.
-ex_elim y22.
-ex_elim h_tree_rx22s2x2_530x2 h_tree_y22s2x2_530x2.
-move=>[sigma_call2].
-subst h_call2.
-move=>[H_tree_rx22s2x2_530x2 H_tree_y22s2x2_530x2].
-store_valid.
-ssl_read r.
+try rename y2 into y22.
+try rename h_tree_y2s2x2_527x2 into h_tree_y22s2x2_527x2.
+try rename H_tree_y2s2x2_527x2 into H_tree_y22s2x2_527x2.
+try rename h_tree_lx21s11x2_526x21 into h_tree_lx21s11x2_526x2.
+try rename H_tree_lx21s11x2_526x21 into H_tree_lx21s11x2_526x2.
+try rename h_tree_lx21s11x2_526x2 into h_tree_lx22s11x2_526x2.
+try rename H_tree_lx21s11x2_526x2 into H_tree_lx22s11x2_526x2.
+try rename h_tree_lx22s11x2_526x2 into h_tree_lx22s1x2_526x2.
+try rename H_tree_lx22s11x2_526x2 into H_tree_lx22s1x2_526x2.
+try rename h_tree_r3x2s21x2_527x21 into h_tree_r3x2s21x2_527x2.
+try rename H_tree_r3x2s21x2_527x21 into H_tree_r3x2s21x2_527x2.
+try rename h_tree_r3x2s21x2_527x2 into h_tree_rx22s21x2_527x2.
+try rename H_tree_r3x2s21x2_527x2 into H_tree_rx22s21x2_527x2.
+try rename h_tree_rx22s21x2_527x2 into h_tree_rx22s2x2_527x2.
+try rename H_tree_rx22s21x2_527x2 into H_tree_rx22s2x2_527x2.
+try rename h_tree_lys11y_526y into h_tree_lys11y_526x2.
+try rename H_tree_lys11y_526y into H_tree_lys11y_526x2.
+try rename h_tree_lys11y_526x2 into h_tree_y12s11y_526x2.
+try rename H_tree_lys11y_526x2 into H_tree_y12s11y_526x2.
+try rename h_tree_y12s11y_526x2 into h_tree_y12s1x2_526x2.
+try rename H_tree_y12s11y_526x2 into H_tree_y12s1x2_526x2.
+try rename h_tree_r3ys21y_527y into h_tree_r3ys21y_527x2.
+try rename H_tree_r3ys21y_527y into H_tree_r3ys21y_527x2.
+try rename h_tree_r3ys21y_527x2 into h_tree_y22s21y_527x2.
+try rename H_tree_r3ys21y_527x2 into H_tree_y22s21y_527x2.
+try rename h_tree_y22s21y_527x2 into h_tree_y22s2x2_527x2.
+try rename H_tree_y22s21y_527x2 into H_tree_y22s2x2_527x2.
 ssl_alloc y3.
+try rename y into y3.
+try rename h_tree_yvx22s1x2s2x2_a into h_tree_y3vx22s1x2s2x2_a.
+try rename H_tree_yvx22s1x2s2x2_a into H_tree_y3vx22s1x2s2x2_a.
 ssl_write r.
 ssl_write_post r.
 ssl_write (y3 .+ 1).
@@ -145,18 +213,13 @@ ssl_write y3.
 ssl_write_post y3.
 ssl_emp;
 exists (y3);
-exists (x2 :-> vx22 \+ x2 .+ 1 :-> lx22 \+ x2 .+ 2 :-> rx22 \+ h_tree_lx22s1x2_529x2 \+ h_tree_rx22s2x2_530x2);
-exists (y3 :-> vx22 \+ y3 .+ 1 :-> y12 \+ y3 .+ 2 :-> y22 \+ h_tree_y12s1x2_529x2 \+ h_tree_y22s2x2_530x2);
-sslauto;
-solve [
+exists (x2 :-> vx22 \+ x2 .+ 1 :-> lx22 \+ x2 .+ 2 :-> rx22 \+ h_tree_lx22s1x2_526x2 \+ h_tree_rx22s2x2_527x2);
+exists (y3 :-> vx22 \+ y3 .+ 1 :-> y12 \+ y3 .+ 2 :-> y22 \+ h_tree_y12s1x2_526x2 \+ h_tree_y22s2x2_527x2);
+sslauto.
 unfold_constructor 2;
-exists (vx22), (s1x2), (s2x2), (lx22), (rx22);
-exists (h_tree_lx22s1x2_529x2);
-exists (h_tree_rx22s2x2_530x2);
-sslauto |
+exists (vx22), (s1x2), (s2x2), (lx22), (rx22), (h_tree_lx22s1x2_526x2), (h_tree_rx22s2x2_527x2);
+sslauto.
 unfold_constructor 2;
-exists (vx22), (s1x2), (s2x2), (y12), (y22);
-exists (h_tree_y12s1x2_529x2);
-exists (h_tree_y22s2x2_530x2);
-sslauto ].
+exists (vx22), (s1x2), (s2x2), (y12), (y22), (h_tree_y12s1x2_526x2), (h_tree_y22s2x2_527x2);
+sslauto.
 Qed.
