examples/tree_free.v
@@ -12,19 +12,29 @@ Inductive tree (x : ptr) (s : seq nat) (h : heap) : Prop :=
   @perm_eq nat_eqType (s) (nil) /\ h = empty
 | tree_2 of (x == null) = false of
   exists (v : nat) (s1 : seq nat) (s2 : seq nat) (l : ptr) (r : ptr),
-  exists h_tree_ls1_533 h_tree_rs2_534,
-  @perm_eq nat_eqType (s) ([:: v] ++ s1 ++ s2) /\ h = x :-> v \+ x .+ 1 :-> l \+ x .+ 2 :-> r \+ h_tree_ls1_533 \+ h_tree_rs2_534 /\ tree l s1 h_tree_ls1_533 /\ tree r s2 h_tree_rs2_534.
+  exists h_tree_ls1_531 h_tree_rs2_532,
+  @perm_eq nat_eqType (s) ([:: v] ++ s1 ++ s2) /\ h = x :-> v \+ x .+ 1 :-> l \+ x .+ 2 :-> r \+ h_tree_ls1_531 \+ h_tree_rs2_532 /\ tree l s1 h_tree_ls1_531 /\ tree r s2 h_tree_rs2_532.
 
 Inductive treeN (x : ptr) (n : nat) (h : heap) : Prop :=
 | treeN_1 of x == null of
   n == 0 /\ h = empty
 | treeN_2 of (x == null) = false of
   exists (n1 : nat) (n2 : nat) (l : ptr) (r : ptr) (v : ptr),
-  exists h_treeN_ln1_535 h_treeN_rn2_536,
-  0 <= n1 /\ 0 <= n2 /\ n == 1 + n1 + n2 /\ h = x :-> v \+ x .+ 1 :-> l \+ x .+ 2 :-> r \+ h_treeN_ln1_535 \+ h_treeN_rn2_536 /\ treeN l n1 h_treeN_ln1_535 /\ treeN r n2 h_treeN_rn2_536.
+  exists h_treeN_ln1_533 h_treeN_rn2_534,
+  0 <= n1 /\ 0 <= n2 /\ n == 1 + n1 + n2 /\ h = x :-> v \+ x .+ 1 :-> l \+ x .+ 2 :-> r \+ h_treeN_ln1_533 \+ h_treeN_rn2_534 /\ treeN l n1 h_treeN_ln1_533 /\ treeN r n2 h_treeN_rn2_534.
 
-Lemma tree_perm_eq_trans23 x h s_1 s_2 : perm_eq s_1 s_2 -> tree x s_1 h -> tree x s_2 h. Admitted.
-Hint Resolve tree_perm_eq_trans23: ssl_pred.
+Inductive sll (x : ptr) (s : seq nat) (h : heap) : Prop :=
+| sll_1 of x == null of
+  @perm_eq nat_eqType (s) (nil) /\ h = empty
+| sll_2 of (x == null) = false of
+  exists (v : nat) (s1 : seq nat) (nxt : ptr),
+  exists h_sll_nxts1_535,
+  @perm_eq nat_eqType (s) ([:: v] ++ s1) /\ h = x :-> v \+ x .+ 1 :-> nxt \+ h_sll_nxts1_535 /\ sll nxt s1 h_sll_nxts1_535.
+
+Lemma tree_perm_eq_trans13 x h s_1 s_2 : perm_eq s_1 s_2 -> tree x s_1 h -> tree x s_2 h. Admitted.
+Hint Resolve tree_perm_eq_trans13: ssl_pred.
+Lemma sll_perm_eq_trans14 x h s_1 s_2 : perm_eq s_1 s_2 -> sll x s_1 h -> sll x s_2 h. Admitted.
+Hint Resolve sll_perm_eq_trans14: ssl_pred.
 
 Definition tree_free_type :=
   forall (vprogs : ptr),
@@ -33,8 +43,8 @@ Definition tree_free_type :=
     fun h =>
       let: (x) := vprogs in
       let: (s) := vghosts in
-      exists h_tree_xs_537,
-      h = h_tree_xs_537 /\ tree x s h_tree_xs_537,
+      exists h_tree_xs_536,
+      h = h_tree_xs_536 /\ tree x s h_tree_xs_536,
     [vfun (_: unit) h =>
       let: (x) := vprogs in
       let: (s) := vghosts in
@@ -49,6 +59,7 @@ Program Definition tree_free : tree_free_type :=
       then
         ret tt
       else
+        vx2 <-- @read nat x;
         lx2 <-- @read ptr (x .+ 1);
         rx2 <-- @read ptr (x .+ 2);
         tree_free (lx2);;
@@ -62,41 +73,57 @@ Obligation Tactic := intro; move=>x; ssl_program_simpl.
 Next Obligation.
 ssl_ghostelim_pre.
 move=>s.
-ex_elim h_tree_xs_537.
+ex_elim h_tree_xs_536.
 move=>[sigma_self].
 subst h_self.
-move=>H_tree_xs_537.
+move=>H_tree_xs_536.
 ssl_ghostelim_post.
-ssl_open (x == null);
-ssl_open_post H_tree_xs_537.
-move=>[phi_tree_xs_5370].
-move=>[sigma_tree_xs_537].
-subst h_tree_xs_537.
+ssl_open (x == null) H_tree_xs_536.
+move=>[phi_tree_xs_5360].
+move=>[sigma_tree_xs_536].
+subst h_tree_xs_536.
+shelve.
+ex_elim vx s1x s2x lx rx.
+ex_elim h_tree_lxs1x_531x h_tree_rxs2x_532x.
+move=>[phi_tree_xs_5360].
+move=>[sigma_tree_xs_536].
+subst h_tree_xs_536.
+move=>[H_tree_lxs1x_531x H_tree_rxs2x_532x].
+shelve.
+Unshelve.
+try rename h_tree_xs_536 into h_tree_x_536.
+try rename H_tree_xs_536 into H_tree_x_536.
 ssl_emp;
 sslauto.
-ex_elim vx2 s1x s2x lx2 rx2.
-ex_elim h_tree_lx2s1x_533x h_tree_rx2s2x_534x.
-move=>[phi_tree_xs_5370].
-move=>[sigma_tree_xs_537].
-subst h_tree_xs_537.
-move=>[H_tree_lx2s1x_533x H_tree_rx2s2x_534x].
+try rename h_tree_xs_536 into h_tree_xvxs1xs2x_536.
+try rename H_tree_xs_536 into H_tree_xvxs1xs2x_536.
+ssl_read x.
+try rename vx into vx2.
+try rename h_tree_xvxs1xs2x_536 into h_tree_xvx2s1xs2x_536.
+try rename H_tree_xvxs1xs2x_536 into H_tree_xvx2s1xs2x_536.
 ssl_read (x .+ 1).
+try rename lx into lx2.
+try rename h_tree_lxs1x_531x into h_tree_lx2s1x_531x.
+try rename H_tree_lxs1x_531x into H_tree_lx2s1x_531x.
 ssl_read (x .+ 2).
-ssl_call_pre (h_tree_lx2s1x_533x).
+try rename rx into rx2.
+try rename h_tree_rxs2x_532x into h_tree_rx2s2x_532x.
+try rename H_tree_rxs2x_532x into H_tree_rx2s2x_532x.
+ssl_call_pre (h_tree_lx2s1x_531x).
 ssl_call (s1x).
-exists (h_tree_lx2s1x_533x);
+exists (h_tree_lx2s1x_531x);
+sslauto.
+move=>h_call0.
+move=>[sigma_call0].
+subst h_call0.
+store_valid.
+ssl_call_pre (h_tree_rx2s2x_532x).
+ssl_call (s2x).
+exists (h_tree_rx2s2x_532x);
 sslauto.
 move=>h_call1.
 move=>[sigma_call1].
 subst h_call1.
-store_valid.
-ssl_call_pre (h_tree_rx2s2x_534x).
-ssl_call (s2x).
-exists (h_tree_rx2s2x_534x);
-sslauto.
-move=>h_call2.
-move=>[sigma_call2].
-subst h_call2.
 store_valid.
 ssl_dealloc x.
 ssl_dealloc (x .+ 1).
