examples/tree_size.v
@@ -12,23 +12,33 @@ Inductive tree (x : ptr) (s : seq nat) (h : heap) : Prop :=
   @perm_eq nat_eqType (s) (nil) /\ h = empty
 | tree_2 of (x == null) = false of
   exists (v : nat) (s1 : seq nat) (s2 : seq nat) (l : ptr) (r : ptr),
-  exists h_tree_ls1_525 h_tree_rs2_526,
-  @perm_eq nat_eqType (s) ([:: v] ++ s1 ++ s2) /\ h = x :-> v \+ x .+ 1 :-> l \+ x .+ 2 :-> r \+ h_tree_ls1_525 \+ h_tree_rs2_526 /\ tree l s1 h_tree_ls1_525 /\ tree r s2 h_tree_rs2_526.
+  exists h_tree_ls1_521 h_tree_rs2_522,
+  @perm_eq nat_eqType (s) ([:: v] ++ s1 ++ s2) /\ h = x :-> v \+ x .+ 1 :-> l \+ x .+ 2 :-> r \+ h_tree_ls1_521 \+ h_tree_rs2_522 /\ tree l s1 h_tree_ls1_521 /\ tree r s2 h_tree_rs2_522.
 
 Inductive treeN (x : ptr) (n : nat) (h : heap) : Prop :=
 | treeN_1 of x == null of
   n == 0 /\ h = empty
 | treeN_2 of (x == null) = false of
   exists (n1 : nat) (n2 : nat) (l : ptr) (r : ptr) (v : ptr),
-  exists h_treeN_ln1_527 h_treeN_rn2_528,
-  0 <= n1 /\ 0 <= n2 /\ n == 1 + n1 + n2 /\ h = x :-> v \+ x .+ 1 :-> l \+ x .+ 2 :-> r \+ h_treeN_ln1_527 \+ h_treeN_rn2_528 /\ treeN l n1 h_treeN_ln1_527 /\ treeN r n2 h_treeN_rn2_528.
+  exists h_treeN_ln1_523 h_treeN_rn2_524,
+  0 <= n1 /\ 0 <= n2 /\ n == 1 + n1 + n2 /\ h = x :-> v \+ x .+ 1 :-> l \+ x .+ 2 :-> r \+ h_treeN_ln1_523 \+ h_treeN_rn2_524 /\ treeN l n1 h_treeN_ln1_523 /\ treeN r n2 h_treeN_rn2_524.
 
-Lemma tree_perm_eq_trans16 x h s_1 s_2 : perm_eq s_1 s_2 -> tree x s_1 h -> tree x s_2 h. Admitted.
-Hint Resolve tree_perm_eq_trans16: ssl_pred.
-Lemma pure17 : 0 == 0. Admitted.
-Hint Resolve pure17: ssl_pure.
-Lemma pure18 n1x2 n2x2 : 0 <= 1 + n1x2 + n2x2 -> 0 <= n1x2 -> 0 <= n2x2 -> 1 + n1x2 + n2x2 == 1 + n1x2 + n2x2. Admitted.
-Hint Resolve pure18: ssl_pure.
+Inductive sll (x : ptr) (s : seq nat) (h : heap) : Prop :=
+| sll_1 of x == null of
+  @perm_eq nat_eqType (s) (nil) /\ h = empty
+| sll_2 of (x == null) = false of
+  exists (v : nat) (s1 : seq nat) (nxt : ptr),
+  exists h_sll_nxts1_525,
+  @perm_eq nat_eqType (s) ([:: v] ++ s1) /\ h = x :-> v \+ x .+ 1 :-> nxt \+ h_sll_nxts1_525 /\ sll nxt s1 h_sll_nxts1_525.
+
+Lemma tree_perm_eq_trans4 x h s_1 s_2 : perm_eq s_1 s_2 -> tree x s_1 h -> tree x s_2 h. Admitted.
+Hint Resolve tree_perm_eq_trans4: ssl_pred.
+Lemma sll_perm_eq_trans5 x h s_1 s_2 : perm_eq s_1 s_2 -> sll x s_1 h -> sll x s_2 h. Admitted.
+Hint Resolve sll_perm_eq_trans5: ssl_pred.
+Lemma pure6 : 0 == 0. Admitted.
+Hint Resolve pure6: ssl_pure.
+Lemma pure7 n1x2 n2x2 : 0 <= 1 + n1x2 + n2x2 -> 0 <= n1x2 -> 0 <= n2x2 -> 1 + n1x2 + n2x2 == 1 + n1x2 + n2x2. Admitted.
+Hint Resolve pure7: ssl_pure.
 
 Definition tree_size_type :=
   forall (vprogs : ptr * ptr),
@@ -54,6 +64,7 @@ Program Definition tree_size : tree_size_type :=
       then
         ret tt
       else
+        vx2 <-- @read ptr x;
         lx2 <-- @read ptr (x .+ 1);
         rx2 <-- @read ptr (x .+ 2);
         tree_size (lx2, r);;
@@ -74,57 +85,89 @@ move=>[sigma_self].
 subst h_self.
 move=>H_treeN_xn_a.
 ssl_ghostelim_post.
-ssl_open (x == null);
-ssl_open_post H_treeN_xn_a.
+ssl_open (x == null) H_treeN_xn_a.
 move=>[phi_treeN_xn_a0].
 move=>[sigma_treeN_xn_a].
 subst h_treeN_xn_a.
-ssl_emp;
-exists (empty);
-sslauto;
-solve [
-unfold_constructor 1;
-sslauto ].
-ex_elim n1x2 n2x2 lx2 rx2 vx2.
-ex_elim h_treeN_lx2n1x2_527x h_treeN_rx2n2x2_528x.
+shelve.
+ex_elim n1x n2x lx rx vx.
+ex_elim h_treeN_lxn1x_523x h_treeN_rxn2x_524x.
 move=>[phi_treeN_xn_a0] [phi_treeN_xn_a1] [phi_treeN_xn_a2].
 move=>[sigma_treeN_xn_a].
 subst h_treeN_xn_a.
-move=>[H_treeN_lx2n1x2_527x H_treeN_rx2n2x2_528x].
+move=>[H_treeN_lxn1x_523x H_treeN_rxn2x_524x].
+shelve.
+Unshelve.
+try rename h_treeN_xn_a into h_treeN_x_a.
+try rename H_treeN_xn_a into H_treeN_x_a.
+ssl_emp;
+exists (empty);
+sslauto.
+unfold_constructor 1;
+sslauto.
+try rename h_treeN_xn_a into h_treeN_xn1xn2x_a.
+try rename H_treeN_xn_a into H_treeN_xn1xn2x_a.
+ssl_read x.
+try rename vx into vx2.
 ssl_read (x .+ 1).
+try rename lx into lx2.
+try rename h_treeN_lxn1x_523x into h_treeN_lx2n1x_523x.
+try rename H_treeN_lxn1x_523x into H_treeN_lx2n1x_523x.
 ssl_read (x .+ 2).
-ssl_call_pre (r :-> 0 \+ h_treeN_lx2n1x2_527x).
-ssl_call (n1x2).
-exists (h_treeN_lx2n1x2_527x);
+try rename rx into rx2.
+try rename h_treeN_rxn2x_524x into h_treeN_rx2n2x_524x.
+try rename H_treeN_rxn2x_524x into H_treeN_rx2n2x_524x.
+ssl_call_pre (r :-> 0 \+ h_treeN_lx2n1x_523x).
+ssl_call (n1x).
+exists (h_treeN_lx2n1x_523x);
+sslauto.
+move=>h_call0.
+ex_elim h_treeN_lx2n1x_523x.
+move=>[sigma_call0].
+subst h_call0.
+move=>H_treeN_lx2n1x_523x.
+store_valid.
+ssl_read r.
+try rename n1x into n1x2.
+try rename h_treeN_lx2n1x_523x into h_treeN_lx2n1x2_523x.
+try rename H_treeN_lx2n1x_523x into H_treeN_lx2n1x2_523x.
+try rename h_treeN_xn1xn2x_a into h_treeN_xn1x2n2x_a.
+try rename H_treeN_xn1xn2x_a into H_treeN_xn1x2n2x_a.
+ssl_write r.
+ssl_call_pre (r :-> 0 \+ h_treeN_rx2n2x_524x).
+ssl_call (n2x).
+exists (h_treeN_rx2n2x_524x);
 sslauto.
 move=>h_call1.
-ex_elim h_treeN_lx2n1x2_527x.
+ex_elim h_treeN_rx2n2x_524x.
 move=>[sigma_call1].
 subst h_call1.
-move=>H_treeN_lx2n1x2_527x.
+move=>H_treeN_rx2n2x_524x.
 store_valid.
 ssl_read r.
-ssl_write r.
-ssl_call_pre (r :-> 0 \+ h_treeN_rx2n2x2_528x).
-ssl_call (n2x2).
-exists (h_treeN_rx2n2x2_528x);
-sslauto.
-move=>h_call2.
-ex_elim h_treeN_rx2n2x2_528x.
-move=>[sigma_call2].
-subst h_call2.
-move=>H_treeN_rx2n2x2_528x.
-store_valid.
-ssl_read r.
+try rename n2x into n2x2.
+try rename h_treeN_rx2n2x_524x into h_treeN_rx2n2x2_524x.
+try rename H_treeN_rx2n2x_524x into H_treeN_rx2n2x2_524x.
+try rename h_treeN_xn1x2n2x_a into h_treeN_xn1x2n2x2_a.
+try rename H_treeN_xn1x2n2x_a into H_treeN_xn1x2n2x2_a.
+try rename h_treeN_lx1n11x_523x1 into h_treeN_lx1n11x_523x.
+try rename H_treeN_lx1n11x_523x1 into H_treeN_lx1n11x_523x.
+try rename h_treeN_lx1n11x_523x into h_treeN_lx2n11x_523x.
+try rename H_treeN_lx1n11x_523x into H_treeN_lx2n11x_523x.
+try rename h_treeN_lx2n11x_523x into h_treeN_lx2n1x2_523x.
+try rename H_treeN_lx2n11x_523x into H_treeN_lx2n1x2_523x.
+try rename h_treeN_r3xn21x_524x1 into h_treeN_r3xn21x_524x.
+try rename H_treeN_r3xn21x_524x1 into H_treeN_r3xn21x_524x.
+try rename h_treeN_r3xn21x_524x into h_treeN_r3xn2x2_524x.
+try rename H_treeN_r3xn21x_524x into H_treeN_r3xn2x2_524x.
+try rename h_treeN_r3xn2x2_524x into h_treeN_rx2n2x2_524x.
+try rename H_treeN_r3xn2x2_524x into H_treeN_rx2n2x2_524x.
 ssl_write r.
 ssl_write_post r.
 ssl_emp;
-exists (x :-> vx2 \+ x .+ 1 :-> lx2 \+ x .+ 2 :-> rx2 \+ h_treeN_lx2n1x2_527x \+ h_treeN_rx2n2x2_528x);
-sslauto;
-solve [
+exists (x :-> vx2 \+ x .+ 1 :-> lx2 \+ x .+ 2 :-> rx2 \+ h_treeN_lx2n1x2_523x \+ h_treeN_rx2n2x2_524x);
+sslauto.
 unfold_constructor 2;
-exists (n1x2), (n2x2), (lx2), (rx2), (vx2);
-exists (h_treeN_lx2n1x2_527x);
-exists (h_treeN_rx2n2x2_528x);
-sslauto ].
+exists (n1x2), (n2x2), (lx2), (rx2), (vx2), (h_treeN_lx2n1x2_523x), (h_treeN_rx2n2x2_524x);
+sslauto.
 Qed.
