examples/bst_find_smallest.v
@@ -12,23 +12,23 @@ Inductive bst (x : ptr) (sz : nat) (lo : nat) (hi : nat) (h : heap) : Prop :=
   hi == 0 /\ lo == 7 /\ sz == 0 /\ h = empty
 | bst_2 of (x == null) = false of
   exists (sz1 : nat) (sz2 : nat) (v : nat) (hi2 : nat) (hi1 : nat) (lo1 : nat) (lo2 : nat) (l : ptr) (r : ptr),
-  exists h_bst_lsz1lo1hi1_570 h_bst_rsz2lo2hi2_571,
-  0 <= sz1 /\ 0 <= sz2 /\ 0 <= v /\ hi == (if hi2 <= v then v else hi2) /\ hi1 <= v /\ lo == (if v <= lo1 then v else lo1) /\ sz == 1 + sz1 + sz2 /\ v <= 7 /\ v <= lo2 /\ h = x :-> v \+ x .+ 1 :-> l \+ x .+ 2 :-> r \+ h_bst_lsz1lo1hi1_570 \+ h_bst_rsz2lo2hi2_571 /\ bst l sz1 lo1 hi1 h_bst_lsz1lo1hi1_570 /\ bst r sz2 lo2 hi2 h_bst_rsz2lo2hi2_571.
+  exists h_bst_lsz1lo1hi1_521 h_bst_rsz2lo2hi2_522,
+  0 <= sz1 /\ 0 <= sz2 /\ 0 <= v /\ hi == (if hi2 <= v then v else hi2) /\ hi1 <= v /\ lo == (if v <= lo1 then v else lo1) /\ sz == 1 + sz1 + sz2 /\ v <= 7 /\ v <= lo2 /\ h = x :-> v \+ x .+ 1 :-> l \+ x .+ 2 :-> r \+ h_bst_lsz1lo1hi1_521 \+ h_bst_rsz2lo2hi2_522 /\ bst l sz1 lo1 hi1 h_bst_lsz1lo1hi1_521 /\ bst r sz2 lo2 hi2 h_bst_rsz2lo2hi2_522.
 
-Lemma pure75 : 0 == 0. Admitted.
-Hint Resolve pure75: ssl_pure.
-Lemma pure76 : 7 == 7. Admitted.
-Hint Resolve pure76: ssl_pure.
-Lemma pure77 hi2x lo2x hi1x vx2 lo1x : hi1x <= vx2 -> vx2 <= lo2x -> (if hi2x <= vx2 then vx2 else hi2x) <= 7 -> 0 <= vx2 -> vx2 <= 7 -> 0 <= (if vx2 <= lo1x then vx2 else lo1x) -> 0 <= lo1x. Admitted.
-Hint Resolve pure77: ssl_pure.
-Lemma pure78 hi2x lo2x hi1x vx2 lo1x : hi1x <= vx2 -> vx2 <= lo2x -> (if hi2x <= vx2 then vx2 else hi2x) <= 7 -> 0 <= vx2 -> vx2 <= 7 -> 0 <= (if vx2 <= lo1x then vx2 else lo1x) -> hi1x <= 7. Admitted.
-Hint Resolve pure78: ssl_pure.
-Lemma pure79 sz1x sz2x : 0 <= sz2x -> 0 <= sz1x -> 0 <= 1 + sz1x + sz2x -> 1 + sz1x + sz2x == 1 + sz1x + sz2x. Admitted.
-Hint Resolve pure79: ssl_pure.
-Lemma pure80 hi2x lo2x hi1x vx2 lo1x2 : 0 <= (if vx2 <= lo1x2 then vx2 else lo1x2) -> hi1x <= vx2 -> vx2 <= lo2x -> (if hi2x <= vx2 then vx2 else hi2x) <= 7 -> 0 <= vx2 -> vx2 <= 7 -> (if hi2x <= vx2 then vx2 else hi2x) == (if hi2x <= vx2 then vx2 else hi2x). Admitted.
-Hint Resolve pure80: ssl_pure.
-Lemma pure81 hi2x lo2x hi1x vx2 lo1x2 : 0 <= (if vx2 <= lo1x2 then vx2 else lo1x2) -> hi1x <= vx2 -> vx2 <= lo2x -> (if hi2x <= vx2 then vx2 else hi2x) <= 7 -> 0 <= vx2 -> vx2 <= 7 -> (if vx2 <= lo1x2 then vx2 else lo1x2) == (if vx2 <= lo1x2 then vx2 else lo1x2). Admitted.
-Hint Resolve pure81: ssl_pure.
+Lemma pure26 : 0 == 0. Admitted.
+Hint Resolve pure26: ssl_pure.
+Lemma pure27 : 7 == 7. Admitted.
+Hint Resolve pure27: ssl_pure.
+Lemma pure28 hi2x lo2x hi1x vx2 lo1x : hi1x <= vx2 -> vx2 <= lo2x -> (if hi2x <= vx2 then vx2 else hi2x) <= 7 -> 0 <= vx2 -> vx2 <= 7 -> 0 <= (if vx2 <= lo1x then vx2 else lo1x) -> 0 <= lo1x. Admitted.
+Hint Resolve pure28: ssl_pure.
+Lemma pure29 hi2x lo2x hi1x vx2 lo1x : hi1x <= vx2 -> vx2 <= lo2x -> (if hi2x <= vx2 then vx2 else hi2x) <= 7 -> 0 <= vx2 -> vx2 <= 7 -> 0 <= (if vx2 <= lo1x then vx2 else lo1x) -> hi1x <= 7. Admitted.
+Hint Resolve pure29: ssl_pure.
+Lemma pure30 sz1x sz2x : 0 <= 1 + sz1x + sz2x -> 0 <= sz1x -> 0 <= sz2x -> 1 + sz1x + sz2x == 1 + sz1x + sz2x. Admitted.
+Hint Resolve pure30: ssl_pure.
+Lemma pure31 hi2x lo2x hi1x vx2 lo1x2 : 0 <= (if vx2 <= lo1x2 then vx2 else lo1x2) -> hi1x <= vx2 -> vx2 <= lo2x -> (if hi2x <= vx2 then vx2 else hi2x) <= 7 -> 0 <= vx2 -> vx2 <= 7 -> (if hi2x <= vx2 then vx2 else hi2x) == (if hi2x <= vx2 then vx2 else hi2x). Admitted.
+Hint Resolve pure31: ssl_pure.
+Lemma pure32 hi2x lo2x hi1x vx2 lo1x2 : 0 <= (if vx2 <= lo1x2 then vx2 else lo1x2) -> hi1x <= vx2 -> vx2 <= lo2x -> (if hi2x <= vx2 then vx2 else hi2x) <= 7 -> 0 <= vx2 -> vx2 <= 7 -> (if vx2 <= lo1x2 then vx2 else lo1x2) == (if vx2 <= lo1x2 then vx2 else lo1x2). Admitted.
+Hint Resolve pure32: ssl_pure.
 
 Definition bst_find_smallest_type :=
   forall (vprogs : ptr * ptr),
@@ -50,6 +50,7 @@ Program Definition bst_find_smallest : bst_find_smallest_type :=
   Fix (fun (bst_find_smallest : bst_find_smallest_type) vprogs =>
     let: (x, retv) := vprogs in
     Do (
+      unused2 <-- @read ptr retv;
       if x == null
       then
         retv ::= 7;;
@@ -57,6 +58,7 @@ Program Definition bst_find_smallest : bst_find_smallest_type :=
       else
         vx2 <-- @read nat x;
         lx2 <-- @read ptr (x .+ 1);
+        rx2 <-- @read ptr (x .+ 2);
         bst_find_smallest (lx2, retv);;
         lo1x2 <-- @read nat retv;
         retv ::= (if vx2 <= lo1x2 then vx2 else lo1x2);;
@@ -65,55 +67,120 @@ Program Definition bst_find_smallest : bst_find_smallest_type :=
 Obligation Tactic := intro; move=>[x retv]; ssl_program_simpl.
 Next Obligation.
 ssl_ghostelim_pre.
-move=>[[[lo sz] hi] unused2].
+move=>[[[lo sz] hi] unused].
 ex_elim h_bst_xszlohi_a.
 move=>[phi_self0] [phi_self1] [phi_self2].
 move=>[sigma_self].
 subst h_self.
 move=>H_bst_xszlohi_a.
 ssl_ghostelim_post.
-ssl_open (x == null);
-ssl_open_post H_bst_xszlohi_a.
+ssl_read retv.
+try rename unused into unused2.
+ssl_open (x == null) H_bst_xszlohi_a.
 move=>[phi_bst_xszlohi_a0] [phi_bst_xszlohi_a1] [phi_bst_xszlohi_a2].
 move=>[sigma_bst_xszlohi_a].
 subst h_bst_xszlohi_a.
+shelve.
+ex_elim sz1x sz2x vx hi2x hi1x.
+ex_elim lo1x lo2x lx rx.
+ex_elim h_bst_lxsz1xlo1xhi1x_521x h_bst_rxsz2xlo2xhi2x_522x.
+move=>[phi_bst_xszlohi_a0] [phi_bst_xszlohi_a1] [phi_bst_xszlohi_a2] [phi_bst_xszlohi_a3] [phi_bst_xszlohi_a4] [phi_bst_xszlohi_a5] [phi_bst_xszlohi_a6] [phi_bst_xszlohi_a7] [phi_bst_xszlohi_a8].
+move=>[sigma_bst_xszlohi_a].
+subst h_bst_xszlohi_a.
+move=>[H_bst_lxsz1xlo1xhi1x_521x H_bst_rxsz2xlo2xhi2x_522x].
+shelve.
+Unshelve.
+try rename h_bst_xszlohi_a into h_bst_xszlo_a.
+try rename H_bst_xszlohi_a into H_bst_xszlo_a.
+try rename h_bst_xszlohi_c into h_bst_xszlo_c.
+try rename H_bst_xszlohi_c into H_bst_xszlo_c.
+try rename h_bst_xszlo_a into h_bst_xsz_a.
+try rename H_bst_xszlo_a into H_bst_xsz_a.
+try rename h_bst_xszlo_c into h_bst_xsz_c.
+try rename H_bst_xszlo_c into H_bst_xsz_c.
+try rename h_bst_xsz_a into h_bst_x_a.
+try rename H_bst_xsz_a into H_bst_x_a.
+try rename h_bst_xsz_c into h_bst_x_c.
+try rename H_bst_xsz_c into H_bst_x_c.
 ssl_write retv.
 ssl_write_post retv.
 ssl_emp;
 exists (empty);
-sslauto;
-solve [
-unfold_constructor 1;
-sslauto ].
-ex_elim sz1x sz2x vx2 hi2x hi1x.
-ex_elim lo1x2 lo2x lx2 rx2.
-ex_elim h_bst_lx2sz1xlo1x2hi1x_570x h_bst_rx2sz2xlo2xhi2x_571x.
-move=>[phi_bst_xszlohi_a0] [phi_bst_xszlohi_a1] [phi_bst_xszlohi_a2] [phi_bst_xszlohi_a3] [phi_bst_xszlohi_a4] [phi_bst_xszlohi_a5] [phi_bst_xszlohi_a6] [phi_bst_xszlohi_a7] [phi_bst_xszlohi_a8].
-move=>[sigma_bst_xszlohi_a].
-subst h_bst_xszlohi_a.
-move=>[H_bst_lx2sz1xlo1x2hi1x_570x H_bst_rx2sz2xlo2xhi2x_571x].
-ssl_read x.
-ssl_read (x .+ 1).
-ssl_call_pre (retv :-> unused2 \+ h_bst_lx2sz1xlo1x2hi1x_570x).
-ssl_call (lo1x2, sz1x, hi1x, unused2).
-exists (h_bst_lx2sz1xlo1x2hi1x_570x);
 sslauto.
-move=>h_call1.
-ex_elim h_bst_lx2sz1xlo1x2hi1x_c1.
-move=>[sigma_call1].
-subst h_call1.
-move=>H_bst_lx2sz1xlo1x2hi1x_c1.
+unfold_constructor 1;
+sslauto.
+try rename h_bst_xszlohi_a into h_bst_xszlohi2xvxvxhi2x_a.
+try rename H_bst_xszlohi_a into H_bst_xszlohi2xvxvxhi2x_a.
+try rename h_bst_xszlohi_c into h_bst_xszlohi2xvxvxhi2x_c.
+try rename H_bst_xszlohi_c into H_bst_xszlohi2xvxvxhi2x_c.
+try rename h_bst_xszlohi2xvxvxhi2x_a into h_bst_xszvxlo1xvxlo1xhi2xvxvxhi2x_a.
+try rename H_bst_xszlohi2xvxvxhi2x_a into H_bst_xszvxlo1xvxlo1xhi2xvxvxhi2x_a.
+try rename h_bst_xszlohi2xvxvxhi2x_c into h_bst_xszvxlo1xvxlo1xhi2xvxvxhi2x_c.
+try rename H_bst_xszlohi2xvxvxhi2x_c into H_bst_xszvxlo1xvxlo1xhi2xvxvxhi2x_c.
+try rename h_bst_xszvxlo1xvxlo1xhi2xvxvxhi2x_a into h_bst_xsz1xsz2xvxlo1xvxlo1xhi2xvxvxhi2x_a.
+try rename H_bst_xszvxlo1xvxlo1xhi2xvxvxhi2x_a into H_bst_xsz1xsz2xvxlo1xvxlo1xhi2xvxvxhi2x_a.
+try rename h_bst_xszvxlo1xvxlo1xhi2xvxvxhi2x_c into h_bst_xsz1xsz2xvxlo1xvxlo1xhi2xvxvxhi2x_c.
+try rename H_bst_xszvxlo1xvxlo1xhi2xvxvxhi2x_c into H_bst_xsz1xsz2xvxlo1xvxlo1xhi2xvxvxhi2x_c.
+ssl_read x.
+try rename vx into vx2.
+try rename h_bst_xsz1xsz2xvxlo1xvxlo1xhi2xvxvxhi2x_a into h_bst_xsz1xsz2xvx2lo1xvx2lo1xhi2xvx2vx2hi2x_a.
+try rename H_bst_xsz1xsz2xvxlo1xvxlo1xhi2xvxvxhi2x_a into H_bst_xsz1xsz2xvx2lo1xvx2lo1xhi2xvx2vx2hi2x_a.
+try rename h_bst_xsz1xsz2xvxlo1xvxlo1xhi2xvxvxhi2x_c into h_bst_xsz1xsz2xvx2lo1xvx2lo1xhi2xvx2vx2hi2x_c.
+try rename H_bst_xsz1xsz2xvxlo1xvxlo1xhi2xvxvxhi2x_c into H_bst_xsz1xsz2xvx2lo1xvx2lo1xhi2xvx2vx2hi2x_c.
+ssl_read (x .+ 1).
+try rename lx into lx2.
+try rename h_bst_lxsz1xlo1xhi1x_521x into h_bst_lx2sz1xlo1xhi1x_521x.
+try rename H_bst_lxsz1xlo1xhi1x_521x into H_bst_lx2sz1xlo1xhi1x_521x.
+ssl_read (x .+ 2).
+try rename rx into rx2.
+try rename h_bst_rxsz2xlo2xhi2x_522x into h_bst_rx2sz2xlo2xhi2x_522x.
+try rename H_bst_rxsz2xlo2xhi2x_522x into H_bst_rx2sz2xlo2xhi2x_522x.
+ssl_call_pre (retv :-> unused2 \+ h_bst_lx2sz1xlo1xhi1x_521x).
+ssl_call (lo1x, sz1x, hi1x, unused2).
+exists (h_bst_lx2sz1xlo1xhi1x_521x);
+sslauto.
+move=>h_call0.
+ex_elim h_bst_lx2sz1xlo1xhi1x_c1.
+move=>[sigma_call0].
+subst h_call0.
+move=>H_bst_lx2sz1xlo1xhi1x_c1.
 store_valid.
 ssl_read retv.
+try rename lo1x into lo1x2.
+try rename h_bst_lx2sz1xlo1xhi1x_c1 into h_bst_lx2sz1xlo1x2hi1x_c1.
+try rename H_bst_lx2sz1xlo1xhi1x_c1 into H_bst_lx2sz1xlo1x2hi1x_c1.
+try rename h_bst_xsz1xsz2xvx2lo1xvx2lo1xhi2xvx2vx2hi2x_c into h_bst_xsz1xsz2xvx2lo1x2vx2lo1x2hi2xvx2vx2hi2x_c.
+try rename H_bst_xsz1xsz2xvx2lo1xvx2lo1xhi2xvx2vx2hi2x_c into H_bst_xsz1xsz2xvx2lo1x2vx2lo1x2hi2xvx2vx2hi2x_c.
+try rename h_bst_lx2sz1xlo1xhi1x_521x into h_bst_lx2sz1xlo1x2hi1x_521x.
+try rename H_bst_lx2sz1xlo1xhi1x_521x into H_bst_lx2sz1xlo1x2hi1x_521x.
+try rename h_bst_xsz1xsz2xvx2lo1xvx2lo1xhi2xvx2vx2hi2x_a into h_bst_xsz1xsz2xvx2lo1x2vx2lo1x2hi2xvx2vx2hi2x_a.
+try rename H_bst_xsz1xsz2xvx2lo1xvx2lo1xhi2xvx2vx2hi2x_a into H_bst_xsz1xsz2xvx2lo1x2vx2lo1x2hi2xvx2vx2hi2x_a.
+try rename h_bst_lx1sz11xlo11xhi11x_521x1 into h_bst_lx1sz11xlo11xhi11x_c1.
+try rename H_bst_lx1sz11xlo11xhi11x_521x1 into H_bst_lx1sz11xlo11xhi11x_c1.
+try rename h_bst_lx1sz11xlo11xhi11x_c1 into h_bst_lx1sz11xlo11xhi1x_c1.
+try rename H_bst_lx1sz11xlo11xhi11x_c1 into H_bst_lx1sz11xlo11xhi1x_c1.
+try rename h_bst_lx1sz11xlo11xhi1x_c1 into h_bst_lx1sz11xlo1x2hi1x_c1.
+try rename H_bst_lx1sz11xlo11xhi1x_c1 into H_bst_lx1sz11xlo1x2hi1x_c1.
+try rename h_bst_lx1sz11xlo1x2hi1x_c1 into h_bst_lx2sz11xlo1x2hi1x_c1.
+try rename H_bst_lx1sz11xlo1x2hi1x_c1 into H_bst_lx2sz11xlo1x2hi1x_c1.
+try rename h_bst_lx2sz11xlo1x2hi1x_c1 into h_bst_lx2sz1xlo1x2hi1x_c1.
+try rename H_bst_lx2sz11xlo1x2hi1x_c1 into H_bst_lx2sz1xlo1x2hi1x_c1.
+try rename h_bst_rx1sz2x1lo2x1hi2x1_522x1 into h_bst_rx1sz2x1lo2x1hi2x1_522x.
+try rename H_bst_rx1sz2x1lo2x1hi2x1_522x1 into H_bst_rx1sz2x1lo2x1hi2x1_522x.
+try rename h_bst_rx1sz2x1lo2x1hi2x1_522x into h_bst_rx1sz2x1lo2x1hi2x_522x.
+try rename H_bst_rx1sz2x1lo2x1hi2x1_522x into H_bst_rx1sz2x1lo2x1hi2x_522x.
+try rename h_bst_rx1sz2x1lo2x1hi2x_522x into h_bst_rx1sz2x1lo2xhi2x_522x.
+try rename H_bst_rx1sz2x1lo2x1hi2x_522x into H_bst_rx1sz2x1lo2xhi2x_522x.
+try rename h_bst_rx1sz2x1lo2xhi2x_522x into h_bst_rx2sz2x1lo2xhi2x_522x.
+try rename H_bst_rx1sz2x1lo2xhi2x_522x into H_bst_rx2sz2x1lo2xhi2x_522x.
+try rename h_bst_rx2sz2x1lo2xhi2x_522x into h_bst_rx2sz2xlo2xhi2x_522x.
+try rename H_bst_rx2sz2x1lo2xhi2x_522x into H_bst_rx2sz2xlo2xhi2x_522x.
 ssl_write retv.
 ssl_write_post retv.
 ssl_emp;
-exists (x :-> vx2 \+ x .+ 1 :-> lx2 \+ x .+ 2 :-> rx2 \+ h_bst_lx2sz1xlo1x2hi1x_c1 \+ h_bst_rx2sz2xlo2xhi2x_571x);
-sslauto;
-solve [
+exists (x :-> vx2 \+ x .+ 1 :-> lx2 \+ x .+ 2 :-> rx2 \+ h_bst_lx2sz1xlo1x2hi1x_c1 \+ h_bst_rx2sz2xlo2xhi2x_522x);
+sslauto.
 unfold_constructor 2;
-exists (sz1x), (sz2x), (vx2), (hi2x), (hi1x), (lo1x2), (lo2x), (lx2), (rx2);
-exists (h_bst_lx2sz1xlo1x2hi1x_c1);
-exists (h_bst_rx2sz2xlo2xhi2x_571x);
-sslauto ].
+exists (sz1x), (sz2x), (vx2), (hi2x), (hi1x), (lo1x2), (lo2x), (lx2), (rx2), (h_bst_lx2sz1xlo1x2hi1x_c1), (h_bst_rx2sz2xlo2xhi2x_522x);
+sslauto.
 Qed.
