examples/bst_left_rotate.v
@@ -12,17 +12,17 @@ Inductive bst (x : ptr) (sz : nat) (lo : nat) (hi : nat) (h : heap) : Prop :=
   hi == 0 /\ lo == 7 /\ sz == 0 /\ h = empty
 | bst_2 of (x == null) = false of
   exists (sz1 : nat) (sz2 : nat) (v : nat) (hi2 : nat) (hi1 : nat) (lo1 : nat) (lo2 : nat) (l : ptr) (r : ptr),
-  exists h_bst_lsz1lo1hi1_562 h_bst_rsz2lo2hi2_563,
-  0 <= sz1 /\ 0 <= sz2 /\ 0 <= v /\ hi == (if hi2 <= v then v else hi2) /\ hi1 <= v /\ lo == (if v <= lo1 then v else lo1) /\ sz == 1 + sz1 + sz2 /\ v <= 7 /\ v <= lo2 /\ h = x :-> v \+ x .+ 1 :-> l \+ x .+ 2 :-> r \+ h_bst_lsz1lo1hi1_562 \+ h_bst_rsz2lo2hi2_563 /\ bst l sz1 lo1 hi1 h_bst_lsz1lo1hi1_562 /\ bst r sz2 lo2 hi2 h_bst_rsz2lo2hi2_563.
+  exists h_bst_lsz1lo1hi1_513 h_bst_rsz2lo2hi2_514,
+  0 <= sz1 /\ 0 <= sz2 /\ 0 <= v /\ hi == (if hi2 <= v then v else hi2) /\ hi1 <= v /\ lo == (if v <= lo1 then v else lo1) /\ sz == 1 + sz1 + sz2 /\ v <= 7 /\ v <= lo2 /\ h = x :-> v \+ x .+ 1 :-> l \+ x .+ 2 :-> r \+ h_bst_lsz1lo1hi1_513 \+ h_bst_rsz2lo2hi2_514 /\ bst l sz1 lo1 hi1 h_bst_lsz1lo1hi1_513 /\ bst r sz2 lo2 hi2 h_bst_rsz2lo2hi2_514.
 
-Lemma pure50 sz1 sz1r2 sz2r2 : 0 <= sz1 -> 0 <= 1 + sz1r2 + sz2r2 -> 0 <= sz2r2 -> 0 <= sz1r2 -> 0 <= 1 + sz1 + sz1r2. Admitted.
-Hint Resolve pure50: ssl_pure.
-Lemma pure51 sz1 sz1r2 sz2r2 : 0 <= sz1 -> 0 <= 1 + sz1r2 + sz2r2 -> 0 <= sz2r2 -> 0 <= sz1r2 -> 1 + sz1 + sz1r2 + sz2r2 == sz1 + 1 + sz1r2 + sz2r2. Admitted.
-Hint Resolve pure51: ssl_pure.
-Lemma pure52 lo1r2 vr22 hi1 v2 hi1r2 lo2r2 : vr22 <= 7 -> v2 <= (if vr22 <= lo1r2 then vr22 else lo1r2) -> 0 <= v2 -> vr22 <= lo2r2 -> 0 <= vr22 -> hi1r2 <= vr22 -> hi1 <= v2 -> v2 <= 7 -> v2 <= lo1r2. Admitted.
-Hint Resolve pure52: ssl_pure.
-Lemma pure53 lo1r2 vr22 hi1 v2 hi1r2 lo2r2 : vr22 <= 7 -> v2 <= (if vr22 <= lo1r2 then vr22 else lo1r2) -> 0 <= v2 -> vr22 <= lo2r2 -> 0 <= vr22 -> hi1r2 <= vr22 -> hi1 <= v2 -> v2 <= 7 -> (if hi1r2 <= v2 then v2 else hi1r2) <= vr22. Admitted.
-Hint Resolve pure53: ssl_pure.
+Lemma pure1 sz1 sz1r2 sz2r2 : 0 <= sz1 -> 0 <= 1 + sz1r2 + sz2r2 -> 0 <= sz2r2 -> 0 <= sz1r2 -> 1 + sz1 + sz1r2 + sz2r2 == sz1 + 1 + sz1r2 + sz2r2. Admitted.
+Hint Resolve pure1: ssl_pure.
+Lemma pure2 sz1 sz1r2 sz2r2 : 0 <= sz1 -> 0 <= 1 + sz1r2 + sz2r2 -> 0 <= sz2r2 -> 0 <= sz1r2 -> 0 <= 1 + sz1 + sz1r2. Admitted.
+Hint Resolve pure2: ssl_pure.
+Lemma pure3 lo1r2 vr22 hi1 v2 hi1r2 lo2r2 : vr22 <= 7 -> v2 <= (if vr22 <= lo1r2 then vr22 else lo1r2) -> 0 <= v2 -> vr22 <= lo2r2 -> 0 <= vr22 -> hi1r2 <= vr22 -> hi1 <= v2 -> v2 <= 7 -> v2 <= lo1r2. Admitted.
+Hint Resolve pure3: ssl_pure.
+Lemma pure4 lo1r2 vr22 hi1 v2 hi1r2 lo2r2 : vr22 <= 7 -> v2 <= (if vr22 <= lo1r2 then vr22 else lo1r2) -> 0 <= v2 -> vr22 <= lo2r2 -> 0 <= vr22 -> hi1r2 <= vr22 -> hi1 <= v2 -> v2 <= 7 -> (if hi1r2 <= v2 then v2 else hi1r2) <= vr22. Admitted.
+Hint Resolve pure4: ssl_pure.
 
 Definition bst_left_rotate_type :=
   forall (vprogs : ptr * ptr),
@@ -37,20 +37,25 @@ Definition bst_left_rotate_type :=
       let: (x, retv) := vprogs in
       let: (sz1, sz2, v, hi1, r, lo2, l, lo1, hi2, unused) := vghosts in
       exists sz3 sz4 v3 hi3 lo4 lo3 r3 hi4 y,
-      exists h_bst_xsz3lo3hi3_564 h_bst_r3sz4lo4hi4_565,
-      0 <= sz3 /\ 0 <= sz4 /\ 0 <= v3 /\ hi3 <= v3 /\ sz3 + sz4 == sz1 + sz2 /\ v3 <= 7 /\ v3 <= lo4 /\ h = retv :-> y \+ y :-> v3 \+ y .+ 1 :-> x \+ y .+ 2 :-> r3 \+ h_bst_xsz3lo3hi3_564 \+ h_bst_r3sz4lo4hi4_565 /\ bst x sz3 lo3 hi3 h_bst_xsz3lo3hi3_564 /\ bst r3 sz4 lo4 hi4 h_bst_r3sz4lo4hi4_565
+      exists h_bst_xsz3lo3hi3_515 h_bst_r3sz4lo4hi4_516,
+      0 <= sz3 /\ 0 <= sz4 /\ 0 <= v3 /\ hi3 <= v3 /\ sz3 + sz4 == sz1 + sz2 /\ v3 <= 7 /\ v3 <= lo4 /\ h = retv :-> y \+ y :-> v3 \+ y .+ 1 :-> x \+ y .+ 2 :-> r3 \+ h_bst_xsz3lo3hi3_515 \+ h_bst_r3sz4lo4hi4_516 /\ bst x sz3 lo3 hi3 h_bst_xsz3lo3hi3_515 /\ bst r3 sz4 lo4 hi4 h_bst_r3sz4lo4hi4_516
     ]).
 
 Program Definition bst_left_rotate : bst_left_rotate_type :=
   Fix (fun (bst_left_rotate : bst_left_rotate_type) vprogs =>
     let: (x, retv) := vprogs in
     Do (
+      unused2 <-- @read ptr retv;
+      v2 <-- @read nat x;
+      l2 <-- @read ptr (x .+ 1);
       r2 <-- @read ptr (x .+ 2);
       if r2 == null
       then
         ret tt
       else
+        vr22 <-- @read nat r2;
         lr22 <-- @read ptr (r2 .+ 1);
+        rr22 <-- @read ptr (r2 .+ 2);
         (r2 .+ 1) ::= x;;
         retv ::= r2;;
         (x .+ 2) ::= lr22;;
@@ -59,39 +64,116 @@ Program Definition bst_left_rotate : bst_left_rotate_type :=
 Obligation Tactic := intro; move=>[x retv]; ssl_program_simpl.
 Next Obligation.
 ssl_ghostelim_pre.
-move=>[[[[[[[[[sz1 sz2] v2] hi1] r2] lo2] l2] lo1] hi2] unused2].
-ex_elim h_bst_l2sz1lo1hi1_a h_bst_r2sz2lo2hi2_b.
+move=>[[[[[[[[[sz1 sz2] v] hi1] r] lo2] l] lo1] hi2] unused].
+ex_elim h_bst_lsz1lo1hi1_a h_bst_rsz2lo2hi2_b.
 move=>[phi_self0] [phi_self1] [phi_self2] [phi_self3] [phi_self4] [phi_self5] [phi_self6].
 move=>[sigma_self].
 subst h_self.
-move=>[H_bst_l2sz1lo1hi1_a H_bst_r2sz2lo2hi2_b].
+move=>[H_bst_lsz1lo1hi1_a H_bst_rsz2lo2hi2_b].
 ssl_ghostelim_post.
+ssl_read retv.
+try rename unused into unused2.
+ssl_read x.
+try rename v into v2.
+ssl_read (x .+ 1).
+try rename l into l2.
+try rename h_bst_lsz1lo1hi1_a into h_bst_l2sz1lo1hi1_a.
+try rename H_bst_lsz1lo1hi1_a into H_bst_l2sz1lo1hi1_a.
 ssl_read (x .+ 2).
-ssl_open (r2 == null);
-ssl_open_post H_bst_r2sz2lo2hi2_b.
-ex_elim sz1r2 sz2r2 vr22 hi2r2 hi1r2.
-ex_elim lo1r2 lo2r2 lr22 rr22.
-ex_elim h_bst_lr22sz1r2lo1r2hi1r2_562r2 h_bst_rr22sz2r2lo2r2hi2r2_563r2.
+try rename r into r2.
+try rename h_bst_rsz2lo2hi2_b into h_bst_r2sz2lo2hi2_b.
+try rename H_bst_rsz2lo2hi2_b into H_bst_r2sz2lo2hi2_b.
+ssl_open (r2 == null) H_bst_r2sz2lo2hi2_b.
+move=>[phi_bst_r2sz2lo2hi2_b0] [phi_bst_r2sz2lo2hi2_b1] [phi_bst_r2sz2lo2hi2_b2].
+move=>[sigma_bst_r2sz2lo2hi2_b].
+subst h_bst_r2sz2lo2hi2_b.
+shelve.
+ex_elim sz1r2 sz2r2 vr2 hi2r2 hi1r2.
+ex_elim lo1r2 lo2r2 lr2 rr2.
+ex_elim h_bst_lr2sz1r2lo1r2hi1r2_513r2 h_bst_rr2sz2r2lo2r2hi2r2_514r2.
 move=>[phi_bst_r2sz2lo2hi2_b0] [phi_bst_r2sz2lo2hi2_b1] [phi_bst_r2sz2lo2hi2_b2] [phi_bst_r2sz2lo2hi2_b3] [phi_bst_r2sz2lo2hi2_b4] [phi_bst_r2sz2lo2hi2_b5] [phi_bst_r2sz2lo2hi2_b6] [phi_bst_r2sz2lo2hi2_b7] [phi_bst_r2sz2lo2hi2_b8].
 move=>[sigma_bst_r2sz2lo2hi2_b].
 subst h_bst_r2sz2lo2hi2_b.
-move=>[H_bst_lr22sz1r2lo1r2hi1r2_562r2 H_bst_rr22sz2r2lo2r2hi2r2_563r2].
+move=>[H_bst_lr2sz1r2lo1r2hi1r2_513r2 H_bst_rr2sz2r2lo2r2hi2r2_514r2].
+shelve.
+Unshelve.
+ssl_inconsistency.
+try rename h_bst_r2sz2lo2hi2_b into h_bst_r2sz2lo2hi2r2vr2vr2hi2r2_b.
+try rename H_bst_r2sz2lo2hi2_b into H_bst_r2sz2lo2hi2r2vr2vr2hi2r2_b.
+try rename h_bst_r2sz2lo2hi2r2vr2vr2hi2r2_b into h_bst_r2sz2vr2lo1r2vr2lo1r2hi2r2vr2vr2hi2r2_b.
+try rename H_bst_r2sz2lo2hi2r2vr2vr2hi2r2_b into H_bst_r2sz2vr2lo1r2vr2lo1r2hi2r2vr2vr2hi2r2_b.
+try rename h_bst_r2sz2vr2lo1r2vr2lo1r2hi2r2vr2vr2hi2r2_b into h_bst_r2sz1r2sz2r2vr2lo1r2vr2lo1r2hi2r2vr2vr2hi2r2_b.
+try rename H_bst_r2sz2vr2lo1r2vr2lo1r2hi2r2vr2vr2hi2r2_b into H_bst_r2sz1r2sz2r2vr2lo1r2vr2lo1r2hi2r2vr2vr2hi2r2_b.
+ssl_read r2.
+try rename vr2 into vr22.
+try rename h_bst_r2sz1r2sz2r2vr2lo1r2vr2lo1r2hi2r2vr2vr2hi2r2_b into h_bst_r2sz1r2sz2r2vr22lo1r2vr22lo1r2hi2r2vr22vr22hi2r2_b.
+try rename H_bst_r2sz1r2sz2r2vr2lo1r2vr2lo1r2hi2r2vr2vr2hi2r2_b into H_bst_r2sz1r2sz2r2vr22lo1r2vr22lo1r2hi2r2vr22vr22hi2r2_b.
 ssl_read (r2 .+ 1).
+try rename lr2 into lr22.
+try rename h_bst_lr2sz1r2lo1r2hi1r2_513r2 into h_bst_lr22sz1r2lo1r2hi1r2_513r2.
+try rename H_bst_lr2sz1r2lo1r2hi1r2_513r2 into H_bst_lr22sz1r2lo1r2hi1r2_513r2.
+ssl_read (r2 .+ 2).
+try rename rr2 into rr22.
+try rename h_bst_rr2sz2r2lo2r2hi2r2_514r2 into h_bst_rr22sz2r2lo2r2hi2r2_514r2.
+try rename H_bst_rr2sz2r2lo2r2hi2r2_514r2 into H_bst_rr22sz2r2lo2r2hi2r2_514r2.
+try rename h_bst_xsz3lo3hi3_515 into h_bst_xsz3lo3hi21xv1xv1xhi21x_515.
+try rename H_bst_xsz3lo3hi3_515 into H_bst_xsz3lo3hi21xv1xv1xhi21x_515.
+try rename h_bst_xsz3lo3hi21xv1xv1xhi21x_515 into h_bst_xsz3v1xlo11xv1xlo11xhi21xv1xv1xhi21x_515.
+try rename H_bst_xsz3lo3hi21xv1xv1xhi21x_515 into H_bst_xsz3v1xlo11xv1xlo11xhi21xv1xv1xhi21x_515.
+try rename h_bst_xsz3v1xlo11xv1xlo11xhi21xv1xv1xhi21x_515 into h_bst_xsz11xsz21xv1xlo11xv1xlo11xhi21xv1xv1xhi21x_515.
+try rename H_bst_xsz3v1xlo11xv1xlo11xhi21xv1xv1xhi21x_515 into H_bst_xsz11xsz21xv1xlo11xv1xlo11xhi21xv1xv1xhi21x_515.
+try rename h_bst_r3sz4lo4hi4_516 into h_bst_r3sz4lo4hi4_514r2.
+try rename H_bst_r3sz4lo4hi4_516 into H_bst_r3sz4lo4hi4_514r2.
+try rename h_bst_r3sz4lo4hi4_514r2 into h_bst_r3sz4lo4hi2r2_514r2.
+try rename H_bst_r3sz4lo4hi4_514r2 into H_bst_r3sz4lo4hi2r2_514r2.
+try rename h_bst_r3sz4lo4hi2r2_514r2 into h_bst_r3sz4lo2r2hi2r2_514r2.
+try rename H_bst_r3sz4lo4hi2r2_514r2 into H_bst_r3sz4lo2r2hi2r2_514r2.
+try rename h_bst_r3sz4lo2r2hi2r2_514r2 into h_bst_rr22sz4lo2r2hi2r2_514r2.
+try rename H_bst_r3sz4lo2r2hi2r2_514r2 into H_bst_rr22sz4lo2r2hi2r2_514r2.
+try rename h_bst_rr22sz4lo2r2hi2r2_514r2 into h_bst_rr22sz2r2lo2r2hi2r2_514r2.
+try rename H_bst_rr22sz4lo2r2hi2r2_514r2 into H_bst_rr22sz2r2lo2r2hi2r2_514r2.
+try rename h_bst_l1xsz11xlo11xhi11x_513x into h_bst_l1xsz11xlo11xhi11x_a.
+try rename H_bst_l1xsz11xlo11xhi11x_513x into H_bst_l1xsz11xlo11xhi11x_a.
+try rename h_bst_l1xsz11xlo11xhi11x_a into h_bst_l1xsz11xlo11xhi1_a.
+try rename H_bst_l1xsz11xlo11xhi11x_a into H_bst_l1xsz11xlo11xhi1_a.
+try rename h_bst_l1xsz11xlo11xhi1_a into h_bst_l2sz11xlo11xhi1_a.
+try rename H_bst_l1xsz11xlo11xhi1_a into H_bst_l2sz11xlo11xhi1_a.
+try rename h_bst_xsz11xsz21xv1xlo11xv1xlo11xhi21xv1xv1xhi21x_515 into h_bst_xsz11xsz21xv1xlo1v1xlo1hi21xv1xv1xhi21x_515.
+try rename H_bst_xsz11xsz21xv1xlo11xv1xlo11xhi21xv1xv1xhi21x_515 into H_bst_xsz11xsz21xv1xlo1v1xlo1hi21xv1xv1xhi21x_515.
+try rename h_bst_l2sz11xlo11xhi1_a into h_bst_l2sz11xlo1hi1_a.
+try rename H_bst_l2sz11xlo11xhi1_a into H_bst_l2sz11xlo1hi1_a.
+try rename h_bst_xsz11xsz21xv1xlo1v1xlo1hi21xv1xv1xhi21x_515 into h_bst_xsz1sz21xv1xlo1v1xlo1hi21xv1xv1xhi21x_515.
+try rename H_bst_xsz11xsz21xv1xlo1v1xlo1hi21xv1xv1xhi21x_515 into H_bst_xsz1sz21xv1xlo1v1xlo1hi21xv1xv1xhi21x_515.
+try rename h_bst_l2sz11xlo1hi1_a into h_bst_l2sz1lo1hi1_a.
+try rename H_bst_l2sz11xlo1hi1_a into H_bst_l2sz1lo1hi1_a.
+try rename h_bst_r1xsz21xlo21xhi21x_514x into h_bst_r1xsz21xlo21xhi21x_513r2.
+try rename H_bst_r1xsz21xlo21xhi21x_514x into H_bst_r1xsz21xlo21xhi21x_513r2.
+try rename h_bst_xsz1sz21xv1xlo1v1xlo1hi21xv1xv1xhi21x_515 into h_bst_xsz1sz21xv1xlo1v1xlo1hi1r2v1xv1xhi1r2_515.
+try rename H_bst_xsz1sz21xv1xlo1v1xlo1hi21xv1xv1xhi21x_515 into H_bst_xsz1sz21xv1xlo1v1xlo1hi1r2v1xv1xhi1r2_515.
+try rename h_bst_r1xsz21xlo21xhi21x_513r2 into h_bst_r1xsz21xlo21xhi1r2_513r2.
+try rename H_bst_r1xsz21xlo21xhi21x_513r2 into H_bst_r1xsz21xlo21xhi1r2_513r2.
+try rename h_bst_r1xsz21xlo21xhi1r2_513r2 into h_bst_r1xsz21xlo1r2hi1r2_513r2.
+try rename H_bst_r1xsz21xlo21xhi1r2_513r2 into H_bst_r1xsz21xlo1r2hi1r2_513r2.
+try rename h_bst_r1xsz21xlo1r2hi1r2_513r2 into h_bst_lr22sz21xlo1r2hi1r2_513r2.
+try rename H_bst_r1xsz21xlo1r2hi1r2_513r2 into H_bst_lr22sz21xlo1r2hi1r2_513r2.
+try rename h_bst_lr22sz21xlo1r2hi1r2_513r2 into h_bst_lr22sz1r2lo1r2hi1r2_513r2.
+try rename H_bst_lr22sz21xlo1r2hi1r2_513r2 into H_bst_lr22sz1r2lo1r2hi1r2_513r2.
+try rename h_bst_xsz1sz21xv1xlo1v1xlo1hi1r2v1xv1xhi1r2_515 into h_bst_xsz1sz1r2v1xlo1v1xlo1hi1r2v1xv1xhi1r2_515.
+try rename H_bst_xsz1sz21xv1xlo1v1xlo1hi1r2v1xv1xhi1r2_515 into H_bst_xsz1sz1r2v1xlo1v1xlo1hi1r2v1xv1xhi1r2_515.
 ssl_write (r2 .+ 1).
 ssl_write_post (r2 .+ 1).
 ssl_write retv.
 ssl_write_post retv.
 ssl_write (x .+ 2).
 ssl_write_post (x .+ 2).
+try rename h_bst_xsz1sz1r2v1xlo1v1xlo1hi1r2v1xv1xhi1r2_515 into h_bst_xsz1sz1r2v2lo1v2lo1hi1r2v2v2hi1r2_515.
+try rename H_bst_xsz1sz1r2v1xlo1v1xlo1hi1r2v1xv1xhi1r2_515 into H_bst_xsz1sz1r2v2lo1v2lo1hi1r2v2v2hi1r2_515.
 ssl_emp;
 exists (1 + sz1 + sz1r2), (sz2r2), (vr22), ((if hi1r2 <= v2 then v2 else hi1r2)), (lo2r2), ((if v2 <= lo1 then v2 else lo1)), (rr22), (hi2r2), (r2);
-exists (x :-> v2 \+ x .+ 1 :-> l2 \+ x .+ 2 :-> lr22 \+ h_bst_l2sz1lo1hi1_a \+ h_bst_lr22sz1r2lo1r2hi1r2_562r2);
-exists (h_bst_rr22sz2r2lo2r2hi2r2_563r2);
-sslauto;
-solve [
+exists (x :-> v2 \+ x .+ 1 :-> l2 \+ x .+ 2 :-> lr22 \+ h_bst_l2sz1lo1hi1_a \+ h_bst_lr22sz1r2lo1r2hi1r2_513r2);
+exists (h_bst_rr22sz2r2lo2r2hi2r2_514r2);
+sslauto.
 unfold_constructor 2;
-exists (sz1), (sz1r2), (v2), (hi1r2), (hi1), (lo1), (lo1r2), (l2), (lr22);
-exists (h_bst_l2sz1lo1hi1_a);
-exists (h_bst_lr22sz1r2lo1r2hi1r2_562r2);
-sslauto ].
+exists (sz1), (sz1r2), (v2), (hi1r2), (hi1), (lo1), (lo1r2), (l2), (lr22), (h_bst_l2sz1lo1hi1_a), (h_bst_lr22sz1r2lo1r2hi1r2_513r2);
+sslauto.
 Qed.
