examples/bst_remove_root_no_left.v
@@ -12,21 +12,21 @@ Inductive bst (x : ptr) (sz : nat) (lo : nat) (hi : nat) (h : heap) : Prop :=
   hi == 0 /\ lo == 7 /\ sz == 0 /\ h = empty
 | bst_2 of (x == null) = false of
   exists (sz1 : nat) (sz2 : nat) (v : nat) (hi2 : nat) (hi1 : nat) (lo1 : nat) (lo2 : nat) (l : ptr) (r : ptr),
-  exists h_bst_lsz1lo1hi1_566 h_bst_rsz2lo2hi2_567,
-  0 <= sz1 /\ 0 <= sz2 /\ 0 <= v /\ hi == (if hi2 <= v then v else hi2) /\ hi1 <= v /\ lo == (if v <= lo1 then v else lo1) /\ sz == 1 + sz1 + sz2 /\ v <= 7 /\ v <= lo2 /\ h = x :-> v \+ x .+ 1 :-> l \+ x .+ 2 :-> r \+ h_bst_lsz1lo1hi1_566 \+ h_bst_rsz2lo2hi2_567 /\ bst l sz1 lo1 hi1 h_bst_lsz1lo1hi1_566 /\ bst r sz2 lo2 hi2 h_bst_rsz2lo2hi2_567.
+  exists h_bst_lsz1lo1hi1_517 h_bst_rsz2lo2hi2_518,
+  0 <= sz1 /\ 0 <= sz2 /\ 0 <= v /\ hi == (if hi2 <= v then v else hi2) /\ hi1 <= v /\ lo == (if v <= lo1 then v else lo1) /\ sz == 1 + sz1 + sz2 /\ v <= 7 /\ v <= lo2 /\ h = x :-> v \+ x .+ 1 :-> l \+ x .+ 2 :-> r \+ h_bst_lsz1lo1hi1_517 \+ h_bst_rsz2lo2hi2_518 /\ bst l sz1 lo1 hi1 h_bst_lsz1lo1hi1_517 /\ bst r sz2 lo2 hi2 h_bst_rsz2lo2hi2_518.
 
-Lemma pure54 r2 : r2 == null -> (if null == null then (if r2 == null then 7 else 7) else 7) == 7. Admitted.
-Hint Resolve pure54: ssl_pure.
-Lemma pure55 r2 : r2 == null -> (if r2 == null then (if null == null then 0 else 0) else 0) == 0. Admitted.
-Hint Resolve pure55: ssl_pure.
-Lemma pure56 : 0 == 0. Admitted.
-Hint Resolve pure56: ssl_pure.
-Lemma pure57 sz1r2 sz2r2 : 0 <= sz2r2 -> 0 <= sz1r2 -> 0 <= 1 + sz1r2 + sz2r2 -> 1 + sz1r2 + sz2r2 == 1 + sz1r2 + sz2r2. Admitted.
-Hint Resolve pure57: ssl_pure.
-Lemma pure58 lo1r2 vr22 x v2 hi1r2 retv lo2r2 hi2r2 r2 : vr22 <= 7 -> (r2 == retv) = false -> (retv == null) = false -> v2 <= (if vr22 <= lo1r2 then vr22 else lo1r2) -> 0 <= v2 -> (r2 == null) = false -> vr22 <= lo2r2 -> 0 <= vr22 -> (r2 == x) = false -> hi1r2 <= vr22 -> (x == null) = false -> (retv == x) = false -> v2 <= 7 -> (if r2 == null then (if null == null then 0 else 0) else (if hi2r2 <= vr22 then vr22 else hi2r2)) == (if hi2r2 <= vr22 then vr22 else hi2r2). Admitted.
-Hint Resolve pure58: ssl_pure.
-Lemma pure59 lo1r2 vr22 x v2 hi1r2 retv lo2r2 r2 : vr22 <= 7 -> (r2 == retv) = false -> (retv == null) = false -> v2 <= (if vr22 <= lo1r2 then vr22 else lo1r2) -> 0 <= v2 -> (r2 == null) = false -> vr22 <= lo2r2 -> 0 <= vr22 -> (r2 == x) = false -> hi1r2 <= vr22 -> (x == null) = false -> (retv == x) = false -> v2 <= 7 -> (if null == null then (if r2 == null then 7 else (if vr22 <= lo1r2 then vr22 else lo1r2)) else 7) == (if vr22 <= lo1r2 then vr22 else lo1r2). Admitted.
-Hint Resolve pure59: ssl_pure.
+Lemma pure5 r2 : r2 == null -> (if null == null then (if r2 == null then 7 else 7) else 7) == 7. Admitted.
+Hint Resolve pure5: ssl_pure.
+Lemma pure6 r2 : r2 == null -> (if r2 == null then (if null == null then 0 else 0) else 0) == 0. Admitted.
+Hint Resolve pure6: ssl_pure.
+Lemma pure7 : 0 == 0. Admitted.
+Hint Resolve pure7: ssl_pure.
+Lemma pure8 sz1r2 sz2r2 : 0 <= 1 + sz1r2 + sz2r2 -> 0 <= sz2r2 -> 0 <= sz1r2 -> 1 + sz1r2 + sz2r2 == 1 + sz1r2 + sz2r2. Admitted.
+Hint Resolve pure8: ssl_pure.
+Lemma pure9 lo1r2 vr22 x v2 hi1r2 retv lo2r2 hi2r2 r2 : vr22 <= 7 -> (r2 == retv) = false -> (retv == null) = false -> v2 <= (if vr22 <= lo1r2 then vr22 else lo1r2) -> 0 <= v2 -> (r2 == null) = false -> vr22 <= lo2r2 -> 0 <= vr22 -> (r2 == x) = false -> hi1r2 <= vr22 -> (x == null) = false -> (retv == x) = false -> v2 <= 7 -> (if r2 == null then (if null == null then 0 else 0) else (if hi2r2 <= vr22 then vr22 else hi2r2)) == (if hi2r2 <= vr22 then vr22 else hi2r2). Admitted.
+Hint Resolve pure9: ssl_pure.
+Lemma pure10 lo1r2 vr22 x v2 hi1r2 retv lo2r2 r2 : vr22 <= 7 -> (r2 == retv) = false -> (retv == null) = false -> v2 <= (if vr22 <= lo1r2 then vr22 else lo1r2) -> 0 <= v2 -> (r2 == null) = false -> vr22 <= lo2r2 -> 0 <= vr22 -> (r2 == x) = false -> hi1r2 <= vr22 -> (x == null) = false -> (retv == x) = false -> v2 <= 7 -> (if null == null then (if r2 == null then 7 else (if vr22 <= lo1r2 then vr22 else lo1r2)) else 7) == (if vr22 <= lo1r2 then vr22 else lo1r2). Admitted.
+Hint Resolve pure10: ssl_pure.
 
 Definition bst_remove_root_no_left_type :=
   forall (vprogs : ptr * ptr),
@@ -49,6 +49,8 @@ Program Definition bst_remove_root_no_left : bst_remove_root_no_left_type :=
   Fix (fun (bst_remove_root_no_left : bst_remove_root_no_left_type) vprogs =>
     let: (x, retv) := vprogs in
     Do (
+      unused2 <-- @read ptr retv;
+      v2 <-- @read nat x;
       r2 <-- @read ptr (x .+ 2);
       if null == null
       then
@@ -60,6 +62,9 @@ Program Definition bst_remove_root_no_left : bst_remove_root_no_left_type :=
           retv ::= null;;
           ret tt
         else
+          vr22 <-- @read nat r2;
+          lr22 <-- @read ptr (r2 .+ 1);
+          rr22 <-- @read ptr (r2 .+ 2);
           dealloc x;;
           dealloc (x .+ 1);;
           dealloc (x .+ 2);;
@@ -71,24 +76,86 @@ Program Definition bst_remove_root_no_left : bst_remove_root_no_left_type :=
 Obligation Tactic := intro; move=>[x retv]; ssl_program_simpl.
 Next Obligation.
 ssl_ghostelim_pre.
-move=>[[[[[[[[[sz1 sz2] v2] hi1] l] lo2] lo1] r2] hi2] unused2].
-ex_elim h_bst_lsz1lo1hi1_a h_bst_r2sz2lo2hi2_b.
+move=>[[[[[[[[[sz1 sz2] v] hi1] l] lo2] lo1] r] hi2] unused].
+ex_elim h_bst_lsz1lo1hi1_a h_bst_rsz2lo2hi2_b.
 move=>[phi_self0] [phi_self1] [phi_self2] [phi_self3] [phi_self4] [phi_self5] [phi_self6].
 move=>[sigma_self].
 subst h_self.
-move=>[H_bst_lsz1lo1hi1_a H_bst_r2sz2lo2hi2_b].
+move=>[H_bst_lsz1lo1hi1_a H_bst_rsz2lo2hi2_b].
 ssl_ghostelim_post.
+try rename h_bst_lsz1lo1hi1_a into h_bst_sz1lo1hi1_a.
+try rename H_bst_lsz1lo1hi1_a into H_bst_sz1lo1hi1_a.
+try rename h_bst_yn1lohi_c into h_bst_yn1lorhi1hi2_c.
+try rename H_bst_yn1lohi_c into H_bst_yn1lorhi1hi2_c.
+try rename h_bst_yn1lorhi1hi2_c into h_bst_yn1rlo2lo1rhi1hi2_c.
+try rename H_bst_yn1lorhi1hi2_c into H_bst_yn1rlo2lo1rhi1hi2_c.
+try rename h_bst_yn1rlo2lo1rhi1hi2_c into h_bst_ysz1sz2rlo2lo1rhi1hi2_c.
+try rename H_bst_yn1rlo2lo1rhi1hi2_c into H_bst_ysz1sz2rlo2lo1rhi1hi2_c.
+ssl_read retv.
+try rename unused into unused2.
+ssl_read x.
+try rename v into v2.
 ssl_read (x .+ 2).
-ssl_open (null == null);
-ssl_open_post H_bst_lsz1lo1hi1_a.
-move=>[phi_bst_lsz1lo1hi1_a0] [phi_bst_lsz1lo1hi1_a1] [phi_bst_lsz1lo1hi1_a2].
-move=>[sigma_bst_lsz1lo1hi1_a].
-subst h_bst_lsz1lo1hi1_a.
-ssl_open (r2 == null);
-ssl_open_post H_bst_r2sz2lo2hi2_b.
+try rename r into r2.
+try rename h_bst_ysz1sz2rlo2lo1rhi1hi2_c into h_bst_ysz1sz2r2lo2lo1r2hi1hi2_c.
+try rename H_bst_ysz1sz2rlo2lo1rhi1hi2_c into H_bst_ysz1sz2r2lo2lo1r2hi1hi2_c.
+try rename h_bst_rsz2lo2hi2_b into h_bst_r2sz2lo2hi2_b.
+try rename H_bst_rsz2lo2hi2_b into H_bst_r2sz2lo2hi2_b.
+ssl_open (null == null) H_bst_sz1lo1hi1_a.
+move=>[phi_bst_sz1lo1hi1_a0] [phi_bst_sz1lo1hi1_a1] [phi_bst_sz1lo1hi1_a2].
+move=>[sigma_bst_sz1lo1hi1_a].
+subst h_bst_sz1lo1hi1_a.
+shelve.
+ex_elim sz10 sz20 v0 hi20 hi10.
+ex_elim lo10 lo20 l0 r0.
+ex_elim h_bst_l0sz10lo10hi10_5170 h_bst_r0sz20lo20hi20_5180.
+move=>[phi_bst_sz1lo1hi1_a0] [phi_bst_sz1lo1hi1_a1] [phi_bst_sz1lo1hi1_a2] [phi_bst_sz1lo1hi1_a3] [phi_bst_sz1lo1hi1_a4] [phi_bst_sz1lo1hi1_a5] [phi_bst_sz1lo1hi1_a6] [phi_bst_sz1lo1hi1_a7] [phi_bst_sz1lo1hi1_a8].
+move=>[sigma_bst_sz1lo1hi1_a].
+subst h_bst_sz1lo1hi1_a.
+move=>[H_bst_l0sz10lo10hi10_5170 H_bst_r0sz20lo20hi20_5180].
+shelve.
+Unshelve.
+try rename h_bst_ysz1sz2r2lo2lo1r2hi1hi2_c into h_bst_ysz1sz2r2lo2lo1r2hi2_c.
+try rename H_bst_ysz1sz2r2lo2lo1r2hi1hi2_c into H_bst_ysz1sz2r2lo2lo1r2hi2_c.
+try rename h_bst_sz1lo1hi1_a into h_bst_sz1lo1_a.
+try rename H_bst_sz1lo1hi1_a into H_bst_sz1lo1_a.
+try rename h_bst_sz1lo1_a into h_bst_sz1_a.
+try rename H_bst_sz1lo1_a into H_bst_sz1_a.
+try rename h_bst_ysz1sz2r2lo2lo1r2hi2_c into h_bst_ysz1sz2r2lo2r2hi2_c.
+try rename H_bst_ysz1sz2r2lo2lo1r2hi2_c into H_bst_ysz1sz2r2lo2r2hi2_c.
+try rename h_bst_sz1_a into h_bst__a.
+try rename H_bst_sz1_a into H_bst__a.
+try rename h_bst_ysz1sz2r2lo2r2hi2_c into h_bst_ysz2r2lo2r2hi2_c.
+try rename H_bst_ysz1sz2r2lo2r2hi2_c into H_bst_ysz2r2lo2r2hi2_c.
+ssl_open (r2 == null) H_bst_r2sz2lo2hi2_b.
 move=>[phi_bst_r2sz2lo2hi2_b0] [phi_bst_r2sz2lo2hi2_b1] [phi_bst_r2sz2lo2hi2_b2].
 move=>[sigma_bst_r2sz2lo2hi2_b].
 subst h_bst_r2sz2lo2hi2_b.
+shelve.
+ex_elim sz1r2 sz2r2 vr2 hi2r2 hi1r2.
+ex_elim lo1r2 lo2r2 lr2 rr2.
+ex_elim h_bst_lr2sz1r2lo1r2hi1r2_517r2 h_bst_rr2sz2r2lo2r2hi2r2_518r2.
+move=>[phi_bst_r2sz2lo2hi2_b0] [phi_bst_r2sz2lo2hi2_b1] [phi_bst_r2sz2lo2hi2_b2] [phi_bst_r2sz2lo2hi2_b3] [phi_bst_r2sz2lo2hi2_b4] [phi_bst_r2sz2lo2hi2_b5] [phi_bst_r2sz2lo2hi2_b6] [phi_bst_r2sz2lo2hi2_b7] [phi_bst_r2sz2lo2hi2_b8].
+move=>[sigma_bst_r2sz2lo2hi2_b].
+subst h_bst_r2sz2lo2hi2_b.
+move=>[H_bst_lr2sz1r2lo1r2hi1r2_517r2 H_bst_rr2sz2r2lo2r2hi2r2_518r2].
+shelve.
+shelve.
+Unshelve.
+try rename h_bst_r2sz2lo2hi2_b into h_bst_r2sz2lo2_b.
+try rename H_bst_r2sz2lo2hi2_b into H_bst_r2sz2lo2_b.
+try rename h_bst_ysz2r2lo2r2hi2_c into h_bst_ysz2r2lo2r2_c.
+try rename H_bst_ysz2r2lo2r2hi2_c into H_bst_ysz2r2lo2r2_c.
+try rename h_bst_ysz2r2lo2r2_c into h_bst_ysz2r2r2_c.
+try rename H_bst_ysz2r2lo2r2_c into H_bst_ysz2r2r2_c.
+try rename h_bst_r2sz2lo2_b into h_bst_r2sz2_b.
+try rename H_bst_r2sz2lo2_b into H_bst_r2sz2_b.
+try rename h_bst_ysz2r2r2_c into h_bst_yr2r2_c.
+try rename H_bst_ysz2r2r2_c into H_bst_yr2r2_c.
+try rename h_bst_r2sz2_b into h_bst_r2_b.
+try rename H_bst_r2sz2_b into H_bst_r2_b.
+try rename h_bst_yr2r2_c into h_bst_r2r2_c.
+try rename H_bst_yr2r2_c into H_bst_r2r2_c.
 ssl_dealloc x.
 ssl_dealloc (x .+ 1).
 ssl_dealloc (x .+ 2).
@@ -97,17 +164,57 @@ ssl_write_post retv.
 ssl_emp;
 exists ((if r2 == null then (if null == null then 0 else 0) else 0)), ((if null == null then (if r2 == null then 7 else 7) else 7)), (0 + 0), (null);
 exists (empty);
-sslauto;
-solve [
+sslauto.
 unfold_constructor 1;
-sslauto ].
-ex_elim sz1r2 sz2r2 vr22 hi2r2 hi1r2.
-ex_elim lo1r2 lo2r2 lr22 rr22.
-ex_elim h_bst_lr22sz1r2lo1r2hi1r2_566r2 h_bst_rr22sz2r2lo2r2hi2r2_567r2.
-move=>[phi_bst_r2sz2lo2hi2_b0] [phi_bst_r2sz2lo2hi2_b1] [phi_bst_r2sz2lo2hi2_b2] [phi_bst_r2sz2lo2hi2_b3] [phi_bst_r2sz2lo2hi2_b4] [phi_bst_r2sz2lo2hi2_b5] [phi_bst_r2sz2lo2hi2_b6] [phi_bst_r2sz2lo2hi2_b7] [phi_bst_r2sz2lo2hi2_b8].
-move=>[sigma_bst_r2sz2lo2hi2_b].
-subst h_bst_r2sz2lo2hi2_b.
-move=>[H_bst_lr22sz1r2lo1r2hi1r2_566r2 H_bst_rr22sz2r2lo2r2hi2r2_567r2].
+sslauto.
+try rename h_bst_r2sz2lo2hi2_b into h_bst_r2sz2lo2hi2r2vr2vr2hi2r2_b.
+try rename H_bst_r2sz2lo2hi2_b into H_bst_r2sz2lo2hi2r2vr2vr2hi2r2_b.
+try rename h_bst_ysz2r2lo2r2hi2_c into h_bst_ysz2r2lo2r2hi2r2vr2vr2hi2r2_c.
+try rename H_bst_ysz2r2lo2r2hi2_c into H_bst_ysz2r2lo2r2hi2r2vr2vr2hi2r2_c.
+try rename h_bst_r2sz2lo2hi2r2vr2vr2hi2r2_b into h_bst_r2sz2vr2lo1r2vr2lo1r2hi2r2vr2vr2hi2r2_b.
+try rename H_bst_r2sz2lo2hi2r2vr2vr2hi2r2_b into H_bst_r2sz2vr2lo1r2vr2lo1r2hi2r2vr2vr2hi2r2_b.
+try rename h_bst_ysz2r2lo2r2hi2r2vr2vr2hi2r2_c into h_bst_ysz2r2vr2lo1r2vr2lo1r2r2hi2r2vr2vr2hi2r2_c.
+try rename H_bst_ysz2r2lo2r2hi2r2vr2vr2hi2r2_c into H_bst_ysz2r2vr2lo1r2vr2lo1r2r2hi2r2vr2vr2hi2r2_c.
+try rename h_bst_ysz2r2vr2lo1r2vr2lo1r2r2hi2r2vr2vr2hi2r2_c into h_bst_ysz1r2sz2r2r2vr2lo1r2vr2lo1r2r2hi2r2vr2vr2hi2r2_c.
+try rename H_bst_ysz2r2vr2lo1r2vr2lo1r2r2hi2r2vr2vr2hi2r2_c into H_bst_ysz1r2sz2r2r2vr2lo1r2vr2lo1r2r2hi2r2vr2vr2hi2r2_c.
+try rename h_bst_r2sz2vr2lo1r2vr2lo1r2hi2r2vr2vr2hi2r2_b into h_bst_r2sz1r2sz2r2vr2lo1r2vr2lo1r2hi2r2vr2vr2hi2r2_b.
+try rename H_bst_r2sz2vr2lo1r2vr2lo1r2hi2r2vr2vr2hi2r2_b into H_bst_r2sz1r2sz2r2vr2lo1r2vr2lo1r2hi2r2vr2vr2hi2r2_b.
+ssl_read r2.
+try rename vr2 into vr22.
+try rename h_bst_r2sz1r2sz2r2vr2lo1r2vr2lo1r2hi2r2vr2vr2hi2r2_b into h_bst_r2sz1r2sz2r2vr22lo1r2vr22lo1r2hi2r2vr22vr22hi2r2_b.
+try rename H_bst_r2sz1r2sz2r2vr2lo1r2vr2lo1r2hi2r2vr2vr2hi2r2_b into H_bst_r2sz1r2sz2r2vr22lo1r2vr22lo1r2hi2r2vr22vr22hi2r2_b.
+try rename h_bst_ysz1r2sz2r2r2vr2lo1r2vr2lo1r2r2hi2r2vr2vr2hi2r2_c into h_bst_ysz1r2sz2r2r2vr22lo1r2vr22lo1r2r2hi2r2vr22vr22hi2r2_c.
+try rename H_bst_ysz1r2sz2r2r2vr2lo1r2vr2lo1r2r2hi2r2vr2vr2hi2r2_c into H_bst_ysz1r2sz2r2r2vr22lo1r2vr22lo1r2r2hi2r2vr22vr22hi2r2_c.
+ssl_read (r2 .+ 1).
+try rename lr2 into lr22.
+try rename h_bst_lr2sz1r2lo1r2hi1r2_517r2 into h_bst_lr22sz1r2lo1r2hi1r2_517r2.
+try rename H_bst_lr2sz1r2lo1r2hi1r2_517r2 into H_bst_lr22sz1r2lo1r2hi1r2_517r2.
+ssl_read (r2 .+ 2).
+try rename rr2 into rr22.
+try rename h_bst_rr2sz2r2lo2r2hi2r2_518r2 into h_bst_rr22sz2r2lo2r2hi2r2_518r2.
+try rename H_bst_rr2sz2r2lo2r2hi2r2_518r2 into H_bst_rr22sz2r2lo2r2hi2r2_518r2.
+try rename h_bst_l1ysz11ylo11yhi11y_517y into h_bst_l1ysz11ylo11yhi11y_517r2.
+try rename H_bst_l1ysz11ylo11yhi11y_517y into H_bst_l1ysz11ylo11yhi11y_517r2.
+try rename h_bst_l1ysz11ylo11yhi11y_517r2 into h_bst_l1ysz11ylo11yhi1r2_517r2.
+try rename H_bst_l1ysz11ylo11yhi11y_517r2 into H_bst_l1ysz11ylo11yhi1r2_517r2.
+try rename h_bst_l1ysz11ylo11yhi1r2_517r2 into h_bst_lr22sz11ylo11yhi1r2_517r2.
+try rename H_bst_l1ysz11ylo11yhi1r2_517r2 into H_bst_lr22sz11ylo11yhi1r2_517r2.
+try rename h_bst_lr22sz11ylo11yhi1r2_517r2 into h_bst_lr22sz11ylo1r2hi1r2_517r2.
+try rename H_bst_lr22sz11ylo11yhi1r2_517r2 into H_bst_lr22sz11ylo1r2hi1r2_517r2.
+try rename h_bst_lr22sz11ylo1r2hi1r2_517r2 into h_bst_lr22sz1r2lo1r2hi1r2_517r2.
+try rename H_bst_lr22sz11ylo1r2hi1r2_517r2 into H_bst_lr22sz1r2lo1r2hi1r2_517r2.
+try rename h_bst_r1ysz21ylo21yhi21y_518y into h_bst_r1ysz21ylo21yhi21y_518r2.
+try rename H_bst_r1ysz21ylo21yhi21y_518y into H_bst_r1ysz21ylo21yhi21y_518r2.
+try rename h_bst_r1ysz21ylo21yhi21y_518r2 into h_bst_r1ysz21ylo21yhi2r2_518r2.
+try rename H_bst_r1ysz21ylo21yhi21y_518r2 into H_bst_r1ysz21ylo21yhi2r2_518r2.
+try rename h_bst_r1ysz21ylo21yhi2r2_518r2 into h_bst_r1ysz21ylo2r2hi2r2_518r2.
+try rename H_bst_r1ysz21ylo21yhi2r2_518r2 into H_bst_r1ysz21ylo2r2hi2r2_518r2.
+try rename h_bst_r1ysz21ylo2r2hi2r2_518r2 into h_bst_rr22sz21ylo2r2hi2r2_518r2.
+try rename H_bst_r1ysz21ylo2r2hi2r2_518r2 into H_bst_rr22sz21ylo2r2hi2r2_518r2.
+try rename h_bst_rr22sz21ylo2r2hi2r2_518r2 into h_bst_rr22sz2r2lo2r2hi2r2_518r2.
+try rename H_bst_rr22sz21ylo2r2hi2r2_518r2 into H_bst_rr22sz2r2lo2r2hi2r2_518r2.
+try rename h_bst_ysz1r2sz2r2r2vr22lo1r2vr22lo1r2r2hi2r2vr22vr22hi2r2_c into h_bst_r2sz1r2sz2r2r2vr22lo1r2vr22lo1r2r2hi2r2vr22vr22hi2r2_c.
+try rename H_bst_ysz1r2sz2r2r2vr22lo1r2vr22lo1r2r2hi2r2vr22vr22hi2r2_c into H_bst_r2sz1r2sz2r2r2vr22lo1r2vr22lo1r2r2hi2r2vr22vr22hi2r2_c.
 ssl_dealloc x.
 ssl_dealloc (x .+ 1).
 ssl_dealloc (x .+ 2).
@@ -115,12 +222,10 @@ ssl_write retv.
 ssl_write_post retv.
 ssl_emp;
 exists ((if r2 == null then (if null == null then 0 else 0) else (if hi2r2 <= vr22 then vr22 else hi2r2))), ((if null == null then (if r2 == null then 7 else (if vr22 <= lo1r2 then vr22 else lo1r2)) else 7)), (0 + 1 + sz1r2 + sz2r2), (r2);
-exists (r2 :-> vr22 \+ r2 .+ 1 :-> lr22 \+ r2 .+ 2 :-> rr22 \+ h_bst_lr22sz1r2lo1r2hi1r2_566r2 \+ h_bst_rr22sz2r2lo2r2hi2r2_567r2);
-sslauto;
-solve [
+exists (r2 :-> vr22 \+ r2 .+ 1 :-> lr22 \+ r2 .+ 2 :-> rr22 \+ h_bst_lr22sz1r2lo1r2hi1r2_517r2 \+ h_bst_rr22sz2r2lo2r2hi2r2_518r2);
+sslauto.
 unfold_constructor 2;
-exists (sz1r2), (sz2r2), (vr22), (hi2r2), (hi1r2), (lo1r2), (lo2r2), (lr22), (rr22);
-exists (h_bst_lr22sz1r2lo1r2hi1r2_566r2);
-exists (h_bst_rr22sz2r2lo2r2hi2r2_567r2);
-sslauto ].
+exists (sz1r2), (sz2r2), (vr22), (hi2r2), (hi1r2), (lo1r2), (lo2r2), (lr22), (rr22), (h_bst_lr22sz1r2lo1r2hi1r2_517r2), (h_bst_rr22sz2r2lo2r2hi2r2_518r2);
+sslauto.
+ssl_inconsistency.
 Qed.
