examples/bst_remove_root_no_right.v
@@ -12,21 +12,21 @@ Inductive bst (x : ptr) (sz : nat) (lo : nat) (hi : nat) (h : heap) : Prop :=
   hi == 0 /\ lo == 7 /\ sz == 0 /\ h = empty
 | bst_2 of (x == null) = false of
   exists (sz1 : nat) (sz2 : nat) (v : nat) (hi2 : nat) (hi1 : nat) (lo1 : nat) (lo2 : nat) (l : ptr) (r : ptr),
-  exists h_bst_lsz1lo1hi1_572 h_bst_rsz2lo2hi2_573,
-  0 <= sz1 /\ 0 <= sz2 /\ 0 <= v /\ hi == (if hi2 <= v then v else hi2) /\ hi1 <= v /\ lo == (if v <= lo1 then v else lo1) /\ sz == 1 + sz1 + sz2 /\ v <= 7 /\ v <= lo2 /\ h = x :-> v \+ x .+ 1 :-> l \+ x .+ 2 :-> r \+ h_bst_lsz1lo1hi1_572 \+ h_bst_rsz2lo2hi2_573 /\ bst l sz1 lo1 hi1 h_bst_lsz1lo1hi1_572 /\ bst r sz2 lo2 hi2 h_bst_rsz2lo2hi2_573.
+  exists h_bst_lsz1lo1hi1_523 h_bst_rsz2lo2hi2_524,
+  0 <= sz1 /\ 0 <= sz2 /\ 0 <= v /\ hi == (if hi2 <= v then v else hi2) /\ hi1 <= v /\ lo == (if v <= lo1 then v else lo1) /\ sz == 1 + sz1 + sz2 /\ v <= 7 /\ v <= lo2 /\ h = x :-> v \+ x .+ 1 :-> l \+ x .+ 2 :-> r \+ h_bst_lsz1lo1hi1_523 \+ h_bst_rsz2lo2hi2_524 /\ bst l sz1 lo1 hi1 h_bst_lsz1lo1hi1_523 /\ bst r sz2 lo2 hi2 h_bst_rsz2lo2hi2_524.
 
-Lemma pure82 l2 : l2 == null -> (if null == null then (if l2 == null then 0 else 0) else 0) == 0. Admitted.
-Hint Resolve pure82: ssl_pure.
-Lemma pure83 l2 : l2 == null -> (if l2 == null then (if null == null then 7 else 7) else 7) == 7. Admitted.
-Hint Resolve pure83: ssl_pure.
-Lemma pure84 : 0 == 0. Admitted.
-Hint Resolve pure84: ssl_pure.
-Lemma pure85 sz1l2 sz2l2 : 0 <= 1 + sz1l2 + sz2l2 -> 0 <= sz1l2 -> 0 <= sz2l2 -> 1 + sz1l2 + sz2l2 == 1 + sz1l2 + sz2l2. Admitted.
-Hint Resolve pure85: ssl_pure.
-Lemma pure86 lo2l2 x v2 retv vl22 l2 hi2l2 hi1l2 : (if hi2l2 <= vl22 then vl22 else hi2l2) <= v2 -> hi1l2 <= vl22 -> vl22 <= 7 -> (retv == null) = false -> (l2 == x) = false -> 0 <= v2 -> (l2 == retv) = false -> (l2 == null) = false -> (x == null) = false -> 0 <= vl22 -> (retv == x) = false -> vl22 <= lo2l2 -> v2 <= 7 -> (if null == null then (if l2 == null then 0 else (if hi2l2 <= vl22 then vl22 else hi2l2)) else 0) == (if hi2l2 <= vl22 then vl22 else hi2l2). Admitted.
-Hint Resolve pure86: ssl_pure.
-Lemma pure87 lo2l2 x v2 retv lo1l2 vl22 l2 hi2l2 hi1l2 : (if hi2l2 <= vl22 then vl22 else hi2l2) <= v2 -> hi1l2 <= vl22 -> vl22 <= 7 -> (retv == null) = false -> (l2 == x) = false -> 0 <= v2 -> (l2 == retv) = false -> (l2 == null) = false -> (x == null) = false -> 0 <= vl22 -> (retv == x) = false -> vl22 <= lo2l2 -> v2 <= 7 -> (if l2 == null then (if null == null then 7 else 7) else (if vl22 <= lo1l2 then vl22 else lo1l2)) == (if vl22 <= lo1l2 then vl22 else lo1l2). Admitted.
-Hint Resolve pure87: ssl_pure.
+Lemma pure33 l2 : l2 == null -> (if null == null then (if l2 == null then 0 else 0) else 0) == 0. Admitted.
+Hint Resolve pure33: ssl_pure.
+Lemma pure34 l2 : l2 == null -> (if l2 == null then (if null == null then 7 else 7) else 7) == 7. Admitted.
+Hint Resolve pure34: ssl_pure.
+Lemma pure35 : 0 == 0. Admitted.
+Hint Resolve pure35: ssl_pure.
+Lemma pure36 sz1l2 sz2l2 : 0 <= sz2l2 -> 0 <= sz1l2 -> 0 <= 1 + sz1l2 + sz2l2 -> 1 + sz1l2 + sz2l2 == 1 + sz1l2 + sz2l2. Admitted.
+Hint Resolve pure36: ssl_pure.
+Lemma pure37 lo2l2 x v2 retv vl22 l2 hi2l2 hi1l2 : (if hi2l2 <= vl22 then vl22 else hi2l2) <= v2 -> hi1l2 <= vl22 -> vl22 <= 7 -> (retv == null) = false -> (l2 == x) = false -> 0 <= v2 -> (l2 == retv) = false -> (l2 == null) = false -> (x == null) = false -> 0 <= vl22 -> (retv == x) = false -> vl22 <= lo2l2 -> v2 <= 7 -> (if null == null then (if l2 == null then 0 else (if hi2l2 <= vl22 then vl22 else hi2l2)) else 0) == (if hi2l2 <= vl22 then vl22 else hi2l2). Admitted.
+Hint Resolve pure37: ssl_pure.
+Lemma pure38 lo2l2 x v2 retv lo1l2 vl22 l2 hi2l2 hi1l2 : (if hi2l2 <= vl22 then vl22 else hi2l2) <= v2 -> hi1l2 <= vl22 -> vl22 <= 7 -> (retv == null) = false -> (l2 == x) = false -> 0 <= v2 -> (l2 == retv) = false -> (l2 == null) = false -> (x == null) = false -> 0 <= vl22 -> (retv == x) = false -> vl22 <= lo2l2 -> v2 <= 7 -> (if l2 == null then (if null == null then 7 else 7) else (if vl22 <= lo1l2 then vl22 else lo1l2)) == (if vl22 <= lo1l2 then vl22 else lo1l2). Admitted.
+Hint Resolve pure38: ssl_pure.
 
 Definition bst_remove_root_no_right_type :=
   forall (vprogs : ptr * ptr),
@@ -49,6 +49,8 @@ Program Definition bst_remove_root_no_right : bst_remove_root_no_right_type :=
   Fix (fun (bst_remove_root_no_right : bst_remove_root_no_right_type) vprogs =>
     let: (x, retv) := vprogs in
     Do (
+      unused2 <-- @read ptr retv;
+      v2 <-- @read nat x;
       l2 <-- @read ptr (x .+ 1);
       if l2 == null
       then
@@ -62,6 +64,9 @@ Program Definition bst_remove_root_no_right : bst_remove_root_no_right_type :=
         else
           ret tt
       else
+        vl22 <-- @read nat l2;
+        ll22 <-- @read ptr (l2 .+ 1);
+        rl22 <-- @read ptr (l2 .+ 2);
         if null == null
         then
           dealloc x;;
@@ -75,24 +80,86 @@ Program Definition bst_remove_root_no_right : bst_remove_root_no_right_type :=
 Obligation Tactic := intro; move=>[x retv]; ssl_program_simpl.
 Next Obligation.
 ssl_ghostelim_pre.
-move=>[[[[[[[[[sz1 sz2] v2] hi1] r] lo2] l2] lo1] hi2] unused2].
-ex_elim h_bst_l2sz1lo1hi1_a h_bst_rsz2lo2hi2_b.
+move=>[[[[[[[[[sz1 sz2] v] hi1] r] lo2] l] lo1] hi2] unused].
+ex_elim h_bst_lsz1lo1hi1_a h_bst_rsz2lo2hi2_b.
 move=>[phi_self0] [phi_self1] [phi_self2] [phi_self3] [phi_self4] [phi_self5] [phi_self6].
 move=>[sigma_self].
 subst h_self.
-move=>[H_bst_l2sz1lo1hi1_a H_bst_rsz2lo2hi2_b].
+move=>[H_bst_lsz1lo1hi1_a H_bst_rsz2lo2hi2_b].
 ssl_ghostelim_post.
+try rename h_bst_rsz2lo2hi2_b into h_bst_sz2lo2hi2_b.
+try rename H_bst_rsz2lo2hi2_b into H_bst_sz2lo2hi2_b.
+try rename h_bst_yn1lohi_c into h_bst_yn1lolhi1hi2_c.
+try rename H_bst_yn1lohi_c into H_bst_yn1lolhi1hi2_c.
+try rename h_bst_yn1lolhi1hi2_c into h_bst_yn1llo2lo1lhi1hi2_c.
+try rename H_bst_yn1lolhi1hi2_c into H_bst_yn1llo2lo1lhi1hi2_c.
+try rename h_bst_yn1llo2lo1lhi1hi2_c into h_bst_ysz1sz2llo2lo1lhi1hi2_c.
+try rename H_bst_yn1llo2lo1lhi1hi2_c into H_bst_ysz1sz2llo2lo1lhi1hi2_c.
+ssl_read retv.
+try rename unused into unused2.
+ssl_read x.
+try rename v into v2.
 ssl_read (x .+ 1).
-ssl_open (l2 == null);
-ssl_open_post H_bst_l2sz1lo1hi1_a.
+try rename l into l2.
+try rename h_bst_lsz1lo1hi1_a into h_bst_l2sz1lo1hi1_a.
+try rename H_bst_lsz1lo1hi1_a into H_bst_l2sz1lo1hi1_a.
+try rename h_bst_ysz1sz2llo2lo1lhi1hi2_c into h_bst_ysz1sz2l2lo2lo1l2hi1hi2_c.
+try rename H_bst_ysz1sz2llo2lo1lhi1hi2_c into H_bst_ysz1sz2l2lo2lo1l2hi1hi2_c.
+ssl_open (l2 == null) H_bst_l2sz1lo1hi1_a.
 move=>[phi_bst_l2sz1lo1hi1_a0] [phi_bst_l2sz1lo1hi1_a1] [phi_bst_l2sz1lo1hi1_a2].
 move=>[sigma_bst_l2sz1lo1hi1_a].
 subst h_bst_l2sz1lo1hi1_a.
-ssl_open (null == null);
-ssl_open_post H_bst_rsz2lo2hi2_b.
-move=>[phi_bst_rsz2lo2hi2_b0] [phi_bst_rsz2lo2hi2_b1] [phi_bst_rsz2lo2hi2_b2].
-move=>[sigma_bst_rsz2lo2hi2_b].
-subst h_bst_rsz2lo2hi2_b.
+shelve.
+ex_elim sz1l2 sz2l2 vl2 hi2l2 hi1l2.
+ex_elim lo1l2 lo2l2 ll2 rl2.
+ex_elim h_bst_ll2sz1l2lo1l2hi1l2_523l2 h_bst_rl2sz2l2lo2l2hi2l2_524l2.
+move=>[phi_bst_l2sz1lo1hi1_a0] [phi_bst_l2sz1lo1hi1_a1] [phi_bst_l2sz1lo1hi1_a2] [phi_bst_l2sz1lo1hi1_a3] [phi_bst_l2sz1lo1hi1_a4] [phi_bst_l2sz1lo1hi1_a5] [phi_bst_l2sz1lo1hi1_a6] [phi_bst_l2sz1lo1hi1_a7] [phi_bst_l2sz1lo1hi1_a8].
+move=>[sigma_bst_l2sz1lo1hi1_a].
+subst h_bst_l2sz1lo1hi1_a.
+move=>[H_bst_ll2sz1l2lo1l2hi1l2_523l2 H_bst_rl2sz2l2lo2l2hi2l2_524l2].
+shelve.
+Unshelve.
+try rename h_bst_ysz1sz2l2lo2lo1l2hi1hi2_c into h_bst_ysz1sz2l2lo2lo1l2hi2_c.
+try rename H_bst_ysz1sz2l2lo2lo1l2hi1hi2_c into H_bst_ysz1sz2l2lo2lo1l2hi2_c.
+try rename h_bst_l2sz1lo1hi1_a into h_bst_l2sz1lo1_a.
+try rename H_bst_l2sz1lo1hi1_a into H_bst_l2sz1lo1_a.
+try rename h_bst_ysz1sz2l2lo2lo1l2hi2_c into h_bst_ysz1sz2l2lo2l2hi2_c.
+try rename H_bst_ysz1sz2l2lo2lo1l2hi2_c into H_bst_ysz1sz2l2lo2l2hi2_c.
+try rename h_bst_l2sz1lo1_a into h_bst_l2sz1_a.
+try rename H_bst_l2sz1lo1_a into H_bst_l2sz1_a.
+try rename h_bst_l2sz1_a into h_bst_l2_a.
+try rename H_bst_l2sz1_a into H_bst_l2_a.
+try rename h_bst_ysz1sz2l2lo2l2hi2_c into h_bst_ysz2l2lo2l2hi2_c.
+try rename H_bst_ysz1sz2l2lo2l2hi2_c into H_bst_ysz2l2lo2l2hi2_c.
+ssl_open (null == null) H_bst_sz2lo2hi2_b.
+move=>[phi_bst_sz2lo2hi2_b0] [phi_bst_sz2lo2hi2_b1] [phi_bst_sz2lo2hi2_b2].
+move=>[sigma_bst_sz2lo2hi2_b].
+subst h_bst_sz2lo2hi2_b.
+shelve.
+ex_elim sz10 sz20 v0 hi20 hi10.
+ex_elim lo10 lo20 l0 r0.
+ex_elim h_bst_l0sz10lo10hi10_5230 h_bst_r0sz20lo20hi20_5240.
+move=>[phi_bst_sz2lo2hi2_b0] [phi_bst_sz2lo2hi2_b1] [phi_bst_sz2lo2hi2_b2] [phi_bst_sz2lo2hi2_b3] [phi_bst_sz2lo2hi2_b4] [phi_bst_sz2lo2hi2_b5] [phi_bst_sz2lo2hi2_b6] [phi_bst_sz2lo2hi2_b7] [phi_bst_sz2lo2hi2_b8].
+move=>[sigma_bst_sz2lo2hi2_b].
+subst h_bst_sz2lo2hi2_b.
+move=>[H_bst_l0sz10lo10hi10_5230 H_bst_r0sz20lo20hi20_5240].
+shelve.
+shelve.
+Unshelve.
+try rename h_bst_ysz2l2lo2l2hi2_c into h_bst_ysz2l2lo2l2_c.
+try rename H_bst_ysz2l2lo2l2hi2_c into H_bst_ysz2l2lo2l2_c.
+try rename h_bst_sz2lo2hi2_b into h_bst_sz2lo2_b.
+try rename H_bst_sz2lo2hi2_b into H_bst_sz2lo2_b.
+try rename h_bst_sz2lo2_b into h_bst_sz2_b.
+try rename H_bst_sz2lo2_b into H_bst_sz2_b.
+try rename h_bst_ysz2l2lo2l2_c into h_bst_ysz2l2l2_c.
+try rename H_bst_ysz2l2lo2l2_c into H_bst_ysz2l2l2_c.
+try rename h_bst_sz2_b into h_bst__b.
+try rename H_bst_sz2_b into H_bst__b.
+try rename h_bst_ysz2l2l2_c into h_bst_yl2l2_c.
+try rename H_bst_ysz2l2l2_c into H_bst_yl2l2_c.
+try rename h_bst_yl2l2_c into h_bst_l2l2_c.
+try rename H_bst_yl2l2_c into H_bst_l2l2_c.
 ssl_dealloc x.
 ssl_dealloc (x .+ 1).
 ssl_dealloc (x .+ 2).
@@ -101,22 +168,84 @@ ssl_write_post retv.
 ssl_emp;
 exists ((if null == null then (if l2 == null then 0 else 0) else 0)), ((if l2 == null then (if null == null then 7 else 7) else 7)), (0 + 0), (null);
 exists (empty);
-sslauto;
-solve [
+sslauto.
 unfold_constructor 1;
-sslauto ].
-ex_elim sz1l2 sz2l2 vl22 hi2l2 hi1l2.
-ex_elim lo1l2 lo2l2 ll22 rl22.
-ex_elim h_bst_ll22sz1l2lo1l2hi1l2_572l2 h_bst_rl22sz2l2lo2l2hi2l2_573l2.
-move=>[phi_bst_l2sz1lo1hi1_a0] [phi_bst_l2sz1lo1hi1_a1] [phi_bst_l2sz1lo1hi1_a2] [phi_bst_l2sz1lo1hi1_a3] [phi_bst_l2sz1lo1hi1_a4] [phi_bst_l2sz1lo1hi1_a5] [phi_bst_l2sz1lo1hi1_a6] [phi_bst_l2sz1lo1hi1_a7] [phi_bst_l2sz1lo1hi1_a8].
-move=>[sigma_bst_l2sz1lo1hi1_a].
-subst h_bst_l2sz1lo1hi1_a.
-move=>[H_bst_ll22sz1l2lo1l2hi1l2_572l2 H_bst_rl22sz2l2lo2l2hi2l2_573l2].
-ssl_open (null == null);
-ssl_open_post H_bst_rsz2lo2hi2_b.
-move=>[phi_bst_rsz2lo2hi2_b0] [phi_bst_rsz2lo2hi2_b1] [phi_bst_rsz2lo2hi2_b2].
-move=>[sigma_bst_rsz2lo2hi2_b].
-subst h_bst_rsz2lo2hi2_b.
+sslauto.
+ssl_inconsistency.
+try rename h_bst_ysz1sz2l2lo2lo1l2hi1hi2_c into h_bst_ysz1sz2l2lo2lo1l2hi2l2vl2vl2hi2l2hi2_c.
+try rename H_bst_ysz1sz2l2lo2lo1l2hi1hi2_c into H_bst_ysz1sz2l2lo2lo1l2hi2l2vl2vl2hi2l2hi2_c.
+try rename h_bst_l2sz1lo1hi1_a into h_bst_l2sz1lo1hi2l2vl2vl2hi2l2_a.
+try rename H_bst_l2sz1lo1hi1_a into H_bst_l2sz1lo1hi2l2vl2vl2hi2l2_a.
+try rename h_bst_ysz1sz2l2lo2lo1l2hi2l2vl2vl2hi2l2hi2_c into h_bst_ysz1sz2l2lo2vl2lo1l2vl2lo1l2l2hi2l2vl2vl2hi2l2hi2_c.
+try rename H_bst_ysz1sz2l2lo2lo1l2hi2l2vl2vl2hi2l2hi2_c into H_bst_ysz1sz2l2lo2vl2lo1l2vl2lo1l2l2hi2l2vl2vl2hi2l2hi2_c.
+try rename h_bst_l2sz1lo1hi2l2vl2vl2hi2l2_a into h_bst_l2sz1vl2lo1l2vl2lo1l2hi2l2vl2vl2hi2l2_a.
+try rename H_bst_l2sz1lo1hi2l2vl2vl2hi2l2_a into H_bst_l2sz1vl2lo1l2vl2lo1l2hi2l2vl2vl2hi2l2_a.
+try rename h_bst_ysz1sz2l2lo2vl2lo1l2vl2lo1l2l2hi2l2vl2vl2hi2l2hi2_c into h_bst_ysz1l2sz2l2sz2l2lo2vl2lo1l2vl2lo1l2l2hi2l2vl2vl2hi2l2hi2_c.
+try rename H_bst_ysz1sz2l2lo2vl2lo1l2vl2lo1l2l2hi2l2vl2vl2hi2l2hi2_c into H_bst_ysz1l2sz2l2sz2l2lo2vl2lo1l2vl2lo1l2l2hi2l2vl2vl2hi2l2hi2_c.
+try rename h_bst_l2sz1vl2lo1l2vl2lo1l2hi2l2vl2vl2hi2l2_a into h_bst_l2sz1l2sz2l2vl2lo1l2vl2lo1l2hi2l2vl2vl2hi2l2_a.
+try rename H_bst_l2sz1vl2lo1l2vl2lo1l2hi2l2vl2vl2hi2l2_a into H_bst_l2sz1l2sz2l2vl2lo1l2vl2lo1l2hi2l2vl2vl2hi2l2_a.
+ssl_read l2.
+try rename vl2 into vl22.
+try rename h_bst_l2sz1l2sz2l2vl2lo1l2vl2lo1l2hi2l2vl2vl2hi2l2_a into h_bst_l2sz1l2sz2l2vl22lo1l2vl22lo1l2hi2l2vl22vl22hi2l2_a.
+try rename H_bst_l2sz1l2sz2l2vl2lo1l2vl2lo1l2hi2l2vl2vl2hi2l2_a into H_bst_l2sz1l2sz2l2vl22lo1l2vl22lo1l2hi2l2vl22vl22hi2l2_a.
+try rename h_bst_ysz1l2sz2l2sz2l2lo2vl2lo1l2vl2lo1l2l2hi2l2vl2vl2hi2l2hi2_c into h_bst_ysz1l2sz2l2sz2l2lo2vl22lo1l2vl22lo1l2l2hi2l2vl22vl22hi2l2hi2_c.
+try rename H_bst_ysz1l2sz2l2sz2l2lo2vl2lo1l2vl2lo1l2l2hi2l2vl2vl2hi2l2hi2_c into H_bst_ysz1l2sz2l2sz2l2lo2vl22lo1l2vl22lo1l2l2hi2l2vl22vl22hi2l2hi2_c.
+ssl_read (l2 .+ 1).
+try rename ll2 into ll22.
+try rename h_bst_ll2sz1l2lo1l2hi1l2_523l2 into h_bst_ll22sz1l2lo1l2hi1l2_523l2.
+try rename H_bst_ll2sz1l2lo1l2hi1l2_523l2 into H_bst_ll22sz1l2lo1l2hi1l2_523l2.
+ssl_read (l2 .+ 2).
+try rename rl2 into rl22.
+try rename h_bst_rl2sz2l2lo2l2hi2l2_524l2 into h_bst_rl22sz2l2lo2l2hi2l2_524l2.
+try rename H_bst_rl2sz2l2lo2l2hi2l2_524l2 into H_bst_rl22sz2l2lo2l2hi2l2_524l2.
+ssl_open (null == null) H_bst_sz2lo2hi2_b.
+move=>[phi_bst_sz2lo2hi2_b0] [phi_bst_sz2lo2hi2_b1] [phi_bst_sz2lo2hi2_b2].
+move=>[sigma_bst_sz2lo2hi2_b].
+subst h_bst_sz2lo2hi2_b.
+shelve.
+ex_elim sz10 sz20 v0 hi20 hi10.
+ex_elim lo10 lo20 l0 r0.
+ex_elim h_bst_l0sz10lo10hi10_5230 h_bst_r0sz20lo20hi20_5240.
+move=>[phi_bst_sz2lo2hi2_b0] [phi_bst_sz2lo2hi2_b1] [phi_bst_sz2lo2hi2_b2] [phi_bst_sz2lo2hi2_b3] [phi_bst_sz2lo2hi2_b4] [phi_bst_sz2lo2hi2_b5] [phi_bst_sz2lo2hi2_b6] [phi_bst_sz2lo2hi2_b7] [phi_bst_sz2lo2hi2_b8].
+move=>[sigma_bst_sz2lo2hi2_b].
+subst h_bst_sz2lo2hi2_b.
+move=>[H_bst_l0sz10lo10hi10_5230 H_bst_r0sz20lo20hi20_5240].
+shelve.
+Unshelve.
+try rename h_bst_sz2lo2hi2_b into h_bst_sz2lo2_b.
+try rename H_bst_sz2lo2hi2_b into H_bst_sz2lo2_b.
+try rename h_bst_ysz1l2sz2l2sz2l2lo2vl22lo1l2vl22lo1l2l2hi2l2vl22vl22hi2l2hi2_c into h_bst_ysz1l2sz2l2sz2l2lo2vl22lo1l2vl22lo1l2l2hi2l2vl22vl22hi2l2_c.
+try rename H_bst_ysz1l2sz2l2sz2l2lo2vl22lo1l2vl22lo1l2l2hi2l2vl22vl22hi2l2hi2_c into H_bst_ysz1l2sz2l2sz2l2lo2vl22lo1l2vl22lo1l2l2hi2l2vl22vl22hi2l2_c.
+try rename h_bst_ysz1l2sz2l2sz2l2lo2vl22lo1l2vl22lo1l2l2hi2l2vl22vl22hi2l2_c into h_bst_ysz1l2sz2l2sz2l2vl22lo1l2vl22lo1l2l2hi2l2vl22vl22hi2l2_c.
+try rename H_bst_ysz1l2sz2l2sz2l2lo2vl22lo1l2vl22lo1l2l2hi2l2vl22vl22hi2l2_c into H_bst_ysz1l2sz2l2sz2l2vl22lo1l2vl22lo1l2l2hi2l2vl22vl22hi2l2_c.
+try rename h_bst_sz2lo2_b into h_bst_sz2_b.
+try rename H_bst_sz2lo2_b into H_bst_sz2_b.
+try rename h_bst_sz2_b into h_bst__b.
+try rename H_bst_sz2_b into H_bst__b.
+try rename h_bst_ysz1l2sz2l2sz2l2vl22lo1l2vl22lo1l2l2hi2l2vl22vl22hi2l2_c into h_bst_ysz1l2sz2l2l2vl22lo1l2vl22lo1l2l2hi2l2vl22vl22hi2l2_c.
+try rename H_bst_ysz1l2sz2l2sz2l2vl22lo1l2vl22lo1l2l2hi2l2vl22vl22hi2l2_c into H_bst_ysz1l2sz2l2l2vl22lo1l2vl22lo1l2l2hi2l2vl22vl22hi2l2_c.
+try rename h_bst_l1ysz11ylo11yhi11y_523y into h_bst_l1ysz11ylo11yhi11y_523l2.
+try rename H_bst_l1ysz11ylo11yhi11y_523y into H_bst_l1ysz11ylo11yhi11y_523l2.
+try rename h_bst_l1ysz11ylo11yhi11y_523l2 into h_bst_l1ysz11ylo11yhi1l2_523l2.
+try rename H_bst_l1ysz11ylo11yhi11y_523l2 into H_bst_l1ysz11ylo11yhi1l2_523l2.
+try rename h_bst_l1ysz11ylo11yhi1l2_523l2 into h_bst_ll22sz11ylo11yhi1l2_523l2.
+try rename H_bst_l1ysz11ylo11yhi1l2_523l2 into H_bst_ll22sz11ylo11yhi1l2_523l2.
+try rename h_bst_ll22sz11ylo11yhi1l2_523l2 into h_bst_ll22sz11ylo1l2hi1l2_523l2.
+try rename H_bst_ll22sz11ylo11yhi1l2_523l2 into H_bst_ll22sz11ylo1l2hi1l2_523l2.
+try rename h_bst_ll22sz11ylo1l2hi1l2_523l2 into h_bst_ll22sz1l2lo1l2hi1l2_523l2.
+try rename H_bst_ll22sz11ylo1l2hi1l2_523l2 into H_bst_ll22sz1l2lo1l2hi1l2_523l2.
+try rename h_bst_r1ysz21ylo21yhi21y_524y into h_bst_r1ysz21ylo21yhi21y_524l2.
+try rename H_bst_r1ysz21ylo21yhi21y_524y into H_bst_r1ysz21ylo21yhi21y_524l2.
+try rename h_bst_r1ysz21ylo21yhi21y_524l2 into h_bst_r1ysz21ylo21yhi2l2_524l2.
+try rename H_bst_r1ysz21ylo21yhi21y_524l2 into H_bst_r1ysz21ylo21yhi2l2_524l2.
+try rename h_bst_r1ysz21ylo21yhi2l2_524l2 into h_bst_r1ysz21ylo2l2hi2l2_524l2.
+try rename H_bst_r1ysz21ylo21yhi2l2_524l2 into H_bst_r1ysz21ylo2l2hi2l2_524l2.
+try rename h_bst_r1ysz21ylo2l2hi2l2_524l2 into h_bst_rl22sz21ylo2l2hi2l2_524l2.
+try rename H_bst_r1ysz21ylo2l2hi2l2_524l2 into H_bst_rl22sz21ylo2l2hi2l2_524l2.
+try rename h_bst_rl22sz21ylo2l2hi2l2_524l2 into h_bst_rl22sz2l2lo2l2hi2l2_524l2.
+try rename H_bst_rl22sz21ylo2l2hi2l2_524l2 into H_bst_rl22sz2l2lo2l2hi2l2_524l2.
+try rename h_bst_ysz1l2sz2l2l2vl22lo1l2vl22lo1l2l2hi2l2vl22vl22hi2l2_c into h_bst_l2sz1l2sz2l2l2vl22lo1l2vl22lo1l2l2hi2l2vl22vl22hi2l2_c.
+try rename H_bst_ysz1l2sz2l2l2vl22lo1l2vl22lo1l2l2hi2l2vl22vl22hi2l2_c into H_bst_l2sz1l2sz2l2l2vl22lo1l2vl22lo1l2l2hi2l2vl22vl22hi2l2_c.
 ssl_dealloc x.
 ssl_dealloc (x .+ 1).
 ssl_dealloc (x .+ 2).
@@ -124,12 +253,10 @@ ssl_write retv.
 ssl_write_post retv.
 ssl_emp;
 exists ((if null == null then (if l2 == null then 0 else (if hi2l2 <= vl22 then vl22 else hi2l2)) else 0)), ((if l2 == null then (if null == null then 7 else 7) else (if vl22 <= lo1l2 then vl22 else lo1l2))), (1 + sz1l2 + sz2l2 + 0), (l2);
-exists (l2 :-> vl22 \+ l2 .+ 1 :-> ll22 \+ l2 .+ 2 :-> rl22 \+ h_bst_ll22sz1l2lo1l2hi1l2_572l2 \+ h_bst_rl22sz2l2lo2l2hi2l2_573l2);
-sslauto;
-solve [
+exists (l2 :-> vl22 \+ l2 .+ 1 :-> ll22 \+ l2 .+ 2 :-> rl22 \+ h_bst_ll22sz1l2lo1l2hi1l2_523l2 \+ h_bst_rl22sz2l2lo2l2hi2l2_524l2);
+sslauto.
 unfold_constructor 2;
-exists (sz1l2), (sz2l2), (vl22), (hi2l2), (hi1l2), (lo1l2), (lo2l2), (ll22), (rl22);
-exists (h_bst_ll22sz1l2lo1l2hi1l2_572l2);
-exists (h_bst_rl22sz2l2lo2l2hi2l2_573l2);
-sslauto ].
+exists (sz1l2), (sz2l2), (vl22), (hi2l2), (hi1l2), (lo1l2), (lo2l2), (ll22), (rl22), (h_bst_ll22sz1l2lo1l2hi1l2_523l2), (h_bst_rl22sz2l2lo2l2hi2l2_524l2);
+sslauto.
+ssl_inconsistency.
 Qed.
