examples/bst_right_rotate.v
@@ -12,17 +12,17 @@ Inductive bst (x : ptr) (sz : nat) (lo : nat) (hi : nat) (h : heap) : Prop :=
   hi == 0 /\ lo == 7 /\ sz == 0 /\ h = empty
 | bst_2 of (x == null) = false of
   exists (sz1 : nat) (sz2 : nat) (v : nat) (hi2 : nat) (hi1 : nat) (lo1 : nat) (lo2 : nat) (l : ptr) (r : ptr),
-  exists h_bst_lsz1lo1hi1_574 h_bst_rsz2lo2hi2_575,
-  0 <= sz1 /\ 0 <= sz2 /\ 0 <= v /\ hi == (if hi2 <= v then v else hi2) /\ hi1 <= v /\ lo == (if v <= lo1 then v else lo1) /\ sz == 1 + sz1 + sz2 /\ v <= 7 /\ v <= lo2 /\ h = x :-> v \+ x .+ 1 :-> l \+ x .+ 2 :-> r \+ h_bst_lsz1lo1hi1_574 \+ h_bst_rsz2lo2hi2_575 /\ bst l sz1 lo1 hi1 h_bst_lsz1lo1hi1_574 /\ bst r sz2 lo2 hi2 h_bst_rsz2lo2hi2_575.
+  exists h_bst_lsz1lo1hi1_525 h_bst_rsz2lo2hi2_526,
+  0 <= sz1 /\ 0 <= sz2 /\ 0 <= v /\ hi == (if hi2 <= v then v else hi2) /\ hi1 <= v /\ lo == (if v <= lo1 then v else lo1) /\ sz == 1 + sz1 + sz2 /\ v <= 7 /\ v <= lo2 /\ h = x :-> v \+ x .+ 1 :-> l \+ x .+ 2 :-> r \+ h_bst_lsz1lo1hi1_525 \+ h_bst_rsz2lo2hi2_526 /\ bst l sz1 lo1 hi1 h_bst_lsz1lo1hi1_525 /\ bst r sz2 lo2 hi2 h_bst_rsz2lo2hi2_526.
 
-Lemma pure88 sz1l2 sz2l2 sz2 : 0 <= sz2l2 -> 0 <= sz2 -> 0 <= 1 + sz1l2 + sz2l2 -> 0 <= sz1l2 -> sz1l2 + 1 + sz2l2 + sz2 == 1 + sz1l2 + sz2l2 + sz2. Admitted.
-Hint Resolve pure88: ssl_pure.
-Lemma pure89 sz2l2 sz2 sz1l2 : 0 <= sz2l2 -> 0 <= sz2 -> 0 <= 1 + sz1l2 + sz2l2 -> 0 <= sz1l2 -> 0 <= 1 + sz2l2 + sz2. Admitted.
-Hint Resolve pure89: ssl_pure.
-Lemma pure90 lo2l2 v2 vl22 hi2l2 lo2 hi1l2 : (if hi2l2 <= vl22 then vl22 else hi2l2) <= v2 -> hi1l2 <= vl22 -> vl22 <= 7 -> 0 <= v2 -> v2 <= lo2 -> 0 <= vl22 -> vl22 <= lo2l2 -> v2 <= 7 -> hi2l2 <= v2. Admitted.
-Hint Resolve pure90: ssl_pure.
-Lemma pure91 lo2l2 v2 vl22 hi2l2 lo2 hi1l2 : (if hi2l2 <= vl22 then vl22 else hi2l2) <= v2 -> hi1l2 <= vl22 -> vl22 <= 7 -> 0 <= v2 -> v2 <= lo2 -> 0 <= vl22 -> vl22 <= lo2l2 -> v2 <= 7 -> vl22 <= (if v2 <= lo2l2 then v2 else lo2l2). Admitted.
-Hint Resolve pure91: ssl_pure.
+Lemma pure39 sz2l2 sz2 sz1l2 : 0 <= sz2l2 -> 0 <= sz2 -> 0 <= 1 + sz1l2 + sz2l2 -> 0 <= sz1l2 -> 0 <= 1 + sz2l2 + sz2. Admitted.
+Hint Resolve pure39: ssl_pure.
+Lemma pure40 sz1l2 sz2l2 sz2 : 0 <= sz2l2 -> 0 <= sz2 -> 0 <= 1 + sz1l2 + sz2l2 -> 0 <= sz1l2 -> sz1l2 + 1 + sz2l2 + sz2 == 1 + sz1l2 + sz2l2 + sz2. Admitted.
+Hint Resolve pure40: ssl_pure.
+Lemma pure41 lo2l2 v2 vl22 hi2l2 lo2 hi1l2 : (if hi2l2 <= vl22 then vl22 else hi2l2) <= v2 -> hi1l2 <= vl22 -> vl22 <= 7 -> 0 <= v2 -> v2 <= lo2 -> 0 <= vl22 -> vl22 <= lo2l2 -> v2 <= 7 -> hi2l2 <= v2. Admitted.
+Hint Resolve pure41: ssl_pure.
+Lemma pure42 lo2l2 v2 vl22 hi2l2 lo2 hi1l2 : (if hi2l2 <= vl22 then vl22 else hi2l2) <= v2 -> hi1l2 <= vl22 -> vl22 <= 7 -> 0 <= v2 -> v2 <= lo2 -> 0 <= vl22 -> vl22 <= lo2l2 -> v2 <= 7 -> vl22 <= (if v2 <= lo2l2 then v2 else lo2l2). Admitted.
+Hint Resolve pure42: ssl_pure.
 
 Definition bst_right_rotate_type :=
   forall (vprogs : ptr * ptr),
@@ -37,19 +37,24 @@ Definition bst_right_rotate_type :=
       let: (x, retv) := vprogs in
       let: (sz1, sz2, v, hi1, l, lo2, lo1, r, hi2, unused) := vghosts in
       exists sz3 sz4 v3 hi3 lo4 l3 lo3 hi4 y,
-      exists h_bst_l3sz3lo3hi3_576 h_bst_xsz4lo4hi4_577,
-      0 <= sz3 /\ 0 <= sz4 /\ 0 <= v3 /\ hi3 <= v3 /\ sz3 + sz4 == sz1 + sz2 /\ v3 <= 7 /\ v3 <= lo4 /\ h = retv :-> y \+ y :-> v3 \+ y .+ 1 :-> l3 \+ y .+ 2 :-> x \+ h_bst_l3sz3lo3hi3_576 \+ h_bst_xsz4lo4hi4_577 /\ bst l3 sz3 lo3 hi3 h_bst_l3sz3lo3hi3_576 /\ bst x sz4 lo4 hi4 h_bst_xsz4lo4hi4_577
+      exists h_bst_l3sz3lo3hi3_527 h_bst_xsz4lo4hi4_528,
+      0 <= sz3 /\ 0 <= sz4 /\ 0 <= v3 /\ hi3 <= v3 /\ sz3 + sz4 == sz1 + sz2 /\ v3 <= 7 /\ v3 <= lo4 /\ h = retv :-> y \+ y :-> v3 \+ y .+ 1 :-> l3 \+ y .+ 2 :-> x \+ h_bst_l3sz3lo3hi3_527 \+ h_bst_xsz4lo4hi4_528 /\ bst l3 sz3 lo3 hi3 h_bst_l3sz3lo3hi3_527 /\ bst x sz4 lo4 hi4 h_bst_xsz4lo4hi4_528
     ]).
 
 Program Definition bst_right_rotate : bst_right_rotate_type :=
   Fix (fun (bst_right_rotate : bst_right_rotate_type) vprogs =>
     let: (x, retv) := vprogs in
     Do (
+      unused2 <-- @read ptr retv;
+      v2 <-- @read nat x;
       l2 <-- @read ptr (x .+ 1);
+      r2 <-- @read ptr (x .+ 2);
       if l2 == null
       then
         ret tt
       else
+        vl22 <-- @read nat l2;
+        ll22 <-- @read ptr (l2 .+ 1);
         rl22 <-- @read ptr (l2 .+ 2);
         (l2 .+ 2) ::= x;;
         retv ::= l2;;
@@ -59,39 +64,116 @@ Program Definition bst_right_rotate : bst_right_rotate_type :=
 Obligation Tactic := intro; move=>[x retv]; ssl_program_simpl.
 Next Obligation.
 ssl_ghostelim_pre.
-move=>[[[[[[[[[sz1 sz2] v2] hi1] l2] lo2] lo1] r2] hi2] unused2].
-ex_elim h_bst_l2sz1lo1hi1_a h_bst_r2sz2lo2hi2_b.
+move=>[[[[[[[[[sz1 sz2] v] hi1] l] lo2] lo1] r] hi2] unused].
+ex_elim h_bst_lsz1lo1hi1_a h_bst_rsz2lo2hi2_b.
 move=>[phi_self0] [phi_self1] [phi_self2] [phi_self3] [phi_self4] [phi_self5] [phi_self6].
 move=>[sigma_self].
 subst h_self.
-move=>[H_bst_l2sz1lo1hi1_a H_bst_r2sz2lo2hi2_b].
+move=>[H_bst_lsz1lo1hi1_a H_bst_rsz2lo2hi2_b].
 ssl_ghostelim_post.
+ssl_read retv.
+try rename unused into unused2.
+ssl_read x.
+try rename v into v2.
 ssl_read (x .+ 1).
-ssl_open (l2 == null);
-ssl_open_post H_bst_l2sz1lo1hi1_a.
-ex_elim sz1l2 sz2l2 vl22 hi2l2 hi1l2.
-ex_elim lo1l2 lo2l2 ll22 rl22.
-ex_elim h_bst_ll22sz1l2lo1l2hi1l2_574l2 h_bst_rl22sz2l2lo2l2hi2l2_575l2.
+try rename l into l2.
+try rename h_bst_lsz1lo1hi1_a into h_bst_l2sz1lo1hi1_a.
+try rename H_bst_lsz1lo1hi1_a into H_bst_l2sz1lo1hi1_a.
+ssl_read (x .+ 2).
+try rename r into r2.
+try rename h_bst_rsz2lo2hi2_b into h_bst_r2sz2lo2hi2_b.
+try rename H_bst_rsz2lo2hi2_b into H_bst_r2sz2lo2hi2_b.
+ssl_open (l2 == null) H_bst_l2sz1lo1hi1_a.
+move=>[phi_bst_l2sz1lo1hi1_a0] [phi_bst_l2sz1lo1hi1_a1] [phi_bst_l2sz1lo1hi1_a2].
+move=>[sigma_bst_l2sz1lo1hi1_a].
+subst h_bst_l2sz1lo1hi1_a.
+shelve.
+ex_elim sz1l2 sz2l2 vl2 hi2l2 hi1l2.
+ex_elim lo1l2 lo2l2 ll2 rl2.
+ex_elim h_bst_ll2sz1l2lo1l2hi1l2_525l2 h_bst_rl2sz2l2lo2l2hi2l2_526l2.
 move=>[phi_bst_l2sz1lo1hi1_a0] [phi_bst_l2sz1lo1hi1_a1] [phi_bst_l2sz1lo1hi1_a2] [phi_bst_l2sz1lo1hi1_a3] [phi_bst_l2sz1lo1hi1_a4] [phi_bst_l2sz1lo1hi1_a5] [phi_bst_l2sz1lo1hi1_a6] [phi_bst_l2sz1lo1hi1_a7] [phi_bst_l2sz1lo1hi1_a8].
 move=>[sigma_bst_l2sz1lo1hi1_a].
 subst h_bst_l2sz1lo1hi1_a.
-move=>[H_bst_ll22sz1l2lo1l2hi1l2_574l2 H_bst_rl22sz2l2lo2l2hi2l2_575l2].
+move=>[H_bst_ll2sz1l2lo1l2hi1l2_525l2 H_bst_rl2sz2l2lo2l2hi2l2_526l2].
+shelve.
+Unshelve.
+ssl_inconsistency.
+try rename h_bst_l2sz1lo1hi1_a into h_bst_l2sz1lo1hi2l2vl2vl2hi2l2_a.
+try rename H_bst_l2sz1lo1hi1_a into H_bst_l2sz1lo1hi2l2vl2vl2hi2l2_a.
+try rename h_bst_l2sz1lo1hi2l2vl2vl2hi2l2_a into h_bst_l2sz1vl2lo1l2vl2lo1l2hi2l2vl2vl2hi2l2_a.
+try rename H_bst_l2sz1lo1hi2l2vl2vl2hi2l2_a into H_bst_l2sz1vl2lo1l2vl2lo1l2hi2l2vl2vl2hi2l2_a.
+try rename h_bst_l2sz1vl2lo1l2vl2lo1l2hi2l2vl2vl2hi2l2_a into h_bst_l2sz1l2sz2l2vl2lo1l2vl2lo1l2hi2l2vl2vl2hi2l2_a.
+try rename H_bst_l2sz1vl2lo1l2vl2lo1l2hi2l2vl2vl2hi2l2_a into H_bst_l2sz1l2sz2l2vl2lo1l2vl2lo1l2hi2l2vl2vl2hi2l2_a.
+ssl_read l2.
+try rename vl2 into vl22.
+try rename h_bst_l2sz1l2sz2l2vl2lo1l2vl2lo1l2hi2l2vl2vl2hi2l2_a into h_bst_l2sz1l2sz2l2vl22lo1l2vl22lo1l2hi2l2vl22vl22hi2l2_a.
+try rename H_bst_l2sz1l2sz2l2vl2lo1l2vl2lo1l2hi2l2vl2vl2hi2l2_a into H_bst_l2sz1l2sz2l2vl22lo1l2vl22lo1l2hi2l2vl22vl22hi2l2_a.
+ssl_read (l2 .+ 1).
+try rename ll2 into ll22.
+try rename h_bst_ll2sz1l2lo1l2hi1l2_525l2 into h_bst_ll22sz1l2lo1l2hi1l2_525l2.
+try rename H_bst_ll2sz1l2lo1l2hi1l2_525l2 into H_bst_ll22sz1l2lo1l2hi1l2_525l2.
 ssl_read (l2 .+ 2).
+try rename rl2 into rl22.
+try rename h_bst_rl2sz2l2lo2l2hi2l2_526l2 into h_bst_rl22sz2l2lo2l2hi2l2_526l2.
+try rename H_bst_rl2sz2l2lo2l2hi2l2_526l2 into H_bst_rl22sz2l2lo2l2hi2l2_526l2.
+try rename h_bst_xsz4lo4hi4_528 into h_bst_xsz4lo4hi21xv1xv1xhi21x_528.
+try rename H_bst_xsz4lo4hi4_528 into H_bst_xsz4lo4hi21xv1xv1xhi21x_528.
+try rename h_bst_xsz4lo4hi21xv1xv1xhi21x_528 into h_bst_xsz4v1xlo11xv1xlo11xhi21xv1xv1xhi21x_528.
+try rename H_bst_xsz4lo4hi21xv1xv1xhi21x_528 into H_bst_xsz4v1xlo11xv1xlo11xhi21xv1xv1xhi21x_528.
+try rename h_bst_xsz4v1xlo11xv1xlo11xhi21xv1xv1xhi21x_528 into h_bst_xsz11xsz21xv1xlo11xv1xlo11xhi21xv1xv1xhi21x_528.
+try rename H_bst_xsz4v1xlo11xv1xlo11xhi21xv1xv1xhi21x_528 into H_bst_xsz11xsz21xv1xlo11xv1xlo11xhi21xv1xv1xhi21x_528.
+try rename h_bst_l3sz3lo3hi3_527 into h_bst_l3sz3lo3hi3_525l2.
+try rename H_bst_l3sz3lo3hi3_527 into H_bst_l3sz3lo3hi3_525l2.
+try rename h_bst_l3sz3lo3hi3_525l2 into h_bst_l3sz3lo3hi1l2_525l2.
+try rename H_bst_l3sz3lo3hi3_525l2 into H_bst_l3sz3lo3hi1l2_525l2.
+try rename h_bst_l3sz3lo3hi1l2_525l2 into h_bst_ll22sz3lo3hi1l2_525l2.
+try rename H_bst_l3sz3lo3hi1l2_525l2 into H_bst_ll22sz3lo3hi1l2_525l2.
+try rename h_bst_ll22sz3lo3hi1l2_525l2 into h_bst_ll22sz3lo1l2hi1l2_525l2.
+try rename H_bst_ll22sz3lo3hi1l2_525l2 into H_bst_ll22sz3lo1l2hi1l2_525l2.
+try rename h_bst_ll22sz3lo1l2hi1l2_525l2 into h_bst_ll22sz1l2lo1l2hi1l2_525l2.
+try rename H_bst_ll22sz3lo1l2hi1l2_525l2 into H_bst_ll22sz1l2lo1l2hi1l2_525l2.
+try rename h_bst_l1xsz11xlo11xhi11x_525x into h_bst_l1xsz11xlo11xhi11x_526l2.
+try rename H_bst_l1xsz11xlo11xhi11x_525x into H_bst_l1xsz11xlo11xhi11x_526l2.
+try rename h_bst_l1xsz11xlo11xhi11x_526l2 into h_bst_l1xsz11xlo11xhi2l2_526l2.
+try rename H_bst_l1xsz11xlo11xhi11x_526l2 into H_bst_l1xsz11xlo11xhi2l2_526l2.
+try rename h_bst_l1xsz11xlo11xhi2l2_526l2 into h_bst_rl22sz11xlo11xhi2l2_526l2.
+try rename H_bst_l1xsz11xlo11xhi2l2_526l2 into H_bst_rl22sz11xlo11xhi2l2_526l2.
+try rename h_bst_rl22sz11xlo11xhi2l2_526l2 into h_bst_rl22sz11xlo2l2hi2l2_526l2.
+try rename H_bst_rl22sz11xlo11xhi2l2_526l2 into H_bst_rl22sz11xlo2l2hi2l2_526l2.
+try rename h_bst_xsz11xsz21xv1xlo11xv1xlo11xhi21xv1xv1xhi21x_528 into h_bst_xsz11xsz21xv1xlo2l2v1xlo2l2hi21xv1xv1xhi21x_528.
+try rename H_bst_xsz11xsz21xv1xlo11xv1xlo11xhi21xv1xv1xhi21x_528 into H_bst_xsz11xsz21xv1xlo2l2v1xlo2l2hi21xv1xv1xhi21x_528.
+try rename h_bst_xsz11xsz21xv1xlo2l2v1xlo2l2hi21xv1xv1xhi21x_528 into h_bst_xsz2l2sz21xv1xlo2l2v1xlo2l2hi21xv1xv1xhi21x_528.
+try rename H_bst_xsz11xsz21xv1xlo2l2v1xlo2l2hi21xv1xv1xhi21x_528 into H_bst_xsz2l2sz21xv1xlo2l2v1xlo2l2hi21xv1xv1xhi21x_528.
+try rename h_bst_rl22sz11xlo2l2hi2l2_526l2 into h_bst_rl22sz2l2lo2l2hi2l2_526l2.
+try rename H_bst_rl22sz11xlo2l2hi2l2_526l2 into H_bst_rl22sz2l2lo2l2hi2l2_526l2.
+try rename h_bst_r1xsz21xlo21xhi21x_526x into h_bst_r1xsz21xlo21xhi21x_b.
+try rename H_bst_r1xsz21xlo21xhi21x_526x into H_bst_r1xsz21xlo21xhi21x_b.
+try rename h_bst_r1xsz21xlo21xhi21x_b into h_bst_r1xsz21xlo21xhi2_b.
+try rename H_bst_r1xsz21xlo21xhi21x_b into H_bst_r1xsz21xlo21xhi2_b.
+try rename h_bst_xsz2l2sz21xv1xlo2l2v1xlo2l2hi21xv1xv1xhi21x_528 into h_bst_xsz2l2sz21xv1xlo2l2v1xlo2l2hi2v1xv1xhi2_528.
+try rename H_bst_xsz2l2sz21xv1xlo2l2v1xlo2l2hi21xv1xv1xhi21x_528 into H_bst_xsz2l2sz21xv1xlo2l2v1xlo2l2hi2v1xv1xhi2_528.
+try rename h_bst_r1xsz21xlo21xhi2_b into h_bst_r1xsz21xlo2hi2_b.
+try rename H_bst_r1xsz21xlo21xhi2_b into H_bst_r1xsz21xlo2hi2_b.
+try rename h_bst_r1xsz21xlo2hi2_b into h_bst_r2sz21xlo2hi2_b.
+try rename H_bst_r1xsz21xlo2hi2_b into H_bst_r2sz21xlo2hi2_b.
+try rename h_bst_xsz2l2sz21xv1xlo2l2v1xlo2l2hi2v1xv1xhi2_528 into h_bst_xsz2l2sz2v1xlo2l2v1xlo2l2hi2v1xv1xhi2_528.
+try rename H_bst_xsz2l2sz21xv1xlo2l2v1xlo2l2hi2v1xv1xhi2_528 into H_bst_xsz2l2sz2v1xlo2l2v1xlo2l2hi2v1xv1xhi2_528.
+try rename h_bst_r2sz21xlo2hi2_b into h_bst_r2sz2lo2hi2_b.
+try rename H_bst_r2sz21xlo2hi2_b into H_bst_r2sz2lo2hi2_b.
 ssl_write (l2 .+ 2).
 ssl_write_post (l2 .+ 2).
 ssl_write retv.
 ssl_write_post retv.
 ssl_write (x .+ 1).
 ssl_write_post (x .+ 1).
+try rename h_bst_xsz2l2sz2v1xlo2l2v1xlo2l2hi2v1xv1xhi2_528 into h_bst_xsz2l2sz2v2lo2l2v2lo2l2hi2v2v2hi2_528.
+try rename H_bst_xsz2l2sz2v1xlo2l2v1xlo2l2hi2v1xv1xhi2_528 into H_bst_xsz2l2sz2v2lo2l2v2lo2l2hi2v2v2hi2_528.
 ssl_emp;
 exists (sz1l2), (1 + sz2l2 + sz2), (vl22), (hi1l2), ((if v2 <= lo2l2 then v2 else lo2l2)), (ll22), (lo1l2), ((if hi2 <= v2 then v2 else hi2)), (l2);
-exists (h_bst_ll22sz1l2lo1l2hi1l2_574l2);
-exists (x :-> v2 \+ x .+ 1 :-> rl22 \+ x .+ 2 :-> r2 \+ h_bst_rl22sz2l2lo2l2hi2l2_575l2 \+ h_bst_r2sz2lo2hi2_b);
-sslauto;
-solve [
+exists (h_bst_ll22sz1l2lo1l2hi1l2_525l2);
+exists (x :-> v2 \+ x .+ 1 :-> rl22 \+ x .+ 2 :-> r2 \+ h_bst_rl22sz2l2lo2l2hi2l2_526l2 \+ h_bst_r2sz2lo2hi2_b);
+sslauto.
 unfold_constructor 2;
-exists (sz2l2), (sz2), (v2), (hi2), (hi2l2), (lo2l2), (lo2), (rl22), (r2);
-exists (h_bst_rl22sz2l2lo2l2hi2l2_575l2);
-exists (h_bst_r2sz2lo2hi2_b);
-sslauto ].
+exists (sz2l2), (sz2), (v2), (hi2), (hi2l2), (lo2l2), (lo2), (rl22), (r2), (h_bst_rl22sz2l2lo2l2hi2l2_526l2), (h_bst_r2sz2lo2hi2_b);
+sslauto.
 Qed.
